<?xml version="1.0"?>


<!DOCTYPE rdf:RDF [
    <!ENTITY dct "http://purl.org/dc/terms/" >
    <!ENTITY prov "http://www.w3.org/ns/prov#" >
    <!ENTITY foaf "http://xmlns.com/foaf/0.1/" >
    <!ENTITY vann "http://purl.org/vocab/vann/" >
    <!ENTITY ma-ont "http://www.w3.org/ns/ma-ont#" >
    <!ENTITY cc "http://creativecommons.org/ns#" >
    <!ENTITY owl "http://www.w3.org/2002/07/owl#" >
    <!ENTITY dc "http://purl.org/dc/elements/1.1/" >
    <!ENTITY xsd "http://www.w3.org/2001/XMLSchema#" >
    <!ENTITY owl2xml "http://www.w3.org/2006/12/owl2-xml#" >
    <!ENTITY skos "http://www.w3.org/2004/02/skos/core#" >
    <!ENTITY rdfs "http://www.w3.org/2000/01/rdf-schema#" >
    <!ENTITY rdf "http://www.w3.org/1999/02/22-rdf-syntax-ns#" >
    <!ENTITY core "http://www.bbc.co.uk/ontologies/coreconcepts/" >
    <!ENTITY vs "http://www.w3.org/2003/06/sw-vocab-status/ns#" >
    <!ENTITY ebuccdm "http://www.ebu.ch/metadata/ontologies/ebuccdm#" >
    <!ENTITY ebucore "http://www.ebu.ch/metadata/ontologies/ebucore/ebucore#" >
]>


<rdf:RDF xmlns="http://www.ebu.ch/metadata/ontologies/ebucore/ebucore#"
     xml:base="http://www.ebu.ch/metadata/ontologies/ebucore/ebucore"
     xmlns:dc="http://purl.org/dc/elements/1.1/"
     xmlns:prov="http://www.w3.org/ns/prov#"
     xmlns:foaf="http://xmlns.com/foaf/0.1/"
     xmlns:ebucore="http://www.ebu.ch/metadata/ontologies/ebucore/ebucore#"
     xmlns:vann="http://purl.org/vocab/vann/"
     xmlns:ebuccdm="http://www.ebu.ch/metadata/ontologies/ebuccdm#"
     xmlns:vs="http://www.w3.org/2003/06/sw-vocab-status/ns#"
     xmlns:ma-ont="http://www.w3.org/ns/ma-ont#"
     xmlns:rdfs="http://www.w3.org/2000/01/rdf-schema#"
     xmlns:owl2xml="http://www.w3.org/2006/12/owl2-xml#"
     xmlns:dct="http://purl.org/dc/terms/"
     xmlns:owl="http://www.w3.org/2002/07/owl#"
     xmlns:xsd="http://www.w3.org/2001/XMLSchema#"
     xmlns:rdf="http://www.w3.org/1999/02/22-rdf-syntax-ns#"
     xmlns:core="http://www.bbc.co.uk/ontologies/coreconcepts/"
     xmlns:skos="http://www.w3.org/2004/02/skos/core#"
     xmlns:cc="http://creativecommons.org/ns#">
    <owl:Ontology rdf:about="http://www.ebu.ch/metadata/ontologies/ebucore/ebucore">
        <dc:issued rdf:datatype="&xsd;date">2013-01-01</dc:issued>
        <dc:modified rdf:datatype="&xsd;date">2015-05-01</dc:modified>
        <cc:licence rdf:datatype="&xsd;string">http://creativecommons.org/licenses/by-sa/3.0/</cc:licence>
        <vann:preferredNamespaceUri rdf:datatype="&xsd;string">http://www.ebu.ch/metadata/ontologies/ebucore/ebucore#</vann:preferredNamespaceUri>
        <dc:publisher xml:lang="ch">European Broadcasting Union (EBU)</dc:publisher>
        <dc:creator xml:lang="ch">Jean Pierre Evain, EBU</dc:creator>
        <owl:versionInfo xml:lang="en">Change dc namespace from  	http://purl.org/dc/terms/  to	http://purl.org/dc/elements/1.1/ {@en} and correct dc: classes and propertes&apos; namespace accordingly.</owl:versionInfo>
        <owl:versionInfo xml:lang="en">Change properties linking to subclasses of skos:Concept from owl:objectProperties to rdf:Properties to support resources or literals.</owl:versionInfo>
        <dc:rights xml:lang="en">Copyright 2015 EBU</dc:rights>
        <dc:title xml:lang="en">EBUCore - the Dublin Core for media</dc:title>
        <owl:versionInfo xml:lang="en">EBUCore based on Dublin Core + SKOS + some BBC Core Concepts + basic FOAF properties  + equivalences to W3C MA-ONT</owl:versionInfo>
        <owl:versionInfo xml:lang="en">KeyEvents and associated subclasses have been introduced as common resources for sport and other developments.</owl:versionInfo>
        <dc:description xml:lang="en">Note to implementers: The EBUCore ontology is used by a variety of users with differnet needs. Several EBUCore properties have no range to allow different implementations using entities or literals. As an implementer, it is your choice to go for one or the other for each property to have consistent expectations when parsing individuals. EBUCore also provides different classes defined as subclasses of skos:Concept. You can use these classes as entities in range of several properties currently left without range. EBUCore is expressed in RDF in order to facilitate such modelling and flexibility. As a consequence, propoerties appear in the documentation as annotation properties.</dc:description>
        <dc:description xml:lang="en">The EBU audio model (ADM incl. existing and 3D audio formats) technical Metadata has been removed from the ontology. There was no clear business case on how such technicial metadata would be searched while making the ontology significantly heavier. This may be reintroduced in the future if the requirements evolve.</dc:description>
        <dc:description xml:lang="en">The EBUCore has been
      designed to make users benefit from the flexibility of RDF to adapt the names of Classes and
      properties to their respective needs. This means users are welcome to add their own subclasses
      (e.g. to define the most appropriate BusinessObjects or Resources or Agents) and subproperties.</dc:description>
        <owl:versionInfo xml:lang="en">Version 1.4</owl:versionInfo>
        <vs:term_status xml:lang="en">stable</vs:term_status>
        <dc:contributor xml:lang="ie">Christophe Debruyne, RIA</dc:contributor>
        <dc:contributor xml:lang="nl">Hugo Manguinhas, Europeana</dc:contributor>
        <dc:contributor xml:lang="nl">Valentine Charles, Europeana</dc:contributor>
        <dc:contributor xml:lang="no">Knut-Olav Hoven, NRK</dc:contributor>
        <dc:contributor xml:lang="no">Robert Engels, NRK</dc:contributor>
        <dc:contributor xml:lang="no">Tormod Vaervagen, NRK</dc:contributor>
        <owl:backwardCompatibleWith rdf:resource="http://www.ebu.ch/metadata/ontologies/ebucore/20150122/ebucore_2015_01_26.rdf"/>
        <owl:priorVersion rdf:resource="http://www.ebu.ch/metadata/ontologies/ebucore/20150122/ebucore_2015_01_26.rdf"/>
        <owl:imports rdf:resource="http://www.w3.org/2004/02/skos/core"/>
    </owl:Ontology>
    


    <!-- 
    ///////////////////////////////////////////////////////////////////////////////////////
    //
    // Annotation properties
    //
    ///////////////////////////////////////////////////////////////////////////////////////
     -->

    


    <!-- http://purl.org/dc/elements/1.1/alternative -->

    <owl:AnnotationProperty rdf:about="&dc;alternative">
        <rdfs:label xml:lang="en">Alternative title</rdfs:label>
        <rdfs:comment xml:lang="en">An alternative to the title.</rdfs:comment>
        <rdfs:domain rdf:resource="&ebucore;BusinessObject"/>
    </owl:AnnotationProperty>
    


    <!-- http://purl.org/dc/elements/1.1/contributor -->

    <owl:AnnotationProperty rdf:about="&dc;contributor">
        <rdfs:label xml:lang="en">Contributor</rdfs:label>
        <rdfs:comment xml:lang="en">An Agent who has participated in any phase of management of a BusinessObject or Resource.</rdfs:comment>
        <rdfs:domain rdf:resource="_:genid230"/>
    </owl:AnnotationProperty>
    


    <!-- http://purl.org/dc/elements/1.1/coverage -->

    <owl:AnnotationProperty rdf:about="&dc;coverage">
        <rdfs:label xml:lang="en">Coverage</rdfs:label>
        <rdfs:comment xml:lang="en">A property to identify the Events and or
            Locations, all real or fictional, covered by the 
            BusinessObject.</rdfs:comment>
        <rdfs:domain rdf:resource="&ebucore;BusinessObject"/>
    </owl:AnnotationProperty>
    


    <!-- http://purl.org/dc/elements/1.1/creator -->

    <owl:AnnotationProperty rdf:about="&dc;creator">
        <rdfs:label xml:lang="en">Creator</rdfs:label>
        <rdfs:comment xml:lang="en">A creator of content such as a director or a producer.</rdfs:comment>
        <rdfs:subPropertyOf rdf:resource="&dc;contributor"/>
    </owl:AnnotationProperty>
    


    <!-- http://purl.org/dc/elements/1.1/date -->

    <rdf:Description rdf:about="&dc;date">
        <rdfs:label xml:lang="en">date</rdfs:label>
        <rdfs:comment xml:lang="en">A date associated with the BusinessObject, Resource or Contact/Person.</rdfs:comment>
    </rdf:Description>
    


    <!-- http://purl.org/dc/elements/1.1/description -->

    <owl:AnnotationProperty rdf:about="&dc;description">
        <rdfs:label rdf:datatype="&xsd;string">Description</rdfs:label>
        <rdfs:comment xml:lang="en">A description of the BusinessObject or Resource.</rdfs:comment>
        <rdfs:domain rdf:resource="_:genid59"/>
    </owl:AnnotationProperty>
    


    <!-- http://purl.org/dc/elements/1.1/format -->

    <owl:AnnotationProperty rdf:about="&dc;format">
        <rdfs:label xml:lang="en">Format</rdfs:label>
        <rdfs:comment xml:lang="en">Information about the Format of a Resource.</rdfs:comment>
        <rdfs:domain rdf:resource="&ebucore;Resource"/>
    </owl:AnnotationProperty>
    


    <!-- http://purl.org/dc/elements/1.1/identifier -->

    <owl:AnnotationProperty rdf:about="&dc;identifier">
        <rdfs:label xml:lang="en">identifier</rdfs:label>
        <rdfs:comment xml:lang="en">An identifier associated with a BusinessObject or a resource.</rdfs:comment>
        <rdfs:domain rdf:resource="_:genid163"/>
    </owl:AnnotationProperty>
    


    <!-- http://purl.org/dc/elements/1.1/issued -->

    <owl:AnnotationProperty rdf:about="&dc;issued">
        <rdfs:label xml:lang="en">Issued</rdfs:label>
        <rdfs:subPropertyOf rdf:resource="&dc;date"/>
    </owl:AnnotationProperty>
    


    <!-- http://purl.org/dc/elements/1.1/language -->

    <owl:AnnotationProperty rdf:about="&dc;language">
        <rdfs:label xml:lang="en">Language</rdfs:label>
        <rdfs:comment xml:lang="en">A Languages used in the BusinessObject or Resource.</rdfs:comment>
        <rdfs:domain rdf:resource="_:genid221"/>
    </owl:AnnotationProperty>
    


    <!-- http://purl.org/dc/elements/1.1/modified -->

    <owl:AnnotationProperty rdf:about="&dc;modified">
        <rdfs:label xml:lang="en">Modified</rdfs:label>
        <rdfs:subPropertyOf rdf:resource="&dc;date"/>
    </owl:AnnotationProperty>
    


    <!-- http://purl.org/dc/elements/1.1/publisher -->

    <owl:AnnotationProperty rdf:about="&dc;publisher">
        <rdfs:label xml:lang="en">Publisher</rdfs:label>
        <rdfs:comment xml:lang="en">An Agent involved in the distribution of content.</rdfs:comment>
        <rdfs:subPropertyOf rdf:resource="&dc;contributor"/>
    </owl:AnnotationProperty>
    


    <!-- http://purl.org/dc/elements/1.1/relation -->

    <rdf:Description rdf:about="&dc;relation">
        <rdfs:label xml:lang="en">Relation</rdfs:label>
        <rdfs:comment xml:lang="en">A relation between BusinessObjects and resources.</rdfs:comment>
    </rdf:Description>
    


    <!-- http://purl.org/dc/elements/1.1/rights -->

    <owl:AnnotationProperty rdf:about="&dc;rights">
        <rdfs:label xml:lang="en">Rights</rdfs:label>
        <rdfs:comment xml:lang="en">Rights information related to an Asset, aPublicationEvent, a BusinessObject or a resource.</rdfs:comment>
        <rdfs:domain rdf:resource="_:genid50"/>
    </owl:AnnotationProperty>
    


    <!-- http://purl.org/dc/elements/1.1/source -->

    <owl:AnnotationProperty rdf:about="&dc;source">
        <rdfs:label xml:lang="en">Source</rdfs:label>
        <rdfs:comment xml:lang="en">To identify a Resource as the source of another Resource.</rdfs:comment>
        <rdfs:domain rdf:resource="&ebucore;Resource"/>
    </owl:AnnotationProperty>
    


    <!-- http://purl.org/dc/elements/1.1/subject -->

    <owl:AnnotationProperty rdf:about="&dc;subject">
        <rdfs:label xml:lang="en">Subject</rdfs:label>
        <rdfs:comment xml:lang="en">To associate a Subject or topic addressed by a
            BusinessObject / Resource.</rdfs:comment>
        <rdfs:domain rdf:resource="_:genid62"/>
    </owl:AnnotationProperty>
    


    <!-- http://purl.org/dc/elements/1.1/title -->

    <owl:AnnotationProperty rdf:about="&dc;title">
        <rdfs:label rdf:datatype="&xsd;string">Title</rdfs:label>
        <rdfs:comment xml:lang="en">The title by which a BusinessObject is known.</rdfs:comment>
        <rdfs:domain rdf:resource="_:genid44"/>
    </owl:AnnotationProperty>
    


    <!-- http://purl.org/dc/elements/1.1/type -->

    <owl:AnnotationProperty rdf:about="&dc;type">
        <rdfs:label xml:lang="en">type</rdfs:label>
        <rdfs:comment xml:lang="en">A concept associated with a BusinessObject or Resource.</rdfs:comment>
        <rdfs:domain rdf:resource="_:genid41"/>
    </owl:AnnotationProperty>
    


    <!-- http://purl.org/dc/terms/description -->

    <owl:AnnotationProperty rdf:about="&dct;description">
        <rdfs:label xml:lang="en">Description</rdfs:label>
        <rdfs:range rdf:resource="&xsd;string"/>
    </owl:AnnotationProperty>
    


    <!-- http://purl.org/dc/terms/title -->

    <owl:AnnotationProperty rdf:about="&dct;title">
        <rdfs:label xml:lang="en">Title</rdfs:label>
        <rdfs:range rdf:resource="&xsd;string"/>
    </owl:AnnotationProperty>
    


    <!-- http://www.bbc.co.uk/ontologies/coreconcepts/dateOfBirth -->

    <owl:AnnotationProperty rdf:about="&core;dateOfBirth">
        <rdfs:label xml:lang="en">Date of birth</rdfs:label>
        <rdfs:comment xml:lang="en">The date when a Contact/Person is born.</rdfs:comment>
        <rdfs:subPropertyOf rdf:resource="&dc;date"/>
        <rdfs:domain rdf:resource="&ebucore;Contact"/>
    </owl:AnnotationProperty>
    


    <!-- http://www.bbc.co.uk/ontologies/coreconcepts/dateOfDeath -->

    <owl:AnnotationProperty rdf:about="&core;dateOfDeath">
        <rdfs:label xml:lang="en">Date of death</rdfs:label>
        <rdfs:comment xml:lang="en">The date when a Contact/Person has passed away.</rdfs:comment>
        <rdfs:subPropertyOf rdf:resource="&dc;date"/>
        <rdfs:domain rdf:resource="&ebucore;Contact"/>
    </owl:AnnotationProperty>
    


    <!-- http://www.bbc.co.uk/ontologies/coreconcepts/gender -->

    <owl:AnnotationProperty rdf:about="&core;gender">
        <rdfs:label xml:lang="en">Gender</rdfs:label>
        <rdfs:comment xml:lang="en">The gender of a person e.g. male or female.</rdfs:comment>
        <rdfs:domain rdf:resource="&ebucore;Contact"/>
    </owl:AnnotationProperty>
    


    <!-- http://www.bbc.co.uk/ontologies/coreconcepts/primaryTopic -->

    <owl:AnnotationProperty rdf:about="&core;primaryTopic">
        <rdfs:label xml:lang="en">Primary topic</rdfs:label>
        <rdfs:comment xml:lang="en">The main subject of interest.</rdfs:comment>
        <rdfs:subPropertyOf rdf:resource="&dc;description"/>
    </owl:AnnotationProperty>
    


    <!-- http://www.bbc.co.uk/ontologies/coreconcepts/slug -->

    <owl:AnnotationProperty rdf:about="&core;slug">
        <rdfs:label xml:lang="en">Slug</rdfs:label>
        <rdfs:comment xml:lang="en">One or more keywords.</rdfs:comment>
        <rdfs:subPropertyOf rdf:resource="&dc;description"/>
    </owl:AnnotationProperty>
    


    <!-- http://www.ebu.ch/metadata/ontologies/ebucore/ebucore#DID -->

    <owl:AnnotationProperty rdf:about="&ebucore;DID">
        <rdfs:label xml:lang="en">DID</rdfs:label>
        <rdfs:comment xml:lang="en">The Data Identifier word (along with the SDID,
            if used), indicates the type of ancillary data that the packet corresponds
            to.</rdfs:comment>
        <rdfs:domain rdf:resource="&ebucore;AncillaryData"/>
    </owl:AnnotationProperty>
    


    <!-- http://www.ebu.ch/metadata/ontologies/ebucore/ebucore#SDID -->

    <owl:AnnotationProperty rdf:about="&ebucore;SDID">
        <rdfs:label xml:lang="en">SDID</rdfs:label>
        <rdfs:comment xml:lang="en">Secondary data identification word for
            ancillary data. Send mode identifier. An identifier which indicates the transmission
            timing for closed caption data.</rdfs:comment>
        <rdfs:domain rdf:resource="&ebucore;AncillaryData"/>
    </owl:AnnotationProperty>
    


    <!-- http://www.ebu.ch/metadata/ontologies/ebucore/ebucore#abridgedTitle -->

    <owl:AnnotationProperty rdf:about="&ebucore;abridgedTitle">
        <rdfs:label xml:lang="en">Abridged title</rdfs:label>
        <rdfs:comment xml:lang="en">A shorter version of the title.</rdfs:comment>
        <rdfs:subPropertyOf rdf:resource="&ebucore;alternativeTitle"/>
    </owl:AnnotationProperty>
    


    <!-- http://www.ebu.ch/metadata/ontologies/ebucore/ebucore#abstract -->

    <owl:AnnotationProperty rdf:about="&ebucore;abstract">
        <rdfs:label xml:lang="en">Abstract</rdfs:label>
        <rdfs:comment xml:lang="en">To provide a brief summary.</rdfs:comment>
        <rdfs:subPropertyOf rdf:resource="&ebucore;description"/>
    </owl:AnnotationProperty>
    


    <!-- http://www.ebu.ch/metadata/ontologies/ebucore/ebucore#adultContent -->

    <owl:AnnotationProperty rdf:about="&ebucore;adultContent">
        <rdfs:label rdf:datatype="&xsd;string">adult content</rdfs:label>
        <rdfs:domain rdf:resource="_:genid128"/>
    </owl:AnnotationProperty>
    


    <!-- http://www.ebu.ch/metadata/ontologies/ebucore/ebucore#agentAddress -->

    <owl:AnnotationProperty rdf:about="&ebucore;agentAddress">
        <rdfs:label xml:lang="en">Address</rdfs:label>
        <rdfs:comment xml:lang="en">To provide the address of an Agent
            (Contact/person or organisation).</rdfs:comment>
        <rdfs:domain rdf:resource="&ebucore;Agent"/>
    </owl:AnnotationProperty>
    


    <!-- http://www.ebu.ch/metadata/ontologies/ebucore/ebucore#agentAge -->

    <owl:AnnotationProperty rdf:about="&ebucore;agentAge">
        <rdfs:label xml:lang="en">Age</rdfs:label>
        <rdfs:comment rdf:datatype="&xsd;string">The age of a Contact/Person</rdfs:comment>
        <rdfs:domain rdf:resource="&ebucore;Contact"/>
    </owl:AnnotationProperty>
    


    <!-- http://www.ebu.ch/metadata/ontologies/ebucore/ebucore#agentCountryOfResidence -->

    <owl:AnnotationProperty rdf:about="&ebucore;agentCountryOfResidence">
        <rdfs:label rdf:datatype="&xsd;string">agent country of residence</rdfs:label>
        <rdfs:domain rdf:resource="&ebucore;Agent"/>
    </owl:AnnotationProperty>
    


    <!-- http://www.ebu.ch/metadata/ontologies/ebucore/ebucore#agentEmailAddress -->

    <owl:AnnotationProperty rdf:about="&ebucore;agentEmailAddress">
        <rdfs:label xml:lang="en">Email</rdfs:label>
        <rdfs:comment xml:lang="en">To provide the email address of an agent
            (Contact/person or organisation).</rdfs:comment>
        <rdfs:domain rdf:resource="&ebucore;Agent"/>
    </owl:AnnotationProperty>
    


    <!-- http://www.ebu.ch/metadata/ontologies/ebucore/ebucore#agentMobileTelephoneNumber -->

    <owl:AnnotationProperty rdf:about="&ebucore;agentMobileTelephoneNumber">
        <rdfs:label xml:lang="en">Mobile</rdfs:label>
        <rdfs:comment xml:lang="en">To provide the mobile telephone number of an
            Agent (Contact/person or organisation)</rdfs:comment>
        <rdfs:domain rdf:resource="&ebucore;Agent"/>
    </owl:AnnotationProperty>
    


    <!-- http://www.ebu.ch/metadata/ontologies/ebucore/ebucore#agentName -->

    <owl:AnnotationProperty rdf:about="&ebucore;agentName">
        <rdfs:label xml:lang="en">Name</rdfs:label>
        <rdfs:comment xml:lang="en">To provide the full name of Contact/person - family and given name.</rdfs:comment>
        <rdfs:domain rdf:resource="&ebucore;Agent"/>
    </owl:AnnotationProperty>
    


    <!-- http://www.ebu.ch/metadata/ontologies/ebucore/ebucore#agentNationality -->

    <owl:AnnotationProperty rdf:about="&ebucore;agentNationality">
        <rdfs:label rdf:datatype="&xsd;string">agent nationality</rdfs:label>
        <rdfs:domain rdf:resource="&ebucore;Agent"/>
    </owl:AnnotationProperty>
    


    <!-- http://www.ebu.ch/metadata/ontologies/ebucore/ebucore#agentNickname -->

    <owl:AnnotationProperty rdf:about="&ebucore;agentNickname">
        <rdfs:label xml:lang="en">Nickname</rdfs:label>
        <rdfs:comment xml:lang="en">To provide a nickname of a Contact/person.</rdfs:comment>
        <rdfs:domain rdf:resource="&ebucore;Agent"/>
    </owl:AnnotationProperty>
    


    <!-- http://www.ebu.ch/metadata/ontologies/ebucore/ebucore#agentPictureIdLocator -->

    <owl:AnnotationProperty rdf:about="&ebucore;agentPictureIdLocator">
        <rdfs:label rdf:datatype="&xsd;string">agent picture id locator</rdfs:label>
        <rdfs:subPropertyOf rdf:resource="&ebucore;locator"/>
    </owl:AnnotationProperty>
    


    <!-- http://www.ebu.ch/metadata/ontologies/ebucore/ebucore#agentTelephoneNumber -->

    <owl:AnnotationProperty rdf:about="&ebucore;agentTelephoneNumber">
        <rdfs:label xml:lang="en">Telephone</rdfs:label>
        <rdfs:comment xml:lang="en">To provide the telephone number of an Agent
            (Contact/person or Organisation).</rdfs:comment>
        <rdfs:domain rdf:resource="&ebucore;Agent"/>
    </owl:AnnotationProperty>
    


    <!-- http://www.ebu.ch/metadata/ontologies/ebucore/ebucore#agentWebHomepage -->

    <owl:AnnotationProperty rdf:about="&ebucore;agentWebHomepage">
        <rdfs:label xml:lang="en">Homepage</rdfs:label>
        <rdfs:comment xml:lang="en">To provide the address of the webpage of an
            Agent (Contact/person or Organisation).</rdfs:comment>
        <rdfs:domain rdf:resource="&ebucore;Agent"/>
    </owl:AnnotationProperty>
    


    <!-- http://www.ebu.ch/metadata/ontologies/ebucore/ebucore#alternativeTitle -->

    <owl:AnnotationProperty rdf:about="&ebucore;alternativeTitle">
        <rdfs:label xml:lang="en">Alternative title</rdfs:label>
        <rdfs:comment xml:lang="en">To provide an alternative title.</rdfs:comment>
        <rdfs:subPropertyOf rdf:resource="&dc;alternative"/>
    </owl:AnnotationProperty>
    


    <!-- http://www.ebu.ch/metadata/ontologies/ebucore/ebucore#appliesOutOf -->

    <owl:AnnotationProperty rdf:about="&ebucore;appliesOutOf">
        <rdfs:label xml:lang="en">Exclusion area</rdfs:label>
        <rdfs:comment xml:lang="en">To define the Location (e.g. country, region) to which Rating and TargetAudience do NOT apply.</rdfs:comment>
        <rdfs:domain rdf:resource="_:genid131"/>
    </owl:AnnotationProperty>
    


    <!-- http://www.ebu.ch/metadata/ontologies/ebucore/ebucore#appliesTo -->

    <owl:AnnotationProperty rdf:about="&ebucore;appliesTo">
        <rdfs:label xml:lang="en">Coverage</rdfs:label>
        <rdfs:comment xml:lang="en">To define the location/region to which Rating and TargetAudience apply.</rdfs:comment>
        <rdfs:domain rdf:resource="_:genid68"/>
    </owl:AnnotationProperty>
    


    <!-- http://www.ebu.ch/metadata/ontologies/ebucore/ebucore#aspectRatio -->

    <owl:AnnotationProperty rdf:about="&ebucore;aspectRatio">
        <rdfs:label xml:lang="en">Aspect ratio</rdfs:label>
        <rdfs:comment xml:lang="en">To provide the aspect ratio of a video frame or
            image. Several types of different aspect ration can apply to the same video image. If
            necessary, specialised aspect ratios can be defined as subproperties.</rdfs:comment>
        <rdfs:domain rdf:resource="_:genid33"/>
    </owl:AnnotationProperty>
    


    <!-- http://www.ebu.ch/metadata/ontologies/ebucore/ebucore#audioChannelNumber -->

    <owl:AnnotationProperty rdf:about="&ebucore;audioChannelNumber">
        <rdfs:label xml:lang="en">Audio channel number</rdfs:label>
        <rdfs:comment xml:lang="en">The total number of audio channels contained in
            the MediaResource.</rdfs:comment>
        <rdfs:domain rdf:resource="&ebucore;MediaResource"/>
    </owl:AnnotationProperty>
    


    <!-- http://www.ebu.ch/metadata/ontologies/ebucore/ebucore#audioMXFLookup -->

    <rdf:Description rdf:about="&ebucore;audioMXFLookup">
        <rdfs:label xml:lang="en">Audio MXFlookup</rdfs:label>
        <rdfs:comment xml:lang="en">The parameters for MXF mapping.</rdfs:comment>
    </rdf:Description>
    


    <!-- http://www.ebu.ch/metadata/ontologies/ebucore/ebucore#audioTrackConfiguration -->

    <owl:AnnotationProperty rdf:about="&ebucore;audioTrackConfiguration">
        <rdfs:label rdf:datatype="&xsd;string">Audio track configuration</rdfs:label>
        <rdfs:comment xml:lang="en">To provide the configuration of an audio track
            (e.g. stereo pair) in a MediaResource.</rdfs:comment>
        <rdfs:domain rdf:resource="&ebucore;MediaResource"/>
    </owl:AnnotationProperty>
    


    <!-- http://www.ebu.ch/metadata/ontologies/ebucore/ebucore#bitRate -->

    <owl:AnnotationProperty rdf:about="&ebucore;bitRate">
        <rdfs:label rdf:datatype="&xsd;string">Bitrate</rdfs:label>
        <rdfs:comment xml:lang="en">To provide the bitrate at which the
            MediaResource can be played in bits/second. Current bitrate if constant, and average bitrate if variable.</rdfs:comment>
        <rdfs:domain rdf:resource="&ebucore;MediaResource"/>
    </owl:AnnotationProperty>
    


    <!-- http://www.ebu.ch/metadata/ontologies/ebucore/ebucore#bitRateMax -->

    <owl:AnnotationProperty rdf:about="&ebucore;bitRateMax">
        <rdfs:label xml:lang="en">Maximum bitrate</rdfs:label>
        <rdfs:comment xml:lang="en">The maximum bitrate when variable, in bits per second.</rdfs:comment>
        <rdfs:domain rdf:resource="&ebucore;MediaResource"/>
    </owl:AnnotationProperty>
    


    <!-- http://www.ebu.ch/metadata/ontologies/ebucore/ebucore#bitRateMode -->

    <owl:AnnotationProperty rdf:about="&ebucore;bitRateMode">
        <rdfs:label xml:lang="en">Bitrate mode</rdfs:label>
        <rdfs:comment xml:lang="en">A flag to indicate if the bit rate is fixed or
            variable.</rdfs:comment>
        <rdfs:domain rdf:resource="&ebucore;MediaResource"/>
    </owl:AnnotationProperty>
    


    <!-- http://www.ebu.ch/metadata/ontologies/ebucore/ebucore#bookmark -->

    <owl:AnnotationProperty rdf:about="&ebucore;bookmark">
        <rdfs:label xml:lang="en">Bookmark</rdfs:label>
        <rdfs:comment xml:lang="en">To provide a bookmark.</rdfs:comment>
        <rdfs:subPropertyOf rdf:resource="&ebucore;description"/>
    </owl:AnnotationProperty>
    


    <!-- http://www.ebu.ch/metadata/ontologies/ebucore/ebucore#businessObjectName -->

    <owl:AnnotationProperty rdf:about="&ebucore;businessObjectName">
        <rdfs:label xml:lang="en">Name</rdfs:label>
        <rdfs:comment xml:lang="en">A name attributed to a
            BusinessObject.</rdfs:comment>
        <rdfs:domain rdf:resource="&ebucore;BusinessObject"/>
    </owl:AnnotationProperty>
    


    <!-- http://www.ebu.ch/metadata/ontologies/ebucore/ebucore#captioningSource -->

    <owl:AnnotationProperty rdf:about="&ebucore;captioningSource">
        <rdfs:label xml:lang="en">Captioning source</rdfs:label>
        <rdfs:comment xml:lang="en">To provide information on the source of a
            captioning file.</rdfs:comment>
        <rdfs:domain rdf:resource="&ebucore;MediaResource"/>
    </owl:AnnotationProperty>
    


    <!-- http://www.ebu.ch/metadata/ontologies/ebucore/ebucore#codecFamily -->

    <owl:AnnotationProperty rdf:about="&ebucore;codecFamily">
        <rdfs:label xml:lang="en">Codec family</rdfs:label>
        <rdfs:comment xml:lang="en">To provide information on the product family of the Codec.</rdfs:comment>
        <rdfs:domain rdf:resource="&ebucore;Codec"/>
    </owl:AnnotationProperty>
    


    <!-- http://www.ebu.ch/metadata/ontologies/ebucore/ebucore#codecName -->

    <owl:AnnotationProperty rdf:about="&ebucore;codecName">
        <rdfs:label xml:lang="en">Codec name</rdfs:label>
        <rdfs:comment xml:lang="en">To provide a name for the Codec, e.g. a product name.</rdfs:comment>
        <rdfs:domain rdf:resource="&ebucore;Codec"/>
    </owl:AnnotationProperty>
    


    <!-- http://www.ebu.ch/metadata/ontologies/ebucore/ebucore#codecVendor -->

    <owl:AnnotationProperty rdf:about="&ebucore;codecVendor">
        <rdfs:label xml:lang="en">Codec vendor</rdfs:label>
        <rdfs:comment xml:lang="en">To provide a name for the vendor of the Codec.</rdfs:comment>
        <rdfs:domain rdf:resource="&ebucore;Codec"/>
    </owl:AnnotationProperty>
    


    <!-- http://www.ebu.ch/metadata/ontologies/ebucore/ebucore#codecVersion -->

    <owl:AnnotationProperty rdf:about="&ebucore;codecVersion">
        <rdfs:label xml:lang="en">Codec version</rdfs:label>
        <rdfs:comment xml:lang="en">To provide information on the version of the Codec.</rdfs:comment>
        <rdfs:domain rdf:resource="&ebucore;Codec"/>
    </owl:AnnotationProperty>
    


    <!-- http://www.ebu.ch/metadata/ontologies/ebucore/ebucore#comments -->

    <owl:AnnotationProperty rdf:about="&ebucore;comments">
        <rdfs:label xml:lang="en">Comments</rdfs:label>
        <rdfs:comment xml:lang="en">To provide a comment.</rdfs:comment>
        <rdfs:subPropertyOf rdf:resource="&ebucore;description"/>
    </owl:AnnotationProperty>
    


    <!-- http://www.ebu.ch/metadata/ontologies/ebucore/ebucore#contactEducation -->

    <owl:AnnotationProperty rdf:about="&ebucore;contactEducation">
        <rdfs:label xml:lang="en">Education</rdfs:label>
        <rdfs:comment xml:lang="en">The education details of a Contact /
            person.</rdfs:comment>
        <rdfs:domain rdf:resource="&ebucore;Contact"/>
    </owl:AnnotationProperty>
    


    <!-- http://www.ebu.ch/metadata/ontologies/ebucore/ebucore#contactFamilyInformation -->

    <owl:AnnotationProperty rdf:about="&ebucore;contactFamilyInformation">
        <rdfs:label xml:lang="en">Family information</rdfs:label>
        <rdfs:comment xml:lang="en">Information on the family of a Contact /
            person.</rdfs:comment>
        <rdfs:domain rdf:resource="&ebucore;Contact"/>
    </owl:AnnotationProperty>
    


    <!-- http://www.ebu.ch/metadata/ontologies/ebucore/ebucore#contactHobbies -->

    <owl:AnnotationProperty rdf:about="&ebucore;contactHobbies">
        <rdfs:label xml:lang="en">Hobbies</rdfs:label>
        <rdfs:comment xml:lang="en">The hobbies of a Contact /
            person.</rdfs:comment>
        <rdfs:domain rdf:resource="&ebucore;Contact"/>
    </owl:AnnotationProperty>
    


    <!-- http://www.ebu.ch/metadata/ontologies/ebucore/ebucore#contactMaritalStatus -->

    <owl:AnnotationProperty rdf:about="&ebucore;contactMaritalStatus">
        <rdfs:label xml:lang="en">Marital status</rdfs:label>
        <rdfs:comment xml:lang="en">The marital status of a Contact /
            person.</rdfs:comment>
        <rdfs:domain rdf:resource="&ebucore;Contact"/>
    </owl:AnnotationProperty>
    


    <!-- http://www.ebu.ch/metadata/ontologies/ebucore/ebucore#contactOccupation -->

    <owl:AnnotationProperty rdf:about="&ebucore;contactOccupation">
        <rdfs:label xml:lang="en">Occupation</rdfs:label>
        <rdfs:comment xml:lang="en">The job / occupation name of a Contact /
            person.</rdfs:comment>
        <rdfs:domain rdf:resource="&ebucore;Contact"/>
    </owl:AnnotationProperty>
    


    <!-- http://www.ebu.ch/metadata/ontologies/ebucore/ebucore#contactUsername -->

    <owl:AnnotationProperty rdf:about="&ebucore;contactUsername">
        <rdfs:label xml:lang="en">Username</rdfs:label>
        <rdfs:comment xml:lang="en">The username by which a Contact / person is
            known e.g. when attributing a rating value.</rdfs:comment>
        <rdfs:domain rdf:resource="&ebucore;Contact"/>
    </owl:AnnotationProperty>
    


    <!-- http://www.ebu.ch/metadata/ontologies/ebucore/ebucore#dateCreated -->

    <owl:AnnotationProperty rdf:about="&ebucore;dateCreated">
        <rdfs:label rdf:datatype="&xsd;string">Creation date/time</rdfs:label>
        <rdfs:comment xml:lang="en">The date of creation of the Resource.</rdfs:comment>
        <rdfs:domain rdf:resource="_:genid82"/>
        <rdfs:subPropertyOf rdf:resource="&dc;date"/>
    </owl:AnnotationProperty>
    


    <!-- http://www.ebu.ch/metadata/ontologies/ebucore/ebucore#dateDigitised -->

    <owl:AnnotationProperty rdf:about="&ebucore;dateDigitised">
        <rdfs:label rdf:datatype="&xsd;string">Digitisation date/time</rdfs:label>
        <rdfs:comment xml:lang="en">To provide the date of digitisation of the Resource.</rdfs:comment>
        <rdfs:domain rdf:resource="_:genid65"/>
        <rdfs:subPropertyOf rdf:resource="&dc;date"/>
    </owl:AnnotationProperty>
    


    <!-- http://www.ebu.ch/metadata/ontologies/ebucore/ebucore#dateIssued -->

    <owl:AnnotationProperty rdf:about="&ebucore;dateIssued">
        <rdfs:label rdf:datatype="&xsd;string">Publication date/time</rdfs:label>
        <rdfs:comment xml:lang="en">To provide the date of release of the Resource.</rdfs:comment>
        <rdfs:subPropertyOf rdf:resource="&dc;issued"/>
    </owl:AnnotationProperty>
    


    <!-- http://www.ebu.ch/metadata/ontologies/ebucore/ebucore#dateModified -->

    <owl:AnnotationProperty rdf:about="&ebucore;dateModified">
        <rdfs:label rdf:datatype="&xsd;string">Modification date/time</rdfs:label>
        <rdfs:comment xml:lang="en">To indicate the date at which the Resource has been modified.</rdfs:comment>
        <rdfs:domain rdf:resource="_:genid142"/>
        <rdfs:subPropertyOf rdf:resource="&dc;modified"/>
    </owl:AnnotationProperty>
    


    <!-- http://www.ebu.ch/metadata/ontologies/ebucore/ebucore#description -->

    <owl:AnnotationProperty rdf:about="&ebucore;description">
        <rdfs:label rdf:datatype="&xsd;string">Description</rdfs:label>
        <rdfs:comment rdf:datatype="&xsd;string">This can be specialised by using sub-properties
            like defined in http://www.ebu.ch/metadata/cs/web/ebu_DescriptionTypeCodeCS_p.xml.htm
            implemented as examples as e.g. &apos;summary&apos; or
            &apos;script&apos;.</rdfs:comment>
        <rdfs:subPropertyOf rdf:resource="&dc;description"/>
        <rdfs:domain rdf:resource="&ebucore;BusinessObject"/>
    </owl:AnnotationProperty>
    


    <!-- http://www.ebu.ch/metadata/ontologies/ebucore/ebucore#dopesheet -->

    <owl:AnnotationProperty rdf:about="&ebucore;dopesheet">
        <rdfs:label xml:lang="en">Dopesheet</rdfs:label>
        <rdfs:comment xml:lang="en">To provide a dopesheet with a title and brief description for news.</rdfs:comment>
        <rdfs:subPropertyOf rdf:resource="&ebucore;description"/>
    </owl:AnnotationProperty>
    


    <!-- http://www.ebu.ch/metadata/ontologies/ebucore/ebucore#duration -->

    <owl:AnnotationProperty rdf:about="&ebucore;duration">
        <rdfs:label xml:lang="en">Duration</rdfs:label>
        <rdfs:comment xml:lang="en">To provide information on the duration of a MediaResource. It corresponds to &apos;duration&apos; in the
            Ontology for Media Resources.</rdfs:comment>
        <rdfs:domain rdf:resource="_:genid194"/>
    </owl:AnnotationProperty>
    


    <!-- http://www.ebu.ch/metadata/ontologies/ebucore/ebucore#durationNormalPlayTime -->

    <owl:AnnotationProperty rdf:about="&ebucore;durationNormalPlayTime">
        <rdfs:label rdf:datatype="&xsd;string">Duration (time)</rdfs:label>
        <rdfs:comment xml:lang="en">To provide a duration as normal
            time.</rdfs:comment>
        <rdfs:subPropertyOf rdf:resource="&ebucore;duration"/>
    </owl:AnnotationProperty>
    


    <!-- http://www.ebu.ch/metadata/ontologies/ebucore/ebucore#durationNumberEditUnit -->

    <owl:AnnotationProperty rdf:about="&ebucore;durationNumberEditUnit">
        <rdfs:label rdf:datatype="&xsd;string">Duration (edit units)</rdfs:label>
        <rdfs:comment xml:lang="en">To provide a duration as a number of EditUnits
            which value is for instance the inverse of the audio sample rate or video frame
            rate.</rdfs:comment>
        <rdfs:subPropertyOf rdf:resource="&ebucore;duration"/>
    </owl:AnnotationProperty>
    


    <!-- http://www.ebu.ch/metadata/ontologies/ebucore/ebucore#durationPublished -->

    <owl:AnnotationProperty rdf:about="&ebucore;durationPublished">
        <rdfs:label xml:lang="en">Published Duration</rdfs:label>
        <rdfs:comment xml:lang="en">To provide information on the published / announced duration of an EditorialObject.</rdfs:comment>
        <rdfs:domain rdf:resource="&ebucore;EditorialObject"/>
    </owl:AnnotationProperty>
    


    <!-- http://www.ebu.ch/metadata/ontologies/ebucore/ebucore#durationPublishedNormalPlayTime -->

    <owl:AnnotationProperty rdf:about="&ebucore;durationPublishedNormalPlayTime">
        <rdfs:label xml:lang="en">Published duration (time)</rdfs:label>
        <rdfs:comment xml:lang="en">To provide a published duration as normal
            time.</rdfs:comment>
        <rdfs:subPropertyOf rdf:resource="&ebucore;durationPublished"/>
    </owl:AnnotationProperty>
    


    <!-- http://www.ebu.ch/metadata/ontologies/ebucore/ebucore#durationPublishedNumberEditUnit -->

    <owl:AnnotationProperty rdf:about="&ebucore;durationPublishedNumberEditUnit">
        <rdfs:label xml:lang="en">Published duration (edit units)</rdfs:label>
        <rdfs:comment xml:lang="en">To provide a published duration as a number of EditUnits
            which value is for instance the inverse of the audio sample rate or video frame
            rate.</rdfs:comment>
        <rdfs:subPropertyOf rdf:resource="&ebucore;durationPublished"/>
    </owl:AnnotationProperty>
    


    <!-- http://www.ebu.ch/metadata/ontologies/ebucore/ebucore#durationPublishedTimecode -->

    <owl:AnnotationProperty rdf:about="&ebucore;durationPublishedTimecode">
        <rdfs:label xml:lang="en">Published duration (timecode)</rdfs:label>
        <rdfs:comment xml:lang="en">The published duration expressed as a
            timecode.</rdfs:comment>
        <rdfs:subPropertyOf rdf:resource="&ebucore;durationPublished"/>
    </owl:AnnotationProperty>
    


    <!-- http://www.ebu.ch/metadata/ontologies/ebucore/ebucore#durationTimecode -->

    <owl:AnnotationProperty rdf:about="&ebucore;durationTimecode">
        <rdfs:label rdf:datatype="&xsd;string">Duration (timecode)</rdfs:label>
        <rdfs:comment xml:lang="en">The duration expressed as a
            timecode.</rdfs:comment>
        <rdfs:subPropertyOf rdf:resource="&ebucore;duration"/>
    </owl:AnnotationProperty>
    


    <!-- http://www.ebu.ch/metadata/ontologies/ebucore/ebucore#editUnit -->

    <owl:AnnotationProperty rdf:about="&ebucore;editUnit">
        <rdfs:label xml:lang="en">Edit unit</rdfs:label>
        <rdfs:comment xml:lang="en">The edit unit is e.g. the inverse of the audio
            sample rate or video frame rate.</rdfs:comment>
        <rdfs:domain rdf:resource="&ebucore;MediaResource"/>
    </owl:AnnotationProperty>
    


    <!-- http://www.ebu.ch/metadata/ontologies/ebucore/ebucore#encodingLevel -->

    <owl:AnnotationProperty rdf:about="&ebucore;encodingLevel">
        <rdfs:label xml:lang="en">Encoding level</rdfs:label>
        <rdfs:comment xml:lang="en">The encoding level.</rdfs:comment>
        <rdfs:domain rdf:resource="&ebucore;Resource"/>
    </owl:AnnotationProperty>
    


    <!-- http://www.ebu.ch/metadata/ontologies/ebucore/ebucore#encodingProfile -->

    <owl:AnnotationProperty rdf:about="&ebucore;encodingProfile">
        <rdfs:label xml:lang="en">Encoding profile</rdfs:label>
        <rdfs:comment xml:lang="en">The encoding profile</rdfs:comment>
        <rdfs:domain rdf:resource="&ebucore;Resource"/>
    </owl:AnnotationProperty>
    


    <!-- http://www.ebu.ch/metadata/ontologies/ebucore/ebucore#end -->

    <owl:AnnotationProperty rdf:about="&ebucore;end">
        <rdfs:label xml:lang="en">End time</rdfs:label>
        <rdfs:comment xml:lang="en">The start point of the media
            resource.</rdfs:comment>
        <rdfs:domain rdf:resource="&ebucore;MediaResource"/>
    </owl:AnnotationProperty>
    


    <!-- http://www.ebu.ch/metadata/ontologies/ebucore/ebucore#endNormalPlayTime -->

    <owl:AnnotationProperty rdf:about="&ebucore;endNormalPlayTime">
        <rdfs:label xml:lang="en">End time (time)</rdfs:label>
        <rdfs:comment xml:lang="en">The start time expressed using a time
            expression.</rdfs:comment>
        <rdfs:subPropertyOf rdf:resource="&ebucore;end"/>
    </owl:AnnotationProperty>
    


    <!-- http://www.ebu.ch/metadata/ontologies/ebucore/ebucore#endNumberEditUnits -->

    <owl:AnnotationProperty rdf:about="&ebucore;endNumberEditUnits">
        <rdfs:label xml:lang="en">End time (edit units)</rdfs:label>
        <rdfs:comment xml:lang="en">A start time expressed as a number of edit
            units.</rdfs:comment>
        <rdfs:subPropertyOf rdf:resource="&ebucore;end"/>
    </owl:AnnotationProperty>
    


    <!-- http://www.ebu.ch/metadata/ontologies/ebucore/ebucore#endTimecode -->

    <owl:AnnotationProperty rdf:about="&ebucore;endTimecode">
        <rdfs:label xml:lang="en">End time (timecode)</rdfs:label>
        <rdfs:comment xml:lang="en">A start time expressed as
            timecode.</rdfs:comment>
        <rdfs:subPropertyOf rdf:resource="&ebucore;end"/>
    </owl:AnnotationProperty>
    


    <!-- http://www.ebu.ch/metadata/ontologies/ebucore/ebucore#eventDescription -->

    <owl:AnnotationProperty rdf:about="&ebucore;eventDescription">
        <rdfs:label xml:lang="en">Description</rdfs:label>
        <rdfs:comment xml:lang="en">To provide a deescription for an
            Event.</rdfs:comment>
        <rdfs:domain rdf:resource="&ebucore;Event"/>
    </owl:AnnotationProperty>
    


    <!-- http://www.ebu.ch/metadata/ontologies/ebucore/ebucore#eventDuration -->

    <owl:AnnotationProperty rdf:about="&ebucore;eventDuration">
        <rdfs:label rdf:datatype="&xsd;string">Duration</rdfs:label>
        <rdfs:comment rdf:datatype="&xsd;string">The duration of an event.</rdfs:comment>
        <rdfs:domain rdf:resource="&ebucore;Event"/>
    </owl:AnnotationProperty>
    


    <!-- http://www.ebu.ch/metadata/ontologies/ebucore/ebucore#eventEndDate -->

    <owl:AnnotationProperty rdf:about="&ebucore;eventEndDate">
        <rdfs:label xml:lang="en">Event end date</rdfs:label>
        <rdfs:comment xml:lang="en">The end date of an Event.</rdfs:comment>
        <rdfs:domain rdf:resource="&ebucore;Event"/>
    </owl:AnnotationProperty>
    


    <!-- http://www.ebu.ch/metadata/ontologies/ebucore/ebucore#eventName -->

    <owl:AnnotationProperty rdf:about="&ebucore;eventName">
        <rdfs:label xml:lang="en">Event name</rdfs:label>
        <rdfs:comment xml:lang="en">To provide a name for an Event.</rdfs:comment>
        <rdfs:domain rdf:resource="&ebucore;Event"/>
    </owl:AnnotationProperty>
    


    <!-- http://www.ebu.ch/metadata/ontologies/ebucore/ebucore#eventStartDate -->

    <owl:AnnotationProperty rdf:about="&ebucore;eventStartDate">
        <rdfs:label xml:lang="en">Event start date</rdfs:label>
        <rdfs:comment xml:lang="en">The start date of an Event.</rdfs:comment>
        <rdfs:domain rdf:resource="&ebucore;Event"/>
    </owl:AnnotationProperty>
    


    <!-- http://www.ebu.ch/metadata/ontologies/ebucore/ebucore#familyName -->

    <owl:AnnotationProperty rdf:about="&ebucore;familyName">
        <rdfs:label xml:lang="en">Family name</rdfs:label>
        <rdfs:comment xml:lang="en">To provide a family name / last name.</rdfs:comment>
        <rdfs:subPropertyOf rdf:resource="&ebucore;agentName"/>
    </owl:AnnotationProperty>
    


    <!-- http://www.ebu.ch/metadata/ontologies/ebucore/ebucore#fictitious -->

    <owl:AnnotationProperty rdf:about="&ebucore;fictitious">
        <rdfs:label xml:lang="en">Fictitious agent indicator</rdfs:label>
        <rdfs:comment xml:lang="en">A flag to indicate if an agent of fictitious
            (set to true).</rdfs:comment>
        <rdfs:domain rdf:resource="&ebucore;Agent"/>
    </owl:AnnotationProperty>
    


    <!-- http://www.ebu.ch/metadata/ontologies/ebucore/ebucore#fileSize -->

    <owl:AnnotationProperty rdf:about="&ebucore;fileSize">
        <rdfs:label rdf:datatype="&xsd;string">File size</rdfs:label>
        <rdfs:comment xml:lang="en">to provide the size of a MediaResource in
            bytes.</rdfs:comment>
        <rdfs:domain rdf:resource="&ebucore;Resource"/>
    </owl:AnnotationProperty>
    


    <!-- http://www.ebu.ch/metadata/ontologies/ebucore/ebucore#filename -->

    <owl:AnnotationProperty rdf:about="&ebucore;filename">
        <rdfs:label xml:lang="en">File name</rdfs:label>
        <rdfs:comment xml:lang="en">The name of the file containing the
            Resource.</rdfs:comment>
        <rdfs:domain rdf:resource="&ebucore;Resource"/>
    </owl:AnnotationProperty>
    


    <!-- http://www.ebu.ch/metadata/ontologies/ebucore/ebucore#frameRate -->

    <owl:AnnotationProperty rdf:about="&ebucore;frameRate">
        <rdfs:label xml:lang="en">Frame rate</rdfs:label>
        <rdfs:comment xml:lang="en">The frame rate of the video signal in frame per
            second.</rdfs:comment>
        <rdfs:domain rdf:resource="&ebucore;VideoTrack"/>
    </owl:AnnotationProperty>
    


    <!-- http://www.ebu.ch/metadata/ontologies/ebucore/ebucore#frameSizeUnit -->

    <owl:AnnotationProperty rdf:about="&ebucore;frameSizeUnit">
        <rdfs:label xml:lang="en">Frame size unit</rdfs:label>
        <rdfs:comment xml:lang="en">The unit used to express the frame width or
            height. The unit by default is &apos;pixel&apos;.</rdfs:comment>
        <rdfs:domain rdf:resource="&ebucore;VideoTrack"/>
    </owl:AnnotationProperty>
    


    <!-- http://www.ebu.ch/metadata/ontologies/ebucore/ebucore#frequency -->

    <owl:AnnotationProperty rdf:about="&ebucore;frequency">
        <rdfs:label xml:lang="en">Frequency</rdfs:label>
        <rdfs:comment xml:lang="en">To provide the frequency of an AudioChannel filter</rdfs:comment>
        <rdfs:domain rdf:resource="&ebucore;AudioChannel"/>
    </owl:AnnotationProperty>
    


    <!-- http://www.ebu.ch/metadata/ontologies/ebucore/ebucore#givenName -->

    <owl:AnnotationProperty rdf:about="&ebucore;givenName">
        <rdfs:label xml:lang="en">Given name</rdfs:label>
        <rdfs:comment xml:lang="en">To provide one or more given names.</rdfs:comment>
        <rdfs:subPropertyOf rdf:resource="&ebucore;agentName"/>
    </owl:AnnotationProperty>
    


    <!-- http://www.ebu.ch/metadata/ontologies/ebucore/ebucore#groupDescription -->

    <owl:AnnotationProperty rdf:about="&ebucore;groupDescription">
        <rdfs:label xml:lang="en">Group description</rdfs:label>
        <rdfs:comment xml:lang="en">A textual description of a
            Group.</rdfs:comment>
        <rdfs:domain rdf:resource="&ebucore;Group"/>
    </owl:AnnotationProperty>
    


    <!-- http://www.ebu.ch/metadata/ontologies/ebucore/ebucore#groupName -->

    <owl:AnnotationProperty rdf:about="&ebucore;groupName">
        <rdfs:label xml:lang="en">Group name</rdfs:label>
        <rdfs:comment xml:lang="en">The name attributed to a Group.</rdfs:comment>
        <rdfs:domain rdf:resource="&ebucore;Group"/>
    </owl:AnnotationProperty>
    


    <!-- http://www.ebu.ch/metadata/ontologies/ebucore/ebucore#hasAffiliation -->

    <owl:AnnotationProperty rdf:about="&ebucore;hasAffiliation">
        <rdfs:label xml:lang="en">Affiliation</rdfs:label>
        <rdfs:comment xml:lang="en">A property to establish the relation between a
            Contact/person and an Organisation.</rdfs:comment>
        <rdfs:domain rdf:resource="&ebucore;Contact"/>
    </owl:AnnotationProperty>
    


    <!-- http://www.ebu.ch/metadata/ontologies/ebucore/ebucore#hasAncillaryData -->

    <owl:AnnotationProperty rdf:about="&ebucore;hasAncillaryData">
        <rdfs:label xml:lang="en">Ancillary data</rdfs:label>
        <rdfs:comment xml:lang="en">A property to signal the presence of
            AncillaryData associated with the EditorialObject and / or MediaResource.</rdfs:comment>
        <rdfs:domain rdf:resource="_:genid30"/>
    </owl:AnnotationProperty>
    


    <!-- http://www.ebu.ch/metadata/ontologies/ebucore/ebucore#hasAncillaryDataFormat -->

    <owl:AnnotationProperty rdf:about="&ebucore;hasAncillaryDataFormat">
        <rdfs:label rdf:datatype="&xsd;string">Ancillary data format</rdfs:label>
        <rdfs:subPropertyOf rdf:resource="&ebucore;hasDataFormat"/>
    </owl:AnnotationProperty>
    


    <!-- http://www.ebu.ch/metadata/ontologies/ebucore/ebucore#hasAnnotation -->

    <owl:AnnotationProperty rdf:about="&ebucore;hasAnnotation">
        <rdfs:label xml:lang="en">Annotation</rdfs:label>
        <rdfs:comment xml:lang="en">A property to signal the presence of Annotation
            information associated with an EditorialObject and / or a MediaResource.</rdfs:comment>
        <rdfs:domain rdf:resource="_:genid240"/>
    </owl:AnnotationProperty>
    


    <!-- http://www.ebu.ch/metadata/ontologies/ebucore/ebucore#hasAnnotationSource -->

    <owl:AnnotationProperty rdf:about="&ebucore;hasAnnotationSource">
        <rdfs:label xml:lang="en">Annotation Source</rdfs:label>
        <rdfs:comment xml:lang="en">To identify the Agent, Contact/person or
            Organisation who has provided the Annotation.</rdfs:comment>
        <rdfs:domain rdf:resource="&ebucore;Annotation"/>
    </owl:AnnotationProperty>
    


    <!-- http://www.ebu.ch/metadata/ontologies/ebucore/ebucore#hasAudioEncodingFormat -->

    <owl:AnnotationProperty rdf:about="&ebucore;hasAudioEncodingFormat">
        <rdfs:label rdf:datatype="&xsd;string">Audio encoding format</rdfs:label>
        <rdfs:subPropertyOf rdf:resource="&ebucore;hasEncodingFormat"/>
    </owl:AnnotationProperty>
    


    <!-- http://www.ebu.ch/metadata/ontologies/ebucore/ebucore#hasAudioFormat -->

    <owl:AnnotationProperty rdf:about="&ebucore;hasAudioFormat">
        <rdfs:label rdf:datatype="&xsd;string">Audio format</rdfs:label>
        <rdfs:subPropertyOf rdf:resource="&ebucore;hasFormat"/>
    </owl:AnnotationProperty>
    


    <!-- http://www.ebu.ch/metadata/ontologies/ebucore/ebucore#hasCaptioning -->

    <owl:AnnotationProperty rdf:about="&ebucore;hasCaptioning">
        <rdfs:label xml:lang="en">Captioning</rdfs:label>
        <rdfs:comment xml:lang="en">To signal the presence of
            Captioning.</rdfs:comment>
        <rdfs:domain rdf:resource="_:genid188"/>
    </owl:AnnotationProperty>
    


    <!-- http://www.ebu.ch/metadata/ontologies/ebucore/ebucore#hasCaptioningFormat -->

    <owl:AnnotationProperty rdf:about="&ebucore;hasCaptioningFormat">
        <rdfs:label rdf:datatype="&xsd;string">Captioning format</rdfs:label>
        <rdfs:subPropertyOf rdf:resource="&ebucore;hasDataFormat"/>
    </owl:AnnotationProperty>
    


    <!-- http://www.ebu.ch/metadata/ontologies/ebucore/ebucore#hasCastRole -->

    <owl:AnnotationProperty rdf:about="&ebucore;hasCastRole">
        <rdfs:label xml:lang="en">Cast role</rdfs:label>
        <rdfs:comment xml:lang="en">To define the roles involved in the creation of or related to the BusinessObject. The Role acts as a link to the Agent fulfilling that function.</rdfs:comment>
        <rdfs:domain rdf:resource="&ebucore;BusinessObject"/>
    </owl:AnnotationProperty>
    


    <!-- http://www.ebu.ch/metadata/ontologies/ebucore/ebucore#hasCodec -->

    <owl:AnnotationProperty rdf:about="&ebucore;hasCodec">
        <rdfs:label rdf:datatype="&xsd;string">Encoder</rdfs:label>
        <rdfs:comment xml:lang="en">To identify the Codec with which the Resource has been encoded.</rdfs:comment>
        <rdfs:domain rdf:resource="&ebucore;Resource"/>
    </owl:AnnotationProperty>
    


    <!-- http://www.ebu.ch/metadata/ontologies/ebucore/ebucore#hasColourSpace -->

    <owl:AnnotationProperty rdf:about="&ebucore;hasColourSpace">
        <rdfs:label rdf:datatype="&xsd;string">Colour space</rdfs:label>
        <rdfs:subPropertyOf rdf:resource="&ebucore;hasFormat"/>
    </owl:AnnotationProperty>
    


    <!-- http://www.ebu.ch/metadata/ontologies/ebucore/ebucore#hasContact -->

    <owl:AnnotationProperty rdf:about="&ebucore;hasContact">
        <rdfs:label xml:lang="en">Contact</rdfs:label>
        <rdfs:comment xml:lang="en">To provide information on a Contact for an
            Organisation or a physical person (e.g. the agent of an actor).</rdfs:comment>
        <rdfs:domain rdf:resource="&ebucore;Agent"/>
    </owl:AnnotationProperty>
    


    <!-- http://www.ebu.ch/metadata/ontologies/ebucore/ebucore#hasContainerFormat -->

    <owl:AnnotationProperty rdf:about="&ebucore;hasContainerFormat">
        <rdfs:label rdf:datatype="&xsd;string">Container format</rdfs:label>
        <rdfs:subPropertyOf rdf:resource="&ebucore;hasFormat"/>
    </owl:AnnotationProperty>
    


    <!-- http://www.ebu.ch/metadata/ontologies/ebucore/ebucore#hasContainerMimeType -->

    <owl:AnnotationProperty rdf:about="&ebucore;hasContainerMimeType">
        <rdfs:label rdf:datatype="&xsd;string">Mime type</rdfs:label>
        <rdfs:subPropertyOf rdf:resource="&ebucore;hasFormat"/>
    </owl:AnnotationProperty>
    


    <!-- http://www.ebu.ch/metadata/ontologies/ebucore/ebucore#hasContributor -->

    <owl:AnnotationProperty rdf:about="&ebucore;hasContributor">
        <rdfs:label xml:lang="en">Contributor</rdfs:label>
        <rdfs:comment xml:lang="en">To provide information on Contacts/persons or
            Organisations who have contributed to the BusinessObject or Resource.</rdfs:comment>
        <rdfs:subPropertyOf rdf:resource="&dc;contributor"/>
    </owl:AnnotationProperty>
    


    <!-- http://www.ebu.ch/metadata/ontologies/ebucore/ebucore#hasCoverage -->

    <owl:AnnotationProperty rdf:about="&ebucore;hasCoverage">
        <rdfs:label xml:lang="en">Coverage</rdfs:label>
        <rdfs:comment xml:lang="en">A property to identify the Events and or
            Locations, all real or fictional, covered by the 
            BusinessObject.</rdfs:comment>
        <rdfs:subPropertyOf rdf:resource="&dc;coverage"/>
    </owl:AnnotationProperty>
    


    <!-- http://www.ebu.ch/metadata/ontologies/ebucore/ebucore#hasCreationLocation -->

    <owl:AnnotationProperty rdf:about="&ebucore;hasCreationLocation">
        <rdfs:label xml:lang="en">Creation location</rdfs:label>
        <rdfs:comment xml:lang="en">The Location where content has been created.</rdfs:comment>
        <rdfs:subPropertyOf rdf:resource="&dc;coverage"/>
    </owl:AnnotationProperty>
    


    <!-- http://www.ebu.ch/metadata/ontologies/ebucore/ebucore#hasCreator -->

    <owl:AnnotationProperty rdf:about="&ebucore;hasCreator">
        <rdfs:label xml:lang="en">Creator</rdfs:label>
        <rdfs:comment xml:lang="en">To identify an Agent involved in the creation of the Resource or BusinessObject.</rdfs:comment>
        <rdfs:subPropertyOf rdf:resource="&dc;creator"/>
    </owl:AnnotationProperty>
    


    <!-- http://www.ebu.ch/metadata/ontologies/ebucore/ebucore#hasDataFormat -->

    <owl:AnnotationProperty rdf:about="&ebucore;hasDataFormat">
        <rdfs:label rdf:datatype="&xsd;string">Data format</rdfs:label>
        <rdfs:subPropertyOf rdf:resource="&ebucore;hasFormat"/>
    </owl:AnnotationProperty>
    


    <!-- http://www.ebu.ch/metadata/ontologies/ebucore/ebucore#hasDepartment -->

    <owl:AnnotationProperty rdf:about="&ebucore;hasDepartment">
        <rdfs:label xml:lang="en">Department</rdfs:label>
        <rdfs:comment xml:lang="en">To identify Departments within an
            Organisation.</rdfs:comment>
        <rdfs:domain rdf:resource="&ebucore;Organisation"/>
    </owl:AnnotationProperty>
    


    <!-- http://www.ebu.ch/metadata/ontologies/ebucore/ebucore#hasDocumentFormat -->

    <owl:AnnotationProperty rdf:about="&ebucore;hasDocumentFormat">
        <rdfs:label rdf:datatype="&xsd;string">has document format</rdfs:label>
        <rdfs:subPropertyOf rdf:resource="&ebucore;hasFormat"/>
    </owl:AnnotationProperty>
    


    <!-- http://www.ebu.ch/metadata/ontologies/ebucore/ebucore#hasDopesheet -->

    <owl:AnnotationProperty rdf:about="&ebucore;hasDopesheet">
        <rdfs:label xml:lang="en">Dopesheet</rdfs:label>
        <rdfs:comment xml:lang="en">To associate a Dopesheet with a NewsItem.</rdfs:comment>
        <rdfs:domain rdf:resource="&ebucore;NewsItem"/>
    </owl:AnnotationProperty>
    


    <!-- http://www.ebu.ch/metadata/ontologies/ebucore/ebucore#hasEncodingFormat -->

    <owl:AnnotationProperty rdf:about="&ebucore;hasEncodingFormat">
        <rdfs:label rdf:datatype="&xsd;string">Encoding format</rdfs:label>
        <rdfs:subPropertyOf rdf:resource="&ebucore;hasFormat"/>
    </owl:AnnotationProperty>
    


    <!-- http://www.ebu.ch/metadata/ontologies/ebucore/ebucore#hasEvent -->

    <owl:AnnotationProperty rdf:about="&ebucore;hasEvent">
        <rdfs:label xml:lang="en">Event</rdfs:label>
        <rdfs:comment xml:lang="en">To associate an Event with a
            Location.</rdfs:comment>
        <rdfs:subPropertyOf rdf:resource="&dc;coverage"/>
        <rdfs:domain rdf:resource="&ebucore;Location"/>
    </owl:AnnotationProperty>
    


    <!-- http://www.ebu.ch/metadata/ontologies/ebucore/ebucore#hasFileFormat -->

    <owl:AnnotationProperty rdf:about="&ebucore;hasFileFormat">
        <rdfs:label rdf:datatype="&xsd;string">File format</rdfs:label>
        <rdfs:subPropertyOf rdf:resource="&ebucore;hasFormat"/>
    </owl:AnnotationProperty>
    


    <!-- http://www.ebu.ch/metadata/ontologies/ebucore/ebucore#hasFormat -->

    <owl:AnnotationProperty rdf:about="&ebucore;hasFormat">
        <rdfs:label xml:lang="en">Format</rdfs:label>
        <rdfs:comment xml:lang="en">A property to define the Format of a Resource.</rdfs:comment>
        <rdfs:subPropertyOf rdf:resource="&dc;format"/>
    </owl:AnnotationProperty>
    


    <!-- http://www.ebu.ch/metadata/ontologies/ebucore/ebucore#hasGenre -->

    <owl:AnnotationProperty rdf:about="&ebucore;hasGenre">
        <rdfs:label xml:lang="en">Genre</rdfs:label>
        <rdfs:comment xml:lang="en">To define a Genre/category associated to the
            BusinesssObject.</rdfs:comment>
        <rdfs:domain rdf:resource="&ebucore;BusinessObject"/>
        <rdfs:subPropertyOf rdf:resource="&ebucore;hasType"/>
    </owl:AnnotationProperty>
    


    <!-- http://www.ebu.ch/metadata/ontologies/ebucore/ebucore#hasImageFormat -->

    <owl:AnnotationProperty rdf:about="&ebucore;hasImageFormat">
        <rdfs:label rdf:datatype="&xsd;string">Image format</rdfs:label>
        <rdfs:subPropertyOf rdf:resource="&ebucore;hasFormat"/>
    </owl:AnnotationProperty>
    


    <!-- http://www.ebu.ch/metadata/ontologies/ebucore/ebucore#hasKeyCareerEvent -->

    <owl:AnnotationProperty rdf:about="&ebucore;hasKeyCareerEvent">
        <rdfs:label rdf:datatype="&xsd;string">Career event</rdfs:label>
        <rdfs:domain rdf:resource="&ebucore;Agent"/>
        <rdfs:subPropertyOf rdf:resource="&ebucore;hasRelatedEvent"/>
    </owl:AnnotationProperty>
    


    <!-- http://www.ebu.ch/metadata/ontologies/ebucore/ebucore#hasKeyPersonalEvent -->

    <owl:AnnotationProperty rdf:about="&ebucore;hasKeyPersonalEvent">
        <rdfs:label rdf:datatype="&xsd;string">Personal event</rdfs:label>
        <rdfs:domain rdf:resource="&ebucore;Agent"/>
        <rdfs:subPropertyOf rdf:resource="&ebucore;hasRelatedEvent"/>
    </owl:AnnotationProperty>
    


    <!-- http://www.ebu.ch/metadata/ontologies/ebucore/ebucore#hasKeyword -->

    <owl:AnnotationProperty rdf:about="&ebucore;hasKeyword">
        <rdfs:label xml:lang="en">Keyword</rdfs:label>
        <rdfs:comment xml:lang="en">To associate a concept, descriptive phrase or
            Keyword that specifies the topic of the BusinessObject or Annotation.</rdfs:comment>
        <rdfs:domain rdf:resource="_:genid56"/>
    </owl:AnnotationProperty>
    


    <!-- http://www.ebu.ch/metadata/ontologies/ebucore/ebucore#hasLanguage -->

    <owl:AnnotationProperty rdf:about="&ebucore;hasLanguage">
        <rdfs:label xml:lang="en">Language</rdfs:label>
        <rdfs:comment xml:lang="en">To associate a Language to a Resource or
            BusinessObject. A controlled vocabulary based on BCP 47 is recommended. This
            property can also be used to identify the presence of sign language (RFC 5646). By
            inheritance, the hasLanguage property applies indifferently at the MediaResource /
            Fragment / Track levels at which the usage is being defined. Best practice recommends to
            use to best possible level of granularity fo describe the usage of language within a
            MediaResource including at Fragment and Track levels.</rdfs:comment>
        <rdfs:subPropertyOf rdf:resource="&dc;language"/>
    </owl:AnnotationProperty>
    


    <!-- http://www.ebu.ch/metadata/ontologies/ebucore/ebucore#hasLocation -->

    <owl:AnnotationProperty rdf:about="&ebucore;hasLocation">
        <rdfs:label xml:lang="en">Location</rdfs:label>
        <rdfs:comment xml:lang="en">To associate a Location with a BusinessObject.</rdfs:comment>
        <rdfs:subPropertyOf rdf:resource="&dc;coverage"/>
        <rdfs:domain rdf:resource="&ebucore;Event"/>
    </owl:AnnotationProperty>
    


    <!-- http://www.ebu.ch/metadata/ontologies/ebucore/ebucore#hasLogo -->

    <owl:AnnotationProperty rdf:about="&ebucore;hasLogo">
        <rdfs:label xml:lang="en">Logo</rdfs:label>
        <rdfs:comment xml:lang="en">Logos can be used in a variety of contexts.
            Logo can be associated with an Organisation or a Service or a PublicationChannel.</rdfs:comment>
        <rdfs:domain rdf:resource="_:genid37"/>
    </owl:AnnotationProperty>
    


    <!-- http://www.ebu.ch/metadata/ontologies/ebucore/ebucore#hasMedium -->

    <owl:AnnotationProperty rdf:about="&ebucore;hasMedium">
        <rdfs:label rdf:datatype="&xsd;string">Medium</rdfs:label>
        <rdfs:subPropertyOf rdf:resource="&ebucore;hasFormat"/>
    </owl:AnnotationProperty>
    


    <!-- http://www.ebu.ch/metadata/ontologies/ebucore/ebucore#hasMetadataAttributor -->

    <owl:AnnotationProperty rdf:about="&ebucore;hasMetadataAttributor">
        <rdfs:label xml:lang="en">Metadata attributor</rdfs:label>
        <rdfs:comment xml:lang="en">To identify the Agent (Contact/person or
            Organisation) who has created the metadata.</rdfs:comment>
        <rdfs:domain rdf:resource="&ebucore;Subject"/>
    </owl:AnnotationProperty>
    


    <!-- http://www.ebu.ch/metadata/ontologies/ebucore/ebucore#hasMimeType -->

    <owl:AnnotationProperty rdf:about="&ebucore;hasMimeType">
        <rdfs:label rdf:datatype="&xsd;string">Mime type</rdfs:label>
        <rdfs:subPropertyOf rdf:resource="&ebucore;hasFormat"/>
    </owl:AnnotationProperty>
    


    <!-- http://www.ebu.ch/metadata/ontologies/ebucore/ebucore#hasObjectType -->

    <owl:AnnotationProperty rdf:about="&ebucore;hasObjectType">
        <rdfs:label rdf:datatype="&xsd;string">Object/asset type</rdfs:label>
        <rdfs:comment xml:lang="en">To define an ObjectType for the BusinessObject
             (e.g. book, report, programme, clip) if not defined as a subClass of BusinessObject.</rdfs:comment>
        <rdfs:domain rdf:resource="&ebucore;BusinessObject"/>
        <rdfs:subPropertyOf rdf:resource="&ebucore;hasType"/>
    </owl:AnnotationProperty>
    


    <!-- http://www.ebu.ch/metadata/ontologies/ebucore/ebucore#hasOriginalLanguage -->

    <owl:AnnotationProperty rdf:about="&ebucore;hasOriginalLanguage">
        <rdfs:label rdf:datatype="&xsd;string">Original language</rdfs:label>
        <rdfs:subPropertyOf rdf:resource="&ebucore;hasLanguage"/>
    </owl:AnnotationProperty>
    


    <!-- http://www.ebu.ch/metadata/ontologies/ebucore/ebucore#hasPictogram -->

    <owl:AnnotationProperty rdf:about="&ebucore;hasPictogram">
        <rdfs:label xml:lang="en">Pictogram</rdfs:label>
        <rdfs:comment xml:lang="en">To provide a visual representation of  TargetAudience or Rating.</rdfs:comment>
        <rdfs:domain rdf:resource="_:genid197"/>
    </owl:AnnotationProperty>
    


    <!-- http://www.ebu.ch/metadata/ontologies/ebucore/ebucore#hasPublicationChannel -->

    <owl:AnnotationProperty rdf:about="&ebucore;hasPublicationChannel">
        <rdfs:label xml:lang="en">Publication channel</rdfs:label>
        <rdfs:comment xml:lang="en">To associate a PublicationEvent with a
            PublicationChannel.</rdfs:comment>
        <rdfs:domain rdf:resource="&ebucore;PublicationEvent"/>
    </owl:AnnotationProperty>
    


    <!-- http://www.ebu.ch/metadata/ontologies/ebucore/ebucore#hasPublicationEvent -->

    <owl:AnnotationProperty rdf:about="&ebucore;hasPublicationEvent">
        <rdfs:label xml:lang="en">Publication event</rdfs:label>
        <rdfs:comment xml:lang="en">To associate PublicationEvents with
            PublicationChannels or as elements of a PublicationHistory or PublicationPlanning.</rdfs:comment>
        <rdfs:domain rdf:resource="_:genid233"/>
    </owl:AnnotationProperty>
    


    <!-- http://www.ebu.ch/metadata/ontologies/ebucore/ebucore#hasPublicationHistory -->

    <owl:AnnotationProperty rdf:about="&ebucore;hasPublicationHistory">
        <rdfs:label rdf:datatype="&xsd;string">has publication history</rdfs:label>
        <rdfs:domain rdf:resource="_:genid18"/>
    </owl:AnnotationProperty>
    


    <!-- http://www.ebu.ch/metadata/ontologies/ebucore/ebucore#hasPublisher -->

    <owl:AnnotationProperty rdf:about="&ebucore;hasPublisher">
        <rdfs:label xml:lang="en">Publisher</rdfs:label>
        <rdfs:comment xml:lang="en">To identify an Agent involved in the publication of the Resource or BusinessObject.</rdfs:comment>
        <rdfs:subPropertyOf rdf:resource="&dc;publisher"/>
    </owl:AnnotationProperty>
    


    <!-- http://www.ebu.ch/metadata/ontologies/ebucore/ebucore#hasRating -->

    <owl:AnnotationProperty rdf:about="&ebucore;hasRating">
        <rdfs:label xml:lang="en">Rating</rdfs:label>
        <rdfs:comment xml:lang="en">To identify the presence of Rating attributed
            to a Resource or BusinessObject.</rdfs:comment>
        <rdfs:domain rdf:resource="_:genid224"/>
    </owl:AnnotationProperty>
    


    <!-- http://www.ebu.ch/metadata/ontologies/ebucore/ebucore#hasRatingSource -->

    <owl:AnnotationProperty rdf:about="&ebucore;hasRatingSource">
        <rdfs:label xml:lang="en">Rating provider</rdfs:label>
        <rdfs:comment xml:lang="en">To identify an Agent (Contact/person or
            Organisation) who has proposed a Rating.</rdfs:comment>
        <rdfs:domain rdf:resource="&ebucore;Rating"/>
    </owl:AnnotationProperty>
    


    <!-- http://www.ebu.ch/metadata/ontologies/ebucore/ebucore#hasRelatedAudioStream -->

    <owl:AnnotationProperty rdf:about="&ebucore;hasRelatedAudioStream">
        <rdfs:label xml:lang="en">Audio stream</rdfs:label>
        <rdfs:comment xml:lang="en">To associate an AudioStream with an AudioTrack.</rdfs:comment>
        <rdfs:domain rdf:resource="&ebucore;AudioTrack"/>
        <rdfs:subPropertyOf rdf:resource="&ebucore;hasRelatedResource"/>
    </owl:AnnotationProperty>
    


    <!-- http://www.ebu.ch/metadata/ontologies/ebucore/ebucore#hasRelatedAudioTrack -->

    <owl:AnnotationProperty rdf:about="&ebucore;hasRelatedAudioTrack">
        <rdfs:label xml:lang="en">Audio track</rdfs:label>
        <rdfs:comment xml:lang="en">To associate an AudioTrack with an AudioStream or an AudioTrackUID.</rdfs:comment>
        <rdfs:subPropertyOf rdf:resource="&ebucore;hasRelatedResource"/>
    </owl:AnnotationProperty>
    


    <!-- http://www.ebu.ch/metadata/ontologies/ebucore/ebucore#hasRelatedEvent -->

    <owl:AnnotationProperty rdf:about="&ebucore;hasRelatedEvent">
        <rdfs:label rdf:datatype="&xsd;string">has related event</rdfs:label>
        <rdfs:domain rdf:resource="_:genid93"/>
        <rdfs:subPropertyOf rdf:resource="&dc;relation"/>
    </owl:AnnotationProperty>
    


    <!-- http://www.ebu.ch/metadata/ontologies/ebucore/ebucore#hasRelatedPicture -->

    <owl:AnnotationProperty rdf:about="&ebucore;hasRelatedPicture">
        <rdfs:label xml:lang="en">Picture</rdfs:label>
        <rdfs:comment xml:lang="en">To associate a Picture with a BusinessObject or a Resource.</rdfs:comment>
        <rdfs:domain rdf:resource="_:genid71"/>
        <rdfs:subPropertyOf rdf:resource="&ebucore;hasRelatedResource"/>
    </owl:AnnotationProperty>
    


    <!-- http://www.ebu.ch/metadata/ontologies/ebucore/ebucore#hasRelatedResource -->

    <rdf:Description rdf:about="&ebucore;hasRelatedResource">
        <rdfs:label rdf:datatype="&xsd;string">Related resource</rdfs:label>
        <rdfs:comment xml:lang="en">To identify a Resource associated with an Asset or a BusinessObject or a PublicationEvent or another Resource.</rdfs:comment>
    </rdf:Description>
    


    <!-- http://www.ebu.ch/metadata/ontologies/ebucore/ebucore#hasRights -->

    <owl:AnnotationProperty rdf:about="&ebucore;hasRights"/>
    


    <!-- http://www.ebu.ch/metadata/ontologies/ebucore/ebucore#hasRightsContact -->

    <owl:AnnotationProperty rdf:about="&ebucore;hasRightsContact">
        <rdfs:label xml:lang="en">Contact</rdfs:label>
        <rdfs:comment xml:lang="en">To identify a Contact/person who can provide
            assistance / guidance regarding the associated Rights.</rdfs:comment>
        <rdfs:domain rdf:resource="&ebucore;Rights"/>
    </owl:AnnotationProperty>
    


    <!-- http://www.ebu.ch/metadata/ontologies/ebucore/ebucore#hasRightsHolder -->

    <owl:AnnotationProperty rdf:about="&ebucore;hasRightsHolder">
        <rdfs:label xml:lang="en">Rights holder</rdfs:label>
        <rdfs:comment xml:lang="en">To identify an Agent (Contact/person or
            Organisation) having/managing Rights.</rdfs:comment>
        <rdfs:domain rdf:resource="&ebucore;Rights"/>
    </owl:AnnotationProperty>
    


    <!-- http://www.ebu.ch/metadata/ontologies/ebucore/ebucore#hasRole -->

    <owl:AnnotationProperty rdf:about="&ebucore;hasRole">
        <rdfs:label xml:lang="en">Role</rdfs:label>
        <rdfs:comment xml:lang="en">To define the role of an Agent (Contact/person
            or Organisation). The association in a particular context is made by declaring the hasCastRole  associated with the BusinessObject.</rdfs:comment>
        <rdfs:domain rdf:resource="&ebucore;Agent"/>
    </owl:AnnotationProperty>
    


    <!-- http://www.ebu.ch/metadata/ontologies/ebucore/ebucore#hasSigning -->

    <owl:AnnotationProperty rdf:about="&ebucore;hasSigning">
        <rdfs:label xml:lang="en">Accessibility - signing</rdfs:label>
        <rdfs:comment xml:lang="en">To identify the presence of Signing associated
            to the BusinessObject/Resource.</rdfs:comment>
        <rdfs:domain rdf:resource="_:genid215"/>
    </owl:AnnotationProperty>
    


    <!-- http://www.ebu.ch/metadata/ontologies/ebucore/ebucore#hasSigningFormat -->

    <owl:AnnotationProperty rdf:about="&ebucore;hasSigningFormat">
        <rdfs:label rdf:datatype="&xsd;string">Signing format</rdfs:label>
        <rdfs:subPropertyOf rdf:resource="&ebucore;hasVideoFormat"/>
    </owl:AnnotationProperty>
    


    <!-- http://www.ebu.ch/metadata/ontologies/ebucore/ebucore#hasSource -->

    <owl:AnnotationProperty rdf:about="&ebucore;hasSource">
        <rdfs:label xml:lang="en">Source</rdfs:label>
        <rdfs:comment xml:lang="en">To identify a Resource as the source of another Resource.</rdfs:comment>
        <rdfs:subPropertyOf rdf:resource="&dc;source"/>
    </owl:AnnotationProperty>
    


    <!-- http://www.ebu.ch/metadata/ontologies/ebucore/ebucore#hasStaff -->

    <owl:AnnotationProperty rdf:about="&ebucore;hasStaff">
        <rdfs:label xml:lang="en">Staff</rdfs:label>
        <rdfs:comment xml:lang="en">To identify staff working within an Organisation.</rdfs:comment>
        <rdfs:domain rdf:resource="&ebucore;Organisation"/>
    </owl:AnnotationProperty>
    


    <!-- http://www.ebu.ch/metadata/ontologies/ebucore/ebucore#hasStorageType -->

    <owl:AnnotationProperty rdf:about="&ebucore;hasStorageType">
        <rdfs:label rdf:datatype="&xsd;string">Storage type</rdfs:label>
        <rdfs:comment xml:lang="en">To define a particular type of storage /
            repository associated with the Locator from where a Resource can be
            accessed.</rdfs:comment>
        <rdfs:domain rdf:resource="&ebucore;Resource"/>
    </owl:AnnotationProperty>
    


    <!-- http://www.ebu.ch/metadata/ontologies/ebucore/ebucore#hasSubject -->

    <owl:AnnotationProperty rdf:about="&ebucore;hasSubject">
        <rdfs:label xml:lang="en">Subject</rdfs:label>
        <rdfs:comment xml:lang="en">To associate a Subject addressed with a
            BusinessObject / Resource.</rdfs:comment>
        <rdfs:subPropertyOf rdf:resource="&dc;subject"/>
    </owl:AnnotationProperty>
    


    <!-- http://www.ebu.ch/metadata/ontologies/ebucore/ebucore#hasSubtitling -->

    <owl:AnnotationProperty rdf:about="&ebucore;hasSubtitling">
        <rdfs:label xml:lang="en">Subtitling</rdfs:label>
        <rdfs:comment xml:lang="en">To signal the presence of Subtitling associated
            with the EditorialObject or MediaResource.</rdfs:comment>
        <rdfs:domain rdf:resource="_:genid15"/>
    </owl:AnnotationProperty>
    


    <!-- http://www.ebu.ch/metadata/ontologies/ebucore/ebucore#hasSubtitlingFormat -->

    <owl:AnnotationProperty rdf:about="&ebucore;hasSubtitlingFormat">
        <rdfs:label rdf:datatype="&xsd;string">Subtitling format</rdfs:label>
        <rdfs:subPropertyOf rdf:resource="&ebucore;hasDataFormat"/>
    </owl:AnnotationProperty>
    


    <!-- http://www.ebu.ch/metadata/ontologies/ebucore/ebucore#hasTargetAudience -->

    <owl:AnnotationProperty rdf:about="&ebucore;hasTargetAudience">
        <rdfs:label rdf:datatype="&xsd;string">Target audience</rdfs:label>
        <rdfs:comment xml:lang="en">To associate a TargetAudience (e.g. for
            parental guiddance or targeting a particular social group) with a
            BusinessObject/Resource.</rdfs:comment>
        <rdfs:domain rdf:resource="&ebucore;BusinessObject"/>
        <rdfs:subPropertyOf rdf:resource="&ebucore;hasType"/>
    </owl:AnnotationProperty>
    


    <!-- http://www.ebu.ch/metadata/ontologies/ebucore/ebucore#hasTheme -->

    <owl:AnnotationProperty rdf:about="&ebucore;hasTheme">
        <rdfs:label rdf:datatype="&xsd;string">Theme</rdfs:label>
        <rdfs:subPropertyOf rdf:resource="&ebucore;hasKeyword"/>
    </owl:AnnotationProperty>
    


    <!-- http://www.ebu.ch/metadata/ontologies/ebucore/ebucore#hasTopic -->

    <owl:AnnotationProperty rdf:about="&ebucore;hasTopic">
        <rdfs:label rdf:datatype="&xsd;string">Topic</rdfs:label>
        <rdfs:subPropertyOf rdf:resource="&ebucore;hasSubject"/>
    </owl:AnnotationProperty>
    


    <!-- http://www.ebu.ch/metadata/ontologies/ebucore/ebucore#hasTrack -->

    <owl:AnnotationProperty rdf:about="&ebucore;hasTrack">
        <rdfs:label xml:lang="en">Track</rdfs:label>
        <rdfs:comment xml:lang="en">To associate audio/data/video tracks with a MediaResource.</rdfs:comment>
        <rdfs:domain rdf:resource="&ebucore;MediaResource"/>
        <rdfs:subPropertyOf rdf:resource="&ebucore;hasRelatedResource"/>
    </owl:AnnotationProperty>
    


    <!-- http://www.ebu.ch/metadata/ontologies/ebucore/ebucore#hasType -->

    <owl:AnnotationProperty rdf:about="&ebucore;hasType">
        <rdfs:label xml:lang="en">Type</rdfs:label>
        <rdfs:comment xml:lang="en">To define a type of BusinessObject is not declared as a subClass of BusinessObject.</rdfs:comment>
        <rdfs:subPropertyOf rdf:resource="&dc;type"/>
        <rdfs:domain rdf:resource="&ebucore;BusinessObject"/>
    </owl:AnnotationProperty>
    


    <!-- http://www.ebu.ch/metadata/ontologies/ebucore/ebucore#hasVideoEncodingFormat -->

    <owl:AnnotationProperty rdf:about="&ebucore;hasVideoEncodingFormat">
        <rdfs:label rdf:datatype="&xsd;string">Video encoding format</rdfs:label>
        <rdfs:subPropertyOf rdf:resource="&ebucore;hasEncodingFormat"/>
    </owl:AnnotationProperty>
    


    <!-- http://www.ebu.ch/metadata/ontologies/ebucore/ebucore#hasVideoFormat -->

    <owl:AnnotationProperty rdf:about="&ebucore;hasVideoFormat">
        <rdfs:label rdf:datatype="&xsd;string">Video format</rdfs:label>
        <rdfs:subPropertyOf rdf:resource="&ebucore;hasFormat"/>
    </owl:AnnotationProperty>
    


    <!-- http://www.ebu.ch/metadata/ontologies/ebucore/ebucore#hash -->

    <owl:AnnotationProperty rdf:about="&ebucore;hash">
        <rdfs:label xml:lang="en">Hash code</rdfs:label>
        <rdfs:comment xml:lang="en">The hash value associated to a Resource. There
            are different methods / algorithms to calculate hash values, which can be defined as
            subproperties.</rdfs:comment>
        <rdfs:domain rdf:resource="&ebucore;Resource"/>
    </owl:AnnotationProperty>
    


    <!-- http://www.ebu.ch/metadata/ontologies/ebucore/ebucore#height -->

    <owl:AnnotationProperty rdf:about="&ebucore;height">
        <rdfs:label xml:lang="en">Height</rdfs:label>
        <rdfs:comment xml:lang="en">The height of e.g. a video frame typically
            expressed as a number of lines or the height of a picture/image expressed in millimeters
            or else.</rdfs:comment>
        <rdfs:domain rdf:resource="&ebucore;Resource"/>
    </owl:AnnotationProperty>
    


    <!-- http://www.ebu.ch/metadata/ontologies/ebucore/ebucore#heightUnit -->

    <owl:AnnotationProperty rdf:about="&ebucore;heightUnit">
        <rdfs:label xml:lang="en">Height unit</rdfs:label>
        <rdfs:comment xml:lang="en">The unit used to measure a Height e.g. in
            pixels or number of lines or millimeters or else.</rdfs:comment>
        <rdfs:domain rdf:resource="&ebucore;Resource"/>
    </owl:AnnotationProperty>
    


    <!-- http://www.ebu.ch/metadata/ontologies/ebucore/ebucore#highPass -->

    <owl:AnnotationProperty rdf:about="&ebucore;highPass">
        <rdfs:label xml:lang="en">High pass frequency</rdfs:label>
        <rdfs:comment xml:lang="en">The high pass frequency of the AudioChannel filter.</rdfs:comment>
        <rdfs:subPropertyOf rdf:resource="&ebucore;frequency"/>
    </owl:AnnotationProperty>
    


    <!-- http://www.ebu.ch/metadata/ontologies/ebucore/ebucore#highlights -->

    <owl:AnnotationProperty rdf:about="&ebucore;highlights">
        <rdfs:label xml:lang="en">Highlights</rdfs:label>
        <rdfs:comment xml:lang="en">To provide highlights.</rdfs:comment>
        <rdfs:subPropertyOf rdf:resource="&ebucore;description"/>
    </owl:AnnotationProperty>
    


    <!-- http://www.ebu.ch/metadata/ontologies/ebucore/ebucore#holdsRightsOver -->

    <owl:AnnotationProperty rdf:about="&ebucore;holdsRightsOver">
        <rdfs:label xml:lang="en">Asset, resource, object</rdfs:label>
        <rdfs:comment xml:lang="en">To identify a BusinessObject or Resource on
            which an Agent (Contact/person or Organisation) holds Rights.</rdfs:comment>
        <rdfs:domain rdf:resource="&ebucore;Agent"/>
    </owl:AnnotationProperty>
    


    <!-- http://www.ebu.ch/metadata/ontologies/ebucore/ebucore#identifier -->

    <owl:AnnotationProperty rdf:about="&ebucore;identifier">
        <rdfs:label xml:lang="en">Identifier</rdfs:label>
        <rdfs:comment xml:lang="en">Corresponds to &apos;identifier&apos;
            in the W3C Ontology for Media Annotation. The URI may be used to express an alternative
            identifier of the resource, or to share an identifier used by other instances of the
            same resource (equivalent to the fucntionality owl:sameAs).</rdfs:comment>
        <rdfs:comment xml:lang="en">This property is intended to provide an
            alternative identifier for the resource, which has no URI counterpart. In the case where
            the alternative identifier can be expressed as a URI, it is recommended to use
            owl:sameAs instead.</rdfs:comment>
        <rdfs:subPropertyOf rdf:resource="&dc;identifier"/>
    </owl:AnnotationProperty>
    


    <!-- http://www.ebu.ch/metadata/ontologies/ebucore/ebucore#isAgent -->

    <owl:AnnotationProperty rdf:about="&ebucore;isAgent">
        <rdfs:label xml:lang="en">Agent</rdfs:label>
        <rdfs:comment xml:lang="en">To identify a Contact/person or Organisation as part of a cast list.</rdfs:comment>
        <rdfs:domain rdf:resource="&ebucore;Cast"/>
    </owl:AnnotationProperty>
    


    <!-- http://www.ebu.ch/metadata/ontologies/ebucore/ebucore#isCharacter -->

    <owl:AnnotationProperty rdf:about="&ebucore;isCharacter">
        <rdfs:label xml:lang="en">Character</rdfs:label>
        <rdfs:comment xml:lang="en">To identify the character personified by a Cast individual.</rdfs:comment>
        <rdfs:domain rdf:resource="&ebucore;Cast"/>
    </owl:AnnotationProperty>
    


    <!-- http://www.ebu.ch/metadata/ontologies/ebucore/ebucore#isCopyrightedBy -->

    <owl:AnnotationProperty rdf:about="&ebucore;isCopyrightedBy">
        <rdfs:label xml:lang="en">Copyright</rdfs:label>
        <rdfs:comment xml:lang="en">Copyright statement.</rdfs:comment>
        <rdfs:subPropertyOf rdf:resource="&ebucore;hasRights"/>
    </owl:AnnotationProperty>
    


    <!-- http://www.ebu.ch/metadata/ontologies/ebucore/ebucore#isCoveredBy -->

    <owl:AnnotationProperty rdf:about="&ebucore;isCoveredBy">
        <rdfs:label xml:lang="en">Rights</rdfs:label>
        <rdfs:comment xml:lang="en">The Rights or policy applicable to the
            BusinessObject, Asset, Resource or PublicationEvent.</rdfs:comment>
        <rdfs:subPropertyOf rdf:resource="&ebucore;hasRights"/>
    </owl:AnnotationProperty>
    


    <!-- http://www.ebu.ch/metadata/ontologies/ebucore/ebucore#isFictitiousContact -->

    <owl:AnnotationProperty rdf:about="&ebucore;isFictitiousContact">
        <rdfs:label xml:lang="en">Fictitious contact</rdfs:label>
        <rdfs:comment xml:lang="en">To identify Contact/persons being fictitious.</rdfs:comment>
        <rdfs:domain rdf:resource="&ebucore;Character"/>
    </owl:AnnotationProperty>
    


    <!-- http://www.ebu.ch/metadata/ontologies/ebucore/ebucore#isNextInSequence -->

    <owl:AnnotationProperty rdf:about="&ebucore;isNextInSequence">
        <rdfs:label rdf:datatype="&xsd;string">Next</rdfs:label>
        <rdfs:comment rdf:datatype="&xsd;string">A link to a an BusinessObject or a Resource following the current BusinessObject or Resource in an ordered sequence</rdfs:comment>
        <rdfs:domain rdf:resource="_:genid27"/>
        <rdfs:subPropertyOf rdf:resource="&dc;relation"/>
    </owl:AnnotationProperty>
    


    <!-- http://www.ebu.ch/metadata/ontologies/ebucore/ebucore#isReferencedBy -->

    <owl:AnnotationProperty rdf:about="&ebucore;isReferencedBy">
        <rdfs:label xml:lang="en">Related object, resource</rdfs:label>
        <rdfs:comment xml:lang="en">To express references across Assets, BusinessObjects or Resources.</rdfs:comment>
        <rdfs:domain rdf:resource="_:genid78"/>
        <rdfs:subPropertyOf rdf:resource="&dc;relation"/>
    </owl:AnnotationProperty>
    


    <!-- http://www.ebu.ch/metadata/ontologies/ebucore/ebucore#keywordDefinition -->

    <owl:AnnotationProperty rdf:about="&ebucore;keywordDefinition">
        <rdfs:label xml:lang="en">Keyword definition</rdfs:label>
        <rdfs:comment xml:lang="en">To provide a definition for a Keyword.</rdfs:comment>
        <rdfs:domain rdf:resource="&ebucore;Keyword"/>
    </owl:AnnotationProperty>
    


    <!-- http://www.ebu.ch/metadata/ontologies/ebucore/ebucore#lineNumber -->

    <owl:AnnotationProperty rdf:about="&ebucore;lineNumber">
        <rdfs:label xml:lang="en">Line number</rdfs:label>
        <rdfs:comment xml:lang="en">To provide the number of the line on which
            ancillary data is being carried and the equivalent in the digital domain.</rdfs:comment>
        <rdfs:domain rdf:resource="&ebucore;AncillaryData"/>
    </owl:AnnotationProperty>
    


    <!-- http://www.ebu.ch/metadata/ontologies/ebucore/ebucore#locationAddress -->

    <owl:AnnotationProperty rdf:about="&ebucore;locationAddress">
        <rdfs:label xml:lang="en">Address</rdfs:label>
        <rdfs:comment xml:lang="en">To provide the address of a
           Location.</rdfs:comment>
        <rdfs:domain rdf:resource="&ebucore;Location"/>
    </owl:AnnotationProperty>
    


    <!-- http://www.ebu.ch/metadata/ontologies/ebucore/ebucore#locationAddressArea -->

    <owl:AnnotationProperty rdf:about="&ebucore;locationAddressArea">
        <rdfs:label xml:lang="en">Area</rdfs:label>
        <rdfs:comment xml:lang="en">To provide the Area part of an
            Adrress.</rdfs:comment>
        <rdfs:subPropertyOf rdf:resource="&ebucore;locationAddress"/>
    </owl:AnnotationProperty>
    


    <!-- http://www.ebu.ch/metadata/ontologies/ebucore/ebucore#locationAddressCountry -->

    <owl:AnnotationProperty rdf:about="&ebucore;locationAddressCountry">
        <rdfs:label xml:lang="en">Country</rdfs:label>
        <rdfs:comment xml:lang="en">To provide the country name and or country
            code.</rdfs:comment>
        <rdfs:subPropertyOf rdf:resource="&ebucore;locationAddress"/>
    </owl:AnnotationProperty>
    


    <!-- http://www.ebu.ch/metadata/ontologies/ebucore/ebucore#locationAddressLine -->

    <owl:AnnotationProperty rdf:about="&ebucore;locationAddressLine">
        <rdfs:label xml:lang="en">Address line</rdfs:label>
        <rdfs:comment xml:lang="en">To write address line with e.g. the street name
            and number.</rdfs:comment>
        <rdfs:subPropertyOf rdf:resource="&ebucore;locationAddress"/>
    </owl:AnnotationProperty>
    


    <!-- http://www.ebu.ch/metadata/ontologies/ebucore/ebucore#locationAddressLocality -->

    <owl:AnnotationProperty rdf:about="&ebucore;locationAddressLocality">
        <rdfs:label xml:lang="en">Locality</rdfs:label>
        <rdfs:comment xml:lang="en">To provide the name of a city, viallge,
            etc.</rdfs:comment>
        <rdfs:subPropertyOf rdf:resource="&ebucore;locationAddress"/>
    </owl:AnnotationProperty>
    


    <!-- http://www.ebu.ch/metadata/ontologies/ebucore/ebucore#locationAddressPostalCode -->

    <owl:AnnotationProperty rdf:about="&ebucore;locationAddressPostalCode">
        <rdfs:label xml:lang="en">Postal code</rdfs:label>
        <rdfs:comment xml:lang="en">To provide an address postal
            code.</rdfs:comment>
        <rdfs:subPropertyOf rdf:resource="&ebucore;locationAddress"/>
    </owl:AnnotationProperty>
    


    <!-- http://www.ebu.ch/metadata/ontologies/ebucore/ebucore#locationAltitude -->

    <owl:AnnotationProperty rdf:about="&ebucore;locationAltitude">
        <rdfs:label xml:lang="en">Altitude</rdfs:label>
        <rdfs:comment xml:lang="en">To define the altitude of a Location in
            meters.</rdfs:comment>
        <rdfs:domain rdf:resource="&ebucore;Location"/>
    </owl:AnnotationProperty>
    


    <!-- http://www.ebu.ch/metadata/ontologies/ebucore/ebucore#locationCoordinateSystemName -->

    <owl:AnnotationProperty rdf:about="&ebucore;locationCoordinateSystemName">
        <rdfs:label xml:lang="en">Coordinate system</rdfs:label>
        <rdfs:comment xml:lang="en">To specify the name of the gps coordinate
            system used for the Location.</rdfs:comment>
        <rdfs:domain rdf:resource="&ebucore;Location"/>
    </owl:AnnotationProperty>
    


    <!-- http://www.ebu.ch/metadata/ontologies/ebucore/ebucore#locationDescription -->

    <owl:AnnotationProperty rdf:about="&ebucore;locationDescription">
        <rdfs:label xml:lang="en">Location description</rdfs:label>
        <rdfs:comment xml:lang="en">To provide a description of a particular Location.</rdfs:comment>
        <rdfs:domain rdf:resource="&ebucore;Location"/>
    </owl:AnnotationProperty>
    


    <!-- http://www.ebu.ch/metadata/ontologies/ebucore/ebucore#locationLatitude -->

    <owl:AnnotationProperty rdf:about="&ebucore;locationLatitude">
        <rdfs:label xml:lang="en">Latitude</rdfs:label>
        <rdfs:comment xml:lang="en">The latitude of the Location.</rdfs:comment>
        <rdfs:domain rdf:resource="&ebucore;Location"/>
    </owl:AnnotationProperty>
    


    <!-- http://www.ebu.ch/metadata/ontologies/ebucore/ebucore#locationLongitude -->

    <owl:AnnotationProperty rdf:about="&ebucore;locationLongitude">
        <rdfs:label xml:lang="en">Longitude</rdfs:label>
        <rdfs:comment xml:lang="en">To define the longitude of the
            Location.</rdfs:comment>
        <rdfs:domain rdf:resource="&ebucore;Location"/>
    </owl:AnnotationProperty>
    


    <!-- http://www.ebu.ch/metadata/ontologies/ebucore/ebucore#locationName -->

    <owl:AnnotationProperty rdf:about="&ebucore;locationName">
        <rdfs:label xml:lang="en">Location name</rdfs:label>
        <rdfs:comment xml:lang="en">The name by which a Location is
            known.</rdfs:comment>
        <rdfs:domain rdf:resource="&ebucore;Location"/>
    </owl:AnnotationProperty>
    


    <!-- http://www.ebu.ch/metadata/ontologies/ebucore/ebucore#locationRegion -->

    <owl:AnnotationProperty rdf:about="&ebucore;locationRegion">
        <rdfs:label xml:lang="en">Region</rdfs:label>
        <rdfs:comment xml:lang="en">To provide a description of a particular region assocoated to the Location.</rdfs:comment>
        <rdfs:domain rdf:resource="&ebucore;Location"/>
    </owl:AnnotationProperty>
    


    <!-- http://www.ebu.ch/metadata/ontologies/ebucore/ebucore#locator -->

    <owl:AnnotationProperty rdf:about="&ebucore;locator">
        <rdfs:label rdf:datatype="&xsd;string">Locator</rdfs:label>
        <rdfs:comment xml:lang="en">A locator from where the Resource can be accessed.</rdfs:comment>
        <rdfs:domain rdf:resource="&ebucore;Resource"/>
    </owl:AnnotationProperty>
    


    <!-- http://www.ebu.ch/metadata/ontologies/ebucore/ebucore#locatorTargetInformation -->

    <owl:AnnotationProperty rdf:about="&ebucore;locatorTargetInformation">
        <rdfs:label xml:lang="en">Target information</rdfs:label>
        <rdfs:comment xml:lang="en">Information about storage accessed by the locator.</rdfs:comment>
        <rdfs:domain rdf:resource="&ebucore;Resource"/>
    </owl:AnnotationProperty>
    


    <!-- http://www.ebu.ch/metadata/ontologies/ebucore/ebucore#loudnessIntegratedLoudness -->

    <owl:AnnotationProperty rdf:about="&ebucore;loudnessIntegratedLoudness">
        <rdfs:label xml:lang="en">Integrated loudness</rdfs:label>
        <rdfs:comment xml:lang="en">The value for integrated loudness measured at AudioProgramme or AudioContent level.</rdfs:comment>
        <rdfs:domain rdf:resource="_:genid227"/>
        <rdfs:subPropertyOf rdf:resource="&ebucore;loudnessParameters"/>
    </owl:AnnotationProperty>
    


    <!-- http://www.ebu.ch/metadata/ontologies/ebucore/ebucore#loudnessMaxMomentary -->

    <owl:AnnotationProperty rdf:about="&ebucore;loudnessMaxMomentary">
        <rdfs:label xml:lang="en">Max momentary loudness</rdfs:label>
        <rdfs:comment xml:lang="en">The value for maximum momentary loudness measured at AudioProgramme or AudioContent level.</rdfs:comment>
        <rdfs:domain rdf:resource="_:genid12"/>
        <rdfs:subPropertyOf rdf:resource="&ebucore;loudnessParameters"/>
    </owl:AnnotationProperty>
    


    <!-- http://www.ebu.ch/metadata/ontologies/ebucore/ebucore#loudnessMaxTruepeak -->

    <owl:AnnotationProperty rdf:about="&ebucore;loudnessMaxTruepeak">
        <rdfs:label xml:lang="en">Max true peak loudness</rdfs:label>
        <rdfs:comment xml:lang="en">The value for maximum true peak loudness measured at AudioProgramme or AudioContent level.</rdfs:comment>
        <rdfs:domain rdf:resource="_:genid206"/>
        <rdfs:subPropertyOf rdf:resource="&ebucore;loudnessParameters"/>
    </owl:AnnotationProperty>
    


    <!-- http://www.ebu.ch/metadata/ontologies/ebucore/ebucore#loudnessMethod -->

    <owl:AnnotationProperty rdf:about="&ebucore;loudnessMethod">
        <rdfs:label xml:lang="en">Loudness method</rdfs:label>
        <rdfs:comment xml:lang="en">The method for loudness measurement at AudioProgramme or AudioContent level.</rdfs:comment>
        <rdfs:domain rdf:resource="_:genid218"/>
        <rdfs:subPropertyOf rdf:resource="&ebucore;loudnessParameters"/>
    </owl:AnnotationProperty>
    


    <!-- http://www.ebu.ch/metadata/ontologies/ebucore/ebucore#loudnessParameters -->

    <owl:AnnotationProperty rdf:about="&ebucore;loudnessParameters">
        <rdfs:label xml:lang="en">loudness parameters</rdfs:label>
        <rdfs:comment xml:lang="en">All the parameters for measurement of loudness at the AudioContent or AudioProgramme level.</rdfs:comment>
        <rdfs:domain rdf:resource="_:genid21"/>
    </owl:AnnotationProperty>
    


    <!-- http://www.ebu.ch/metadata/ontologies/ebucore/ebucore#loudnessRange -->

    <owl:AnnotationProperty rdf:about="&ebucore;loudnessRange">
        <rdfs:label xml:lang="en">Loudness range</rdfs:label>
        <rdfs:comment xml:lang="en">The loudness range measured at AudioProgramme or AudioContent level.</rdfs:comment>
        <rdfs:domain rdf:resource="_:genid53"/>
        <rdfs:subPropertyOf rdf:resource="&ebucore;loudnessParameters"/>
    </owl:AnnotationProperty>
    


    <!-- http://www.ebu.ch/metadata/ontologies/ebucore/ebucore#lounessMaxShortTerm -->

    <owl:AnnotationProperty rdf:about="&ebucore;lounessMaxShortTerm">
        <rdfs:label xml:lang="en">Max short term loudness</rdfs:label>
        <rdfs:comment xml:lang="en">The maximum short term loudness measured at AudioProgramme or AudioContent level.</rdfs:comment>
        <rdfs:domain rdf:resource="_:genid237"/>
        <rdfs:subPropertyOf rdf:resource="&ebucore;loudnessParameters"/>
    </owl:AnnotationProperty>
    


    <!-- http://www.ebu.ch/metadata/ontologies/ebucore/ebucore#lowPass -->

    <owl:AnnotationProperty rdf:about="&ebucore;lowPass">
        <rdfs:label xml:lang="en">Low pass frequency</rdfs:label>
        <rdfs:comment xml:lang="en">The low pass frequency of the AudioChannel filter.</rdfs:comment>
        <rdfs:subPropertyOf rdf:resource="&ebucore;frequency"/>
    </owl:AnnotationProperty>
    


    <!-- http://www.ebu.ch/metadata/ontologies/ebucore/ebucore#mainTitle -->

    <owl:AnnotationProperty rdf:about="&ebucore;mainTitle">
        <rdfs:label xml:lang="en">Main title</rdfs:label>
        <rdfs:comment xml:lang="en">To provide the main title by which the media
            resource is known.</rdfs:comment>
        <rdfs:subPropertyOf rdf:resource="&ebucore;title"/>
    </owl:AnnotationProperty>
    


    <!-- http://www.ebu.ch/metadata/ontologies/ebucore/ebucore#mxfChannelID -->

    <owl:AnnotationProperty rdf:about="&ebucore;mxfChannelID">
        <rdfs:label xml:lang="en">MXF channel ID</rdfs:label>
        <rdfs:comment xml:lang="en">To identify an MXF channel.</rdfs:comment>
        <rdfs:subPropertyOf rdf:resource="&ebucore;audioMXFLookup"/>
    </owl:AnnotationProperty>
    


    <!-- http://www.ebu.ch/metadata/ontologies/ebucore/ebucore#mxfPackageUID -->

    <owl:AnnotationProperty rdf:about="&ebucore;mxfPackageUID">
        <rdfs:label xml:lang="en">MXF package UID</rdfs:label>
        <rdfs:comment xml:lang="en">To identify a MXF package.</rdfs:comment>
        <rdfs:subPropertyOf rdf:resource="&ebucore;audioMXFLookup"/>
    </owl:AnnotationProperty>
    


    <!-- http://www.ebu.ch/metadata/ontologies/ebucore/ebucore#mxfTrackID -->

    <owl:AnnotationProperty rdf:about="&ebucore;mxfTrackID">
        <rdfs:label xml:lang="en">MXF track ID</rdfs:label>
        <rdfs:comment xml:lang="en">To identify a MXF track.</rdfs:comment>
        <rdfs:subPropertyOf rdf:resource="&ebucore;audioMXFLookup"/>
    </owl:AnnotationProperty>
    


    <!-- http://www.ebu.ch/metadata/ontologies/ebucore/ebucore#nameTitle -->

    <owl:AnnotationProperty rdf:about="&ebucore;nameTitle">
        <rdfs:label xml:lang="en">Salutation title</rdfs:label>
        <rdfs:comment xml:lang="en">To provide a salutation title e.g M. Ms, Dr, Pr.</rdfs:comment>
        <rdfs:subPropertyOf rdf:resource="&ebucore;agentName"/>
    </owl:AnnotationProperty>
    


    <!-- http://www.ebu.ch/metadata/ontologies/ebucore/ebucore#noiseFilter -->

    <owl:AnnotationProperty rdf:about="&ebucore;noiseFilter">
        <rdfs:label xml:lang="en">Noise filter</rdfs:label>
        <rdfs:comment xml:lang="en">A flag to signal that a noise filter has been
            used.</rdfs:comment>
        <rdfs:domain rdf:resource="&ebucore;VideoFormat"/>
    </owl:AnnotationProperty>
    


    <!-- http://www.ebu.ch/metadata/ontologies/ebucore/ebucore#notRated -->

    <owl:AnnotationProperty rdf:about="&ebucore;notRated">
        <rdfs:label xml:lang="en">Not rated</rdfs:label>
        <rdfs:comment xml:lang="en">A flag to indicate that the BusinessObejct has not been rated.</rdfs:comment>
        <rdfs:domain rdf:resource="_:genid47"/>
    </owl:AnnotationProperty>
    


    <!-- http://www.ebu.ch/metadata/ontologies/ebucore/ebucore#numberOfTracks -->

    <owl:AnnotationProperty rdf:about="&ebucore;numberOfTracks">
        <rdfs:label xml:lang="en">Number of tracks</rdfs:label>
        <rdfs:comment xml:lang="en">The number of Tracks composing the MediaResource.</rdfs:comment>
        <rdfs:domain rdf:resource="&ebucore;MediaResource"/>
    </owl:AnnotationProperty>
    


    <!-- http://www.ebu.ch/metadata/ontologies/ebucore/ebucore#objectTypeDefinition -->

    <owl:AnnotationProperty rdf:about="&ebucore;objectTypeDefinition">
        <rdfs:label xml:lang="en">Audio object type definition</rdfs:label>
        <rdfs:comment xml:lang="en">To provide a definition of an AudioObject type.</rdfs:comment>
        <rdfs:domain rdf:resource="&ebucore;ObjectType"/>
    </owl:AnnotationProperty>
    


    <!-- http://www.ebu.ch/metadata/ontologies/ebucore/ebucore#officeAddressArea -->

    <owl:AnnotationProperty rdf:about="&ebucore;officeAddressArea">
        <rdfs:label xml:lang="en">Area code</rdfs:label>
        <rdfs:comment xml:lang="en">To provide the Area part of an
            Address.</rdfs:comment>
        <rdfs:subPropertyOf rdf:resource="&ebucore;officeMailAddress"/>
    </owl:AnnotationProperty>
    


    <!-- http://www.ebu.ch/metadata/ontologies/ebucore/ebucore#officeAddressCountry -->

    <owl:AnnotationProperty rdf:about="&ebucore;officeAddressCountry">
        <rdfs:label xml:lang="en">Country</rdfs:label>
        <rdfs:comment xml:lang="en">To provide the country name and or country
            code.</rdfs:comment>
        <rdfs:subPropertyOf rdf:resource="&ebucore;officeMailAddress"/>
    </owl:AnnotationProperty>
    


    <!-- http://www.ebu.ch/metadata/ontologies/ebucore/ebucore#officeAddressLine -->

    <owl:AnnotationProperty rdf:about="&ebucore;officeAddressLine">
        <rdfs:label xml:lang="en">Address line</rdfs:label>
        <rdfs:comment xml:lang="en">To write address line with e.g. the street name
            and number.</rdfs:comment>
        <rdfs:subPropertyOf rdf:resource="&ebucore;officeMailAddress"/>
    </owl:AnnotationProperty>
    


    <!-- http://www.ebu.ch/metadata/ontologies/ebucore/ebucore#officeAddressLocality -->

    <owl:AnnotationProperty rdf:about="&ebucore;officeAddressLocality">
        <rdfs:label xml:lang="en">Locality</rdfs:label>
        <rdfs:comment xml:lang="en">To provide the name of a city, village,
            etc.</rdfs:comment>
        <rdfs:subPropertyOf rdf:resource="&ebucore;officeMailAddress"/>
    </owl:AnnotationProperty>
    


    <!-- http://www.ebu.ch/metadata/ontologies/ebucore/ebucore#officeAddressPostalCode -->

    <owl:AnnotationProperty rdf:about="&ebucore;officeAddressPostalCode">
        <rdfs:label xml:lang="en">Postal code</rdfs:label>
        <rdfs:comment xml:lang="en">To provide an address postal
            code.</rdfs:comment>
        <rdfs:subPropertyOf rdf:resource="&ebucore;officeMailAddress"/>
    </owl:AnnotationProperty>
    


    <!-- http://www.ebu.ch/metadata/ontologies/ebucore/ebucore#officeEmailAddress -->

    <owl:AnnotationProperty rdf:about="&ebucore;officeEmailAddress">
        <rdfs:label xml:lang="en">Office email</rdfs:label>
        <rdfs:comment xml:lang="en">To provide the professional/office email
            address of an agent (Contact/person or organisation).</rdfs:comment>
        <rdfs:subPropertyOf rdf:resource="&ebucore;agentEmailAddress"/>
    </owl:AnnotationProperty>
    


    <!-- http://www.ebu.ch/metadata/ontologies/ebucore/ebucore#officeHomepage -->

    <owl:AnnotationProperty rdf:about="&ebucore;officeHomepage">
        <rdfs:label xml:lang="en">Homepage (office)</rdfs:label>
        <rdfs:comment xml:lang="en">To provide an office/professional/company web
            homepage of an Agent (Contact/person or Organisation).</rdfs:comment>
        <rdfs:domain rdf:resource="&ebucore;Agent"/>
        <rdfs:subPropertyOf rdf:resource="&ebucore;agentWebHomepage"/>
    </owl:AnnotationProperty>
    


    <!-- http://www.ebu.ch/metadata/ontologies/ebucore/ebucore#officeMailAddress -->

    <owl:AnnotationProperty rdf:about="&ebucore;officeMailAddress">
        <rdfs:label xml:lang="en">Office mail address</rdfs:label>
        <rdfs:comment xml:lang="en">To provide the professional / office address of
            an agent (Contact/person or organisation).</rdfs:comment>
        <rdfs:subPropertyOf rdf:resource="&ebucore;agentAddress"/>
    </owl:AnnotationProperty>
    


    <!-- http://www.ebu.ch/metadata/ontologies/ebucore/ebucore#officeMobileTelephoneNumber -->

    <owl:AnnotationProperty rdf:about="&ebucore;officeMobileTelephoneNumber">
        <rdfs:label xml:lang="en">Mobile (office)</rdfs:label>
        <rdfs:comment xml:lang="en">To provide the professional/office/company
            mobile telephone number of an agent (Contact/person or organisation).</rdfs:comment>
        <rdfs:subPropertyOf rdf:resource="&ebucore;agentMobileTelephoneNumber"/>
    </owl:AnnotationProperty>
    


    <!-- http://www.ebu.ch/metadata/ontologies/ebucore/ebucore#officeTelephoneNumber -->

    <owl:AnnotationProperty rdf:about="&ebucore;officeTelephoneNumber">
        <rdfs:label xml:lang="en">Telephone (office)</rdfs:label>
        <rdfs:comment xml:lang="en">To provide an office/professional/company
            telephone number of an Agent (Contact/person or Organisation).</rdfs:comment>
        <rdfs:subPropertyOf rdf:resource="&ebucore;agentTelephoneNumber"/>
    </owl:AnnotationProperty>
    


    <!-- http://www.ebu.ch/metadata/ontologies/ebucore/ebucore#organisationName -->

    <owl:AnnotationProperty rdf:about="&ebucore;organisationName">
        <rdfs:label xml:lang="en">Name</rdfs:label>
        <rdfs:comment xml:lang="en">To provide the full name of an Organisation.</rdfs:comment>
        <rdfs:domain rdf:resource="&ebucore;Agent"/>
    </owl:AnnotationProperty>
    


    <!-- http://www.ebu.ch/metadata/ontologies/ebucore/ebucore#orientation -->

    <owl:AnnotationProperty rdf:about="&ebucore;orientation">
        <rdfs:label xml:lang="en">Orientation</rdfs:label>
        <rdfs:comment xml:lang="en">The orientation of a Document or an Image i.e. landscape or
            portrait.</rdfs:comment>
        <rdfs:domain rdf:resource="_:genid209"/>
    </owl:AnnotationProperty>
    


    <!-- http://www.ebu.ch/metadata/ontologies/ebucore/ebucore#originalTitle -->

    <owl:AnnotationProperty rdf:about="&ebucore;originalTitle">
        <rdfs:label xml:lang="en">Original title</rdfs:label>
        <rdfs:comment xml:lang="en">To provide the original title attributed to the
            media resource e.g. in its original language.</rdfs:comment>
        <rdfs:subPropertyOf rdf:resource="&ebucore;title"/>
    </owl:AnnotationProperty>
    


    <!-- http://www.ebu.ch/metadata/ontologies/ebucore/ebucore#packageByteSize -->

    <owl:AnnotationProperty rdf:about="&ebucore;packageByteSize">
        <rdfs:label xml:lang="en">Package size (in bytes)</rdfs:label>
        <rdfs:comment xml:lang="en">The size of a media package in
            Bytes.</rdfs:comment>
        <rdfs:domain rdf:resource="&ebucore;Resource"/>
    </owl:AnnotationProperty>
    


    <!-- http://www.ebu.ch/metadata/ontologies/ebucore/ebucore#packageName -->

    <owl:AnnotationProperty rdf:about="&ebucore;packageName">
        <rdfs:label xml:lang="en">Package name</rdfs:label>
        <rdfs:comment xml:lang="en">The name attributed to a
            package.</rdfs:comment>
        <rdfs:domain rdf:resource="&ebucore;Resource"/>
    </owl:AnnotationProperty>
    


    <!-- http://www.ebu.ch/metadata/ontologies/ebucore/ebucore#partDefinition -->

    <owl:AnnotationProperty rdf:about="&ebucore;partDefinition">
        <rdfs:label xml:lang="en">Part definition</rdfs:label>
        <rdfs:comment xml:lang="en">A definition associated with the Part.</rdfs:comment>
        <rdfs:domain rdf:resource="&ebucore;Part"/>
    </owl:AnnotationProperty>
    


    <!-- http://www.ebu.ch/metadata/ontologies/ebucore/ebucore#partName -->

    <owl:AnnotationProperty rdf:about="&ebucore;partName">
        <rdfs:label xml:lang="en">Part name</rdfs:label>
        <rdfs:comment xml:lang="en">A name by which the Part is identified.</rdfs:comment>
        <rdfs:domain rdf:resource="&ebucore;Part"/>
    </owl:AnnotationProperty>
    


    <!-- http://www.ebu.ch/metadata/ontologies/ebucore/ebucore#partNumber -->

    <owl:AnnotationProperty rdf:about="&ebucore;partNumber">
        <rdfs:label xml:lang="en">Part number</rdfs:label>
        <rdfs:comment xml:lang="en">The number associated to a Part as one among
            many.</rdfs:comment>
        <rdfs:domain rdf:resource="&ebucore;Part"/>
    </owl:AnnotationProperty>
    


    <!-- http://www.ebu.ch/metadata/ontologies/ebucore/ebucore#partTotalNumber -->

    <owl:AnnotationProperty rdf:about="&ebucore;partTotalNumber">
        <rdfs:label xml:lang="en">Total number of parts</rdfs:label>
        <rdfs:comment xml:lang="en">The total number of Parts associated with a
            BusinessObject.</rdfs:comment>
        <rdfs:domain rdf:resource="&ebucore;Part"/>
    </owl:AnnotationProperty>
    


    <!-- http://www.ebu.ch/metadata/ontologies/ebucore/ebucore#playlist -->

    <owl:AnnotationProperty rdf:about="&ebucore;playlist">
        <rdfs:label xml:lang="en">Playlist</rdfs:label>
        <rdfs:comment xml:lang="en">To describe a playlist.</rdfs:comment>
        <rdfs:subPropertyOf rdf:resource="&ebucore;description"/>
    </owl:AnnotationProperty>
    


    <!-- http://www.ebu.ch/metadata/ontologies/ebucore/ebucore#privateAddressArea -->

    <owl:AnnotationProperty rdf:about="&ebucore;privateAddressArea">
        <rdfs:label xml:lang="en">Area code</rdfs:label>
        <rdfs:comment xml:lang="en">To provide the Area part of an
            Adrress.</rdfs:comment>
        <rdfs:subPropertyOf rdf:resource="&ebucore;privateMailAddress"/>
    </owl:AnnotationProperty>
    


    <!-- http://www.ebu.ch/metadata/ontologies/ebucore/ebucore#privateAddressCountry -->

    <owl:AnnotationProperty rdf:about="&ebucore;privateAddressCountry">
        <rdfs:label xml:lang="en">Country</rdfs:label>
        <rdfs:comment xml:lang="en">To provide the country name and or country
            code.</rdfs:comment>
        <rdfs:subPropertyOf rdf:resource="&ebucore;privateMailAddress"/>
    </owl:AnnotationProperty>
    


    <!-- http://www.ebu.ch/metadata/ontologies/ebucore/ebucore#privateAddressLine -->

    <owl:AnnotationProperty rdf:about="&ebucore;privateAddressLine">
        <rdfs:label xml:lang="en">Address line</rdfs:label>
        <rdfs:comment xml:lang="en">To write address line with e.g. the street name
            and number.</rdfs:comment>
        <rdfs:subPropertyOf rdf:resource="&ebucore;privateMailAddress"/>
    </owl:AnnotationProperty>
    


    <!-- http://www.ebu.ch/metadata/ontologies/ebucore/ebucore#privateAddressLocality -->

    <owl:AnnotationProperty rdf:about="&ebucore;privateAddressLocality">
        <rdfs:label xml:lang="en">Locality</rdfs:label>
        <rdfs:comment xml:lang="en">To provide the name of a city, viallge,
            etc.</rdfs:comment>
        <rdfs:subPropertyOf rdf:resource="&ebucore;privateMailAddress"/>
    </owl:AnnotationProperty>
    


    <!-- http://www.ebu.ch/metadata/ontologies/ebucore/ebucore#privateAddressPostalCode -->

    <owl:AnnotationProperty rdf:about="&ebucore;privateAddressPostalCode">
        <rdfs:label xml:lang="en">Postal code</rdfs:label>
        <rdfs:comment xml:lang="en">To provide an address postal
            code.</rdfs:comment>
        <rdfs:subPropertyOf rdf:resource="&ebucore;privateMailAddress"/>
    </owl:AnnotationProperty>
    


    <!-- http://www.ebu.ch/metadata/ontologies/ebucore/ebucore#privateEmailAddress -->

    <owl:AnnotationProperty rdf:about="&ebucore;privateEmailAddress">
        <rdfs:label xml:lang="en">Private email</rdfs:label>
        <rdfs:comment xml:lang="en">To provide the private email address of an
            agent (Contact/person)</rdfs:comment>
        <rdfs:subPropertyOf rdf:resource="&ebucore;agentEmailAddress"/>
    </owl:AnnotationProperty>
    


    <!-- http://www.ebu.ch/metadata/ontologies/ebucore/ebucore#privateHomepage -->

    <owl:AnnotationProperty rdf:about="&ebucore;privateHomepage">
        <rdfs:label xml:lang="en">Homepage (private)</rdfs:label>
        <rdfs:comment xml:lang="en">To provide an private web homepage of an Agent
            (Contact/person).</rdfs:comment>
        <rdfs:domain rdf:resource="&ebucore;Agent"/>
        <rdfs:subPropertyOf rdf:resource="&ebucore;agentWebHomepage"/>
    </owl:AnnotationProperty>
    


    <!-- http://www.ebu.ch/metadata/ontologies/ebucore/ebucore#privateMailAddress -->

    <owl:AnnotationProperty rdf:about="&ebucore;privateMailAddress">
        <rdfs:label xml:lang="en">Private mail address</rdfs:label>
        <rdfs:comment xml:lang="en">To provide the private / personal address of an
            agent (Contact/person).</rdfs:comment>
        <rdfs:subPropertyOf rdf:resource="&ebucore;agentAddress"/>
    </owl:AnnotationProperty>
    


    <!-- http://www.ebu.ch/metadata/ontologies/ebucore/ebucore#privateMobileTelephoneNumber -->

    <owl:AnnotationProperty rdf:about="&ebucore;privateMobileTelephoneNumber">
        <rdfs:label xml:lang="en">Mobile (private)</rdfs:label>
        <rdfs:comment xml:lang="en">To provide the private mobile telephone number
            of an agent (Contact/person).</rdfs:comment>
        <rdfs:subPropertyOf rdf:resource="&ebucore;agentMobileTelephoneNumber"/>
    </owl:AnnotationProperty>
    


    <!-- http://www.ebu.ch/metadata/ontologies/ebucore/ebucore#privateTelephoneNumber -->

    <owl:AnnotationProperty rdf:about="&ebucore;privateTelephoneNumber">
        <rdfs:label xml:lang="en">Telephone (private)</rdfs:label>
        <rdfs:comment xml:lang="en">To provide the private telephone number of an
            Agent (Contact/person).</rdfs:comment>
        <rdfs:subPropertyOf rdf:resource="&ebucore;agentTelephoneNumber"/>
    </owl:AnnotationProperty>
    


    <!-- http://www.ebu.ch/metadata/ontologies/ebucore/ebucore#promotionalInformation -->

    <owl:AnnotationProperty rdf:about="&ebucore;promotionalInformation">
        <rdfs:label xml:lang="en">Promotional information</rdfs:label>
        <rdfs:comment xml:lang="en">To provide textual promotional information.</rdfs:comment>
        <rdfs:subPropertyOf rdf:resource="&ebucore;description"/>
    </owl:AnnotationProperty>
    


    <!-- http://www.ebu.ch/metadata/ontologies/ebucore/ebucore#pubStatus -->

    <owl:AnnotationProperty rdf:about="&ebucore;pubStatus">
        <rdfs:label xml:lang="en">Publication status</rdfs:label>
        <rdfs:comment xml:lang="en">To indicate a publication status.</rdfs:comment>
        <rdfs:subPropertyOf rdf:resource="&ebucore;description"/>
    </owl:AnnotationProperty>
    


    <!-- http://www.ebu.ch/metadata/ontologies/ebucore/ebucore#publicationChannelName -->

    <owl:AnnotationProperty rdf:about="&ebucore;publicationChannelName">
        <rdfs:label xml:lang="en">Publication channel name</rdfs:label>
        <rdfs:comment xml:lang="en">To provide a name to a PublicationChannel e.g. a TV channel or website.</rdfs:comment>
        <rdfs:domain rdf:resource="&ebucore;PublicationChannel"/>
    </owl:AnnotationProperty>
    


    <!-- http://www.ebu.ch/metadata/ontologies/ebucore/ebucore#publicationEndDateTime -->

    <owl:AnnotationProperty rdf:about="&ebucore;publicationEndDateTime">
        <rdfs:label xml:lang="en">Publication end date &amp; time</rdfs:label>
        <rdfs:comment xml:lang="en">The actual end date and time of a PublicationEvent.</rdfs:comment>
        <rdfs:domain rdf:resource="&ebucore;PublicationEvent"/>
    </owl:AnnotationProperty>
    


    <!-- http://www.ebu.ch/metadata/ontologies/ebucore/ebucore#publicationEventName -->

    <owl:AnnotationProperty rdf:about="&ebucore;publicationEventName">
        <rdfs:label xml:lang="en">Publication event name</rdfs:label>
        <rdfs:comment xml:lang="en">To provide a name to a PublicationEvent.</rdfs:comment>
        <rdfs:domain rdf:resource="&ebucore;PublicationEvent"/>
    </owl:AnnotationProperty>
    


    <!-- http://www.ebu.ch/metadata/ontologies/ebucore/ebucore#publicationScheduleDate -->

    <owl:AnnotationProperty rdf:about="&ebucore;publicationScheduleDate">
        <rdfs:label xml:lang="en">schedule date</rdfs:label>
        <rdfs:comment xml:lang="en">To express specifically the schedule date to which a PublicationEvent is related in particular if the broacdast time is after midnight. For example, the schedule date would be May 29th and the programme is published at 1 am on May 30th, while still associated in the schedule with the night of May 29th.</rdfs:comment>
        <rdfs:domain rdf:resource="&ebucore;PublicationEvent"/>
    </owl:AnnotationProperty>
    


    <!-- http://www.ebu.ch/metadata/ontologies/ebucore/ebucore#publicationStartDateTime -->

    <owl:AnnotationProperty rdf:about="&ebucore;publicationStartDateTime">
        <rdfs:label xml:lang="en">Publication start date &amp; time</rdfs:label>
        <rdfs:comment xml:lang="en">The actual start date and time of a PublicationEvent.</rdfs:comment>
        <rdfs:domain rdf:resource="&ebucore;PublicationEvent"/>
    </owl:AnnotationProperty>
    


    <!-- http://www.ebu.ch/metadata/ontologies/ebucore/ebucore#publishedEndDateTime -->

    <owl:AnnotationProperty rdf:about="&ebucore;publishedEndDateTime">
        <rdfs:label xml:lang="en">Publication end date &amp; time</rdfs:label>
        <rdfs:comment xml:lang="en">The end date and time of a PublicationEvent as
            scheduled.</rdfs:comment>
        <rdfs:domain rdf:resource="&ebucore;PublicationEvent"/>
    </owl:AnnotationProperty>
    


    <!-- http://www.ebu.ch/metadata/ontologies/ebucore/ebucore#publishedStartDateTime -->

    <owl:AnnotationProperty rdf:about="&ebucore;publishedStartDateTime">
        <rdfs:label xml:lang="en">Publication start date &amp; time</rdfs:label>
        <rdfs:comment xml:lang="en">The start date and time of a PublicationEvent
            as scheduled.</rdfs:comment>
        <rdfs:domain rdf:resource="&ebucore;PublicationEvent"/>
    </owl:AnnotationProperty>
    


    <!-- http://www.ebu.ch/metadata/ontologies/ebucore/ebucore#publishedTitle -->

    <owl:AnnotationProperty rdf:about="&ebucore;publishedTitle">
        <rdfs:label xml:lang="en">Published title.</rdfs:label>
        <rdfs:comment xml:lang="en">The title used to identify the work at publication time.</rdfs:comment>
        <rdfs:subPropertyOf rdf:resource="&dc;title"/>
    </owl:AnnotationProperty>
    


    <!-- http://www.ebu.ch/metadata/ontologies/ebucore/ebucore#ratingScaleMax -->

    <owl:AnnotationProperty rdf:about="&ebucore;ratingScaleMax">
        <rdfs:label xml:lang="en">Rating scale (top value)</rdfs:label>
        <rdfs:comment xml:lang="en">The maximum value of the scale used for rating
            a media resource.</rdfs:comment>
        <rdfs:domain rdf:resource="&ebucore;Rating"/>
    </owl:AnnotationProperty>
    


    <!-- http://www.ebu.ch/metadata/ontologies/ebucore/ebucore#ratingScaleMin -->

    <owl:AnnotationProperty rdf:about="&ebucore;ratingScaleMin">
        <rdfs:label xml:lang="en">Rating scale (min. value)</rdfs:label>
        <rdfs:comment xml:lang="en">The minimum value of the scale used for rating
            a Resource.</rdfs:comment>
        <rdfs:domain rdf:resource="&ebucore;Rating"/>
    </owl:AnnotationProperty>
    


    <!-- http://www.ebu.ch/metadata/ontologies/ebucore/ebucore#ratingSystemEnvironment -->

    <owl:AnnotationProperty rdf:about="&ebucore;ratingSystemEnvironment">
        <rdfs:label xml:lang="en">Rating environment</rdfs:label>
        <rdfs:comment xml:lang="en">To identify the environment in which rating applies.</rdfs:comment>
        <rdfs:domain rdf:resource="&ebucore;Rating"/>
    </owl:AnnotationProperty>
    


    <!-- http://www.ebu.ch/metadata/ontologies/ebucore/ebucore#ratingSystemName -->

    <owl:AnnotationProperty rdf:about="&ebucore;ratingSystemName">
        <rdfs:label xml:lang="en">Rating system</rdfs:label>
        <rdfs:comment xml:lang="en">To identify a rating system by its name.</rdfs:comment>
        <rdfs:domain rdf:resource="&ebucore;Rating"/>
    </owl:AnnotationProperty>
    


    <!-- http://www.ebu.ch/metadata/ontologies/ebucore/ebucore#ratingValue -->

    <owl:AnnotationProperty rdf:about="&ebucore;ratingValue">
        <rdfs:label xml:lang="en">Rating</rdfs:label>
        <rdfs:comment xml:lang="en">To express a free text rating value defined in
            a rating classification scheme.</rdfs:comment>
        <rdfs:domain rdf:resource="&ebucore;Rating"/>
    </owl:AnnotationProperty>
    


    <!-- http://www.ebu.ch/metadata/ontologies/ebucore/ebucore#reason -->

    <owl:AnnotationProperty rdf:about="&ebucore;reason">
        <rdfs:label xml:lang="en">Reason</rdfs:label>
        <rdfs:comment xml:lang="en">To provide a reason for which Rating as been attributed as provided.</rdfs:comment>
        <rdfs:domain rdf:resource="&ebucore;Rating"/>
    </owl:AnnotationProperty>
    


    <!-- http://www.ebu.ch/metadata/ontologies/ebucore/ebucore#references -->

    <owl:AnnotationProperty rdf:about="&ebucore;references">
        <rdfs:label xml:lang="en">References</rdfs:label>
        <rdfs:comment xml:lang="en">To express a reference between Assets, BusinessObjects or Resources.</rdfs:comment>
        <rdfs:domain rdf:resource="_:genid8"/>
        <rdfs:subPropertyOf rdf:resource="&dc;relation"/>
    </owl:AnnotationProperty>
    


    <!-- http://www.ebu.ch/metadata/ontologies/ebucore/ebucore#regionDelimX -->

    <owl:AnnotationProperty rdf:about="&ebucore;regionDelimX">
        <rdfs:label xml:lang="en">Region delimiter (x-axis)</rdfs:label>
        <rdfs:comment xml:lang="en">To define the bottom right corner of a zone on
            the x-axis. If present with regionDelimY, the zone definition is complemented by the
            associated values of the height and width.</rdfs:comment>
        <rdfs:domain rdf:resource="&ebucore;Resource"/>
    </owl:AnnotationProperty>
    


    <!-- http://www.ebu.ch/metadata/ontologies/ebucore/ebucore#regionDelimY -->

    <owl:AnnotationProperty rdf:about="&ebucore;regionDelimY">
        <rdfs:label xml:lang="en">Region delimiter (y-axis)</rdfs:label>
        <rdfs:comment xml:lang="en">To define the bottom right corner of a zone on
            the y-axis. If present with regionDelimX, the zone definition is complemented by the
            associated values of the height and width.</rdfs:comment>
        <rdfs:domain rdf:resource="&ebucore;Resource"/>
    </owl:AnnotationProperty>
    


    <!-- http://www.ebu.ch/metadata/ontologies/ebucore/ebucore#relatedLink -->

    <owl:AnnotationProperty rdf:about="&ebucore;relatedLink">
        <rdfs:label xml:lang="en">Related resources</rdfs:label>
        <rdfs:comment xml:lang="en">To provide a link to a web resource containing
            information related to an Agent (Contact/person or Organisation).</rdfs:comment>
        <rdfs:domain rdf:resource="&ebucore;Agent"/>
    </owl:AnnotationProperty>
    


    <!-- http://www.ebu.ch/metadata/ontologies/ebucore/ebucore#replaces -->

    <owl:AnnotationProperty rdf:about="&ebucore;replaces">
        <rdfs:label xml:lang="en">Replaces</rdfs:label>
        <rdfs:comment xml:lang="en">To identify substitution.</rdfs:comment>
        <rdfs:domain rdf:resource="_:genid85"/>
        <rdfs:subPropertyOf rdf:resource="&dc;relation"/>
    </owl:AnnotationProperty>
    


    <!-- http://www.ebu.ch/metadata/ontologies/ebucore/ebucore#requires -->

    <owl:AnnotationProperty rdf:about="&ebucore;requires">
        <rdfs:label xml:lang="en">Requires</rdfs:label>
        <rdfs:comment xml:lang="en">To express dependency.</rdfs:comment>
        <rdfs:domain rdf:resource="_:genid100"/>
        <rdfs:subPropertyOf rdf:resource="&dc;relation"/>
    </owl:AnnotationProperty>
    


    <!-- http://www.ebu.ch/metadata/ontologies/ebucore/ebucore#resourceDescription -->

    <owl:AnnotationProperty rdf:about="&ebucore;resourceDescription">
        <rdfs:label rdf:datatype="&xsd;string">Resource description</rdfs:label>
        <rdfs:comment rdf:datatype="&xsd;string">This can be specialised by using sub-properties
            like defined in http://www.ebu.ch/metadata/cs/web/ebu_DescriptionTypeCodeCS_p.xml.htm
            implemented as examples as e.g. &apos;summary&apos; or
            &apos;script&apos;.</rdfs:comment>
        <rdfs:subPropertyOf rdf:resource="&dc;description"/>
        <rdfs:domain rdf:resource="&ebucore;MediaResource"/>
    </owl:AnnotationProperty>
    


    <!-- http://www.ebu.ch/metadata/ontologies/ebucore/ebucore#resourceName -->

    <owl:AnnotationProperty rdf:about="&ebucore;resourceName">
        <rdfs:label xml:lang="en">Resource description</rdfs:label>
        <rdfs:comment xml:lang="en">A name by which the resource can be identified.</rdfs:comment>
        <rdfs:domain rdf:resource="&ebucore;Resource"/>
    </owl:AnnotationProperty>
    


    <!-- http://www.ebu.ch/metadata/ontologies/ebucore/ebucore#review -->

    <owl:AnnotationProperty rdf:about="&ebucore;review">
        <rdfs:label xml:lang="en">Review</rdfs:label>
        <rdfs:comment xml:lang="en">To provide a text for a review.</rdfs:comment>
        <rdfs:subPropertyOf rdf:resource="&ebucore;description"/>
    </owl:AnnotationProperty>
    


    <!-- http://www.ebu.ch/metadata/ontologies/ebucore/ebucore#rightsExpression -->

    <owl:AnnotationProperty rdf:about="&ebucore;rightsExpression">
        <rdfs:label xml:lang="en">Rights expression</rdfs:label>
        <rdfs:comment xml:lang="en">The expression of Rights as free
            text.</rdfs:comment>
        <rdfs:domain rdf:resource="&ebucore;Rights"/>
    </owl:AnnotationProperty>
    


    <!-- http://www.ebu.ch/metadata/ontologies/ebucore/ebucore#rightsLink -->

    <owl:AnnotationProperty rdf:about="&ebucore;rightsLink">
        <rdfs:label xml:lang="en">Rights web resource</rdfs:label>
        <rdfs:comment xml:lang="en">A link to e.g. a webpage where an expression of
            the rights can be found and consulted.</rdfs:comment>
        <rdfs:domain rdf:resource="&ebucore;Rights"/>
    </owl:AnnotationProperty>
    


    <!-- http://www.ebu.ch/metadata/ontologies/ebucore/ebucore#roleDefinition -->

    <owl:AnnotationProperty rdf:about="&ebucore;roleDefinition">
        <rdfs:label xml:lang="en">Role definition</rdfs:label>
        <rdfs:comment xml:lang="en">To provide a definition for a role</rdfs:comment>
        <rdfs:domain rdf:resource="&ebucore;Role"/>
    </owl:AnnotationProperty>
    


    <!-- http://www.ebu.ch/metadata/ontologies/ebucore/ebucore#sampleSize -->

    <owl:AnnotationProperty rdf:about="&ebucore;sampleSize">
        <rdfs:label xml:lang="en">Sample size</rdfs:label>
        <rdfs:comment xml:lang="en">The size of an audio sample in
            bits. Also called bit depth.</rdfs:comment>
        <rdfs:domain rdf:resource="&ebucore;AudioFormat"/>
    </owl:AnnotationProperty>
    


    <!-- http://www.ebu.ch/metadata/ontologies/ebucore/ebucore#sampleType -->

    <owl:AnnotationProperty rdf:about="&ebucore;sampleType">
        <rdfs:label xml:lang="en">Sample type</rdfs:label>
        <rdfs:comment xml:lang="en">The type of audio sample.</rdfs:comment>
        <rdfs:domain rdf:resource="&ebucore;AudioFormat"/>
    </owl:AnnotationProperty>
    


    <!-- http://www.ebu.ch/metadata/ontologies/ebucore/ebucore#scanningFormat -->

    <owl:AnnotationProperty rdf:about="&ebucore;scanningFormat">
        <rdfs:label xml:lang="en">Sampling format</rdfs:label>
        <rdfs:comment xml:lang="en">To define the scanning format for a
            MediaResource. For video, the two main values are &quot;interlaced&quot; or
            &quot;progressive&quot;.</rdfs:comment>
        <rdfs:domain rdf:resource="&ebucore;VideoFormat"/>
    </owl:AnnotationProperty>
    


    <!-- http://www.ebu.ch/metadata/ontologies/ebucore/ebucore#script -->

    <owl:AnnotationProperty rdf:about="&ebucore;script">
        <rdfs:label xml:lang="en">Script</rdfs:label>
        <rdfs:comment xml:lang="en">To provide a script.</rdfs:comment>
        <rdfs:subPropertyOf rdf:resource="&ebucore;description"/>
    </owl:AnnotationProperty>
    


    <!-- http://www.ebu.ch/metadata/ontologies/ebucore/ebucore#signingSource -->

    <owl:AnnotationProperty rdf:about="&ebucore;signingSource">
        <rdfs:label xml:lang="en">Signing source</rdfs:label>
        <rdfs:comment xml:lang="en">To identify the source of the signing
            resource.</rdfs:comment>
        <rdfs:domain rdf:resource="&ebucore;Signing"/>
    </owl:AnnotationProperty>
    


    <!-- http://www.ebu.ch/metadata/ontologies/ebucore/ebucore#start -->

    <owl:AnnotationProperty rdf:about="&ebucore;start">
        <rdfs:label xml:lang="en">Start time</rdfs:label>
        <rdfs:comment xml:lang="en">The start point of the MediaResource.</rdfs:comment>
        <rdfs:domain rdf:resource="_:genid212"/>
    </owl:AnnotationProperty>
    


    <!-- http://www.ebu.ch/metadata/ontologies/ebucore/ebucore#startNormalPlayTime -->

    <owl:AnnotationProperty rdf:about="&ebucore;startNormalPlayTime">
        <rdfs:label xml:lang="en">Start time (time)</rdfs:label>
        <rdfs:comment xml:lang="en">The start time expressed using a time
            expression.</rdfs:comment>
        <rdfs:subPropertyOf rdf:resource="&ebucore;start"/>
    </owl:AnnotationProperty>
    


    <!-- http://www.ebu.ch/metadata/ontologies/ebucore/ebucore#startNumberEditUnits -->

    <owl:AnnotationProperty rdf:about="&ebucore;startNumberEditUnits">
        <rdfs:label xml:lang="en">Start time (edit units)</rdfs:label>
        <rdfs:comment xml:lang="en">A start time expressed as a number of edit
            units.</rdfs:comment>
        <rdfs:subPropertyOf rdf:resource="&ebucore;start"/>
    </owl:AnnotationProperty>
    


    <!-- http://www.ebu.ch/metadata/ontologies/ebucore/ebucore#startTimecode -->

    <owl:AnnotationProperty rdf:about="&ebucore;startTimecode">
        <rdfs:label xml:lang="en">Start time (timecode)</rdfs:label>
        <rdfs:comment xml:lang="en">A start time expressed as
            timecode.</rdfs:comment>
        <rdfs:subPropertyOf rdf:resource="&ebucore;start"/>
    </owl:AnnotationProperty>
    


    <!-- http://www.ebu.ch/metadata/ontologies/ebucore/ebucore#storageDefinition -->

    <owl:AnnotationProperty rdf:about="&ebucore;storageDefinition">
        <rdfs:label xml:lang="en">Storage definition</rdfs:label>
        <rdfs:comment xml:lang="en">To provide a definition for storage.</rdfs:comment>
        <rdfs:domain rdf:resource="&ebucore;StorageType"/>
    </owl:AnnotationProperty>
    


    <!-- http://www.ebu.ch/metadata/ontologies/ebucore/ebucore#subtitle -->

    <owl:AnnotationProperty rdf:about="&ebucore;subtitle">
        <rdfs:label xml:lang="en">Subtitle</rdfs:label>
        <rdfs:comment xml:lang="en">A complementary subtitle.</rdfs:comment>
        <rdfs:subPropertyOf rdf:resource="&ebucore;alternativeTitle"/>
    </owl:AnnotationProperty>
    


    <!-- http://www.ebu.ch/metadata/ontologies/ebucore/ebucore#subtitlingSource -->

    <owl:AnnotationProperty rdf:about="&ebucore;subtitlingSource">
        <rdfs:label xml:lang="en">Subtitling source</rdfs:label>
        <rdfs:comment xml:lang="en">To identify the source of the Subtitling
            resource.</rdfs:comment>
        <rdfs:domain rdf:resource="&ebucore;Subtitling"/>
    </owl:AnnotationProperty>
    


    <!-- http://www.ebu.ch/metadata/ontologies/ebucore/ebucore#summary -->

    <owl:AnnotationProperty rdf:about="&ebucore;summary">
        <rdfs:label xml:lang="en">Summary</rdfs:label>
        <rdfs:comment xml:lang="en">To provide a summary.</rdfs:comment>
        <rdfs:subPropertyOf rdf:resource="&ebucore;description"/>
    </owl:AnnotationProperty>
    


    <!-- http://www.ebu.ch/metadata/ontologies/ebucore/ebucore#synopsis -->

    <owl:AnnotationProperty rdf:about="&ebucore;synopsis">
        <rdfs:label xml:lang="en">Synopsis</rdfs:label>
        <rdfs:comment xml:lang="en">To provide a summary.</rdfs:comment>
        <rdfs:subPropertyOf rdf:resource="&ebucore;description"/>
    </owl:AnnotationProperty>
    


    <!-- http://www.ebu.ch/metadata/ontologies/ebucore/ebucore#tableOfContent -->

    <owl:AnnotationProperty rdf:about="&ebucore;tableOfContent">
        <rdfs:label xml:lang="en">Table of Content</rdfs:label>
        <rdfs:comment xml:lang="en">To provide a Table of Content.</rdfs:comment>
        <rdfs:subPropertyOf rdf:resource="&ebucore;description"/>
    </owl:AnnotationProperty>
    


    <!-- http://www.ebu.ch/metadata/ontologies/ebucore/ebucore#targetAudienceSystem -->

    <owl:AnnotationProperty rdf:about="&ebucore;targetAudienceSystem">
        <rdfs:label xml:lang="en">Target audience system</rdfs:label>
        <rdfs:comment xml:lang="en">To define the system used to provide a TargetAudience.</rdfs:comment>
        <rdfs:domain rdf:resource="&ebucore;audienceLevel"/>
    </owl:AnnotationProperty>
    


    <!-- http://www.ebu.ch/metadata/ontologies/ebucore/ebucore#textualAnnotation -->

    <owl:AnnotationProperty rdf:about="&ebucore;textualAnnotation">
        <rdfs:label xml:lang="en">Note</rdfs:label>
        <rdfs:comment xml:lang="en">The value of an Annotation as free
            text.</rdfs:comment>
        <rdfs:domain rdf:resource="&ebucore;Annotation"/>
    </owl:AnnotationProperty>
    


    <!-- http://www.ebu.ch/metadata/ontologies/ebucore/ebucore#title -->

    <owl:AnnotationProperty rdf:about="&ebucore;title">
        <rdfs:label xml:lang="en">Title</rdfs:label>
        <rdfs:comment xml:lang="en">All value of the EBU title status
            classification scheme
            (http://www.ebu.ch/metadata/cs/web/ebu_TitleStatusCodeCS_p.xml.htm) are candidates
            subproperties of the title property as implemented for an example with
            alternativeTitle.</rdfs:comment>
        <rdfs:comment xml:lang="en">Specifies the title or name given to the
            resource.  A root for the definition of subproperties defining ebucore titles of different types. The ebucore title type can be used to define sub-properties to optionally refine the category of
            the title.</rdfs:comment>
        <rdfs:subPropertyOf rdf:resource="&dc;title"/>
    </owl:AnnotationProperty>
    


    <!-- http://www.ebu.ch/metadata/ontologies/ebucore/ebucore#trackDefinition -->

    <owl:AnnotationProperty rdf:about="&ebucore;trackDefinition">
        <rdfs:label xml:lang="en">Definition</rdfs:label>
        <rdfs:comment xml:lang="en">To provide a definition associated to a
            Track.</rdfs:comment>
        <rdfs:domain rdf:resource="&ebucore;Track"/>
    </owl:AnnotationProperty>
    


    <!-- http://www.ebu.ch/metadata/ontologies/ebucore/ebucore#trackName -->

    <owl:AnnotationProperty rdf:about="&ebucore;trackName">
        <rdfs:label xml:lang="en">Track name</rdfs:label>
        <rdfs:comment xml:lang="en">The name attributed to a Track.</rdfs:comment>
        <rdfs:domain rdf:resource="&ebucore;Track"/>
    </owl:AnnotationProperty>
    


    <!-- http://www.ebu.ch/metadata/ontologies/ebucore/ebucore#translationTitle -->

    <owl:AnnotationProperty rdf:about="&ebucore;translationTitle">
        <rdfs:label xml:lang="en">Translation title</rdfs:label>
        <rdfs:comment xml:lang="en">A translated version of the title.</rdfs:comment>
        <rdfs:subPropertyOf rdf:resource="&ebucore;alternativeTitle"/>
    </owl:AnnotationProperty>
    


    <!-- http://www.ebu.ch/metadata/ontologies/ebucore/ebucore#versionTitle -->

    <owl:AnnotationProperty rdf:about="&ebucore;versionTitle">
        <rdfs:label xml:lang="en">Version title</rdfs:label>
        <rdfs:comment xml:lang="en">An alternative title specific to a verison of content.</rdfs:comment>
        <rdfs:subPropertyOf rdf:resource="&ebucore;alternativeTitle"/>
    </owl:AnnotationProperty>
    


    <!-- http://www.ebu.ch/metadata/ontologies/ebucore/ebucore#width -->

    <owl:AnnotationProperty rdf:about="&ebucore;width">
        <rdfs:label xml:lang="en">Width</rdfs:label>
        <rdfs:comment xml:lang="en">The width of e.g. a video frame typically
            expressed as a number of pixels, or picture/image in millimeters.</rdfs:comment>
        <rdfs:domain rdf:resource="&ebucore;Resource"/>
    </owl:AnnotationProperty>
    


    <!-- http://www.ebu.ch/metadata/ontologies/ebucore/ebucore#widthUnit -->

    <owl:AnnotationProperty rdf:about="&ebucore;widthUnit">
        <rdfs:label xml:lang="en">Width unit</rdfs:label>
        <rdfs:comment xml:lang="en">The unit used to measure a width e.g. in pixels
            or number of lines or millimeters or else.</rdfs:comment>
        <rdfs:domain rdf:resource="&ebucore;Resource"/>
    </owl:AnnotationProperty>
    


    <!-- http://www.ebu.ch/metadata/ontologies/ebucore/ebucore#wordCount -->

    <owl:AnnotationProperty rdf:about="&ebucore;wordCount">
        <rdfs:label xml:lang="en">Word count</rdfs:label>
        <rdfs:comment xml:lang="en">The number of words contained in a
            document.</rdfs:comment>
        <rdfs:domain rdf:resource="&ebucore;Document"/>
    </owl:AnnotationProperty>
    


    <!-- http://www.ebu.ch/metadata/ontologies/ebucore/ebucore#workingTitle -->

    <owl:AnnotationProperty rdf:about="&ebucore;workingTitle">
        <rdfs:label xml:lang="en">Working title</rdfs:label>
        <rdfs:comment xml:lang="en">A title used while content is not complete.</rdfs:comment>
        <rdfs:subPropertyOf rdf:resource="&ebucore;alternativeTitle"/>
    </owl:AnnotationProperty>
    


    <!-- http://www.ebu.ch/metadata/ontologies/ebucore/ebucore#wrappingType -->

    <owl:AnnotationProperty rdf:about="&ebucore;wrappingType">
        <rdfs:label xml:lang="en">Wrapping type</rdfs:label>
        <rdfs:comment xml:lang="en">To provide additional information on the
            wrapping type of ancillary data.</rdfs:comment>
        <rdfs:domain rdf:resource="&ebucore;AncillaryData"/>
    </owl:AnnotationProperty>
    


    <!-- http://www.w3.org/2004/02/skos/core#prefLabel -->

    <rdf:Description rdf:about="&skos;prefLabel">
        <rdfs:isDefinedBy rdf:resource="http://www.w3.org/2004/02/skos/core"/>
    </rdf:Description>
    


    <!-- http://xmlns.com/foaf/0.1/age -->

    <owl:AnnotationProperty rdf:about="&foaf;age">
        <rdfs:label rdf:datatype="&xsd;string">age</rdfs:label>
        <rdfs:subPropertyOf rdf:resource="&ebucore;agentAge"/>
    </owl:AnnotationProperty>
    


    <!-- http://xmlns.com/foaf/0.1/familyName -->

    <owl:AnnotationProperty rdf:about="&foaf;familyName">
        <rdfs:subPropertyOf rdf:resource="&ebucore;familyName"/>
    </owl:AnnotationProperty>
    


    <!-- http://xmlns.com/foaf/0.1/givenName -->

    <owl:AnnotationProperty rdf:about="&foaf;givenName">
        <rdfs:subPropertyOf rdf:resource="&ebucore;givenName"/>
    </owl:AnnotationProperty>
    


    <!-- http://xmlns.com/foaf/0.1/member -->

    <owl:AnnotationProperty rdf:about="&foaf;member">
        <rdfs:label xml:lang="en">Group member</rdfs:label>
        <rdfs:comment xml:lang="en">To identify an Agent member of a Group.</rdfs:comment>
        <rdfs:domain rdf:resource="&foaf;Group"/>
    </owl:AnnotationProperty>
    


    <!-- http://xmlns.com/foaf/0.1/title -->

    <owl:AnnotationProperty rdf:about="&foaf;title">
        <rdfs:subPropertyOf rdf:resource="&ebucore;nameTitle"/>
    </owl:AnnotationProperty>
    


    <!-- 
    ///////////////////////////////////////////////////////////////////////////////////////
    //
    // Datatypes
    //
    ///////////////////////////////////////////////////////////////////////////////////////
     -->

    


    <!-- http://www.w3.org/2001/XMLSchema#date -->

    <rdfs:Datatype rdf:about="&xsd;date"/>
    


    <!-- http://www.w3.org/2001/XMLSchema#duration -->

    <rdfs:Datatype rdf:about="&xsd;duration"/>
    


    <!-- http://www.w3.org/2001/XMLSchema#time -->

    <rdfs:Datatype rdf:about="&xsd;time"/>
    


    <!-- 
    ///////////////////////////////////////////////////////////////////////////////////////
    //
    // Object Properties
    //
    ///////////////////////////////////////////////////////////////////////////////////////
     -->

    


    <!-- http://purl.org/dc/elements/1.1/relation -->

    <rdf:Description rdf:about="&dc;relation">
        <rdfs:label xml:lang="en">Relation</rdfs:label>
        <rdfs:comment xml:lang="en">A relation between BusinessObjects and resources.</rdfs:comment>
    </rdf:Description>
    


    <!-- http://www.ebu.ch/metadata/ontologies/ebucore/ebucore#appliesOutOf -->

    <owl:ObjectProperty rdf:about="&ebucore;appliesOutOf">
        <rdfs:label xml:lang="en">Exclusion area</rdfs:label>
        <rdfs:comment xml:lang="en">To define the Location (e.g. country, region) to which Rating and TargetAudience do NOT apply.</rdfs:comment>
        <rdfs:range rdf:resource="&ebucore;Location"/>
    </owl:ObjectProperty>
    


    <!-- http://www.ebu.ch/metadata/ontologies/ebucore/ebucore#appliesTo -->

    <owl:ObjectProperty rdf:about="&ebucore;appliesTo">
        <rdfs:label xml:lang="en">Coverage</rdfs:label>
        <rdfs:comment xml:lang="en">To define the location/region to which Rating and TargetAudience apply.</rdfs:comment>
        <rdfs:range rdf:resource="&ebucore;Location"/>
    </owl:ObjectProperty>
    


    <!-- http://www.ebu.ch/metadata/ontologies/ebucore/ebucore#followsInSequence -->

    <owl:ObjectProperty rdf:about="&ebucore;followsInSequence">
        <rdfs:label rdf:datatype="&xsd;string">Previous</rdfs:label>
        <rdfs:comment rdf:datatype="&xsd;string">A link to a an BusinessObject or a Resource preceding the current BusinessObject or Resource in an ordered sequence</rdfs:comment>
        <rdfs:subPropertyOf rdf:resource="&dc;relation"/>
        <rdfs:domain>
            <owl:Class>
                <owl:unionOf rdf:parseType="Collection">
                    <rdf:Description rdf:about="&ebucore;BusinessObject"/>
                    <rdf:Description rdf:about="&ebucore;Resource"/>
                </owl:unionOf>
            </owl:Class>
        </rdfs:domain>
        <rdfs:range>
            <owl:Class>
                <owl:unionOf rdf:parseType="Collection">
                    <rdf:Description rdf:about="&ebucore;BusinessObject"/>
                    <rdf:Description rdf:about="&ebucore;Resource"/>
                </owl:unionOf>
            </owl:Class>
        </rdfs:range>
    </owl:ObjectProperty>
    


    <!-- http://www.ebu.ch/metadata/ontologies/ebucore/ebucore#hasAffiliation -->

    <owl:ObjectProperty rdf:about="&ebucore;hasAffiliation">
        <rdfs:label xml:lang="en">Affiliation</rdfs:label>
        <rdfs:comment xml:lang="en">A property to establish the relation between a
            Contact/person and an Organisation.</rdfs:comment>
        <rdfs:range rdf:resource="&ebucore;Affiliation"/>
    </owl:ObjectProperty>
    


    <!-- http://www.ebu.ch/metadata/ontologies/ebucore/ebucore#hasAncillaryData -->

    <owl:ObjectProperty rdf:about="&ebucore;hasAncillaryData">
        <rdfs:label xml:lang="en">Ancillary data</rdfs:label>
        <rdfs:comment xml:lang="en">A property to signal the presence of
            AncillaryData associated with the EditorialObject and / or MediaResource.</rdfs:comment>
        <rdfs:range rdf:resource="&ebucore;AncillaryData"/>
    </owl:ObjectProperty>
    


    <!-- http://www.ebu.ch/metadata/ontologies/ebucore/ebucore#hasAnnotationSource -->

    <owl:ObjectProperty rdf:about="&ebucore;hasAnnotationSource">
        <rdfs:label xml:lang="en">Annotation Source</rdfs:label>
        <rdfs:comment xml:lang="en">To identify the Agent, Contact/person or
            Organisation who has provided the Annotation.</rdfs:comment>
        <rdfs:range rdf:resource="&ebucore;Agent"/>
    </owl:ObjectProperty>
    


    <!-- http://www.ebu.ch/metadata/ontologies/ebucore/ebucore#hasCaptioning -->

    <owl:ObjectProperty rdf:about="&ebucore;hasCaptioning">
        <rdfs:label xml:lang="en">Captioning</rdfs:label>
        <rdfs:comment xml:lang="en">To signal the presence of
            Captioning.</rdfs:comment>
        <rdfs:range rdf:resource="&ebucore;Captioning"/>
    </owl:ObjectProperty>
    


    <!-- http://www.ebu.ch/metadata/ontologies/ebucore/ebucore#hasCastRole -->

    <owl:ObjectProperty rdf:about="&ebucore;hasCastRole">
        <rdfs:label xml:lang="en">Cast role</rdfs:label>
        <rdfs:comment xml:lang="en">To define the roles involved in the creation of or related to the BusinessObject. The Role acts as a link to the Agent fulfilling that function.</rdfs:comment>
        <rdfs:range rdf:resource="&ebucore;Role"/>
    </owl:ObjectProperty>
    


    <!-- http://www.ebu.ch/metadata/ontologies/ebucore/ebucore#hasContact -->

    <owl:ObjectProperty rdf:about="&ebucore;hasContact">
        <rdfs:label xml:lang="en">Contact</rdfs:label>
        <rdfs:comment xml:lang="en">To provide information on a Contact for an
            Organisation or a physical person (e.g. the agent of an actor).</rdfs:comment>
        <rdfs:range rdf:resource="&ebucore;Contact"/>
    </owl:ObjectProperty>
    


    <!-- http://www.ebu.ch/metadata/ontologies/ebucore/ebucore#hasCreationLocation -->

    <owl:ObjectProperty rdf:about="&ebucore;hasCreationLocation">
        <rdfs:label xml:lang="en">Creation location</rdfs:label>
        <rdfs:comment xml:lang="en">The Location where content has been created.</rdfs:comment>
        <rdfs:range rdf:resource="&ebucore;Location"/>
    </owl:ObjectProperty>
    


    <!-- http://www.ebu.ch/metadata/ontologies/ebucore/ebucore#hasDepartment -->

    <owl:ObjectProperty rdf:about="&ebucore;hasDepartment">
        <rdfs:label xml:lang="en">Department</rdfs:label>
        <rdfs:comment xml:lang="en">To identify Departments within an
            Organisation.</rdfs:comment>
        <rdfs:range rdf:resource="&ebucore;Department"/>
    </owl:ObjectProperty>
    


    <!-- http://www.ebu.ch/metadata/ontologies/ebucore/ebucore#hasDopesheet -->

    <owl:ObjectProperty rdf:about="&ebucore;hasDopesheet">
        <rdfs:label xml:lang="en">Dopesheet</rdfs:label>
        <rdfs:comment xml:lang="en">To associate a Dopesheet with a NewsItem.</rdfs:comment>
        <rdfs:range rdf:resource="&ebucore;Dopesheet"/>
    </owl:ObjectProperty>
    


    <!-- http://www.ebu.ch/metadata/ontologies/ebucore/ebucore#hasEpisode -->

    <owl:ObjectProperty rdf:about="&ebucore;hasEpisode">
        <rdfs:label xml:lang="en">Episode</rdfs:label>
        <rdfs:comment xml:lang="en">To identify an episode of a
            Series or a Season.</rdfs:comment>
        <rdfs:range rdf:resource="&ebucore;Programme"/>
        <rdfs:subPropertyOf rdf:resource="&ebucore;hasRelatedBusinessObject"/>
        <owl:inverseOf rdf:resource="&ebucore;isEpisodeOf"/>
        <rdfs:domain>
            <owl:Class>
                <owl:unionOf rdf:parseType="Collection">
                    <rdf:Description rdf:about="&ebucore;Season"/>
                    <rdf:Description rdf:about="&ebucore;Series"/>
                </owl:unionOf>
            </owl:Class>
        </rdfs:domain>
    </owl:ObjectProperty>
    


    <!-- http://www.ebu.ch/metadata/ontologies/ebucore/ebucore#hasEvent -->

    <owl:ObjectProperty rdf:about="&ebucore;hasEvent">
        <rdfs:label xml:lang="en">Event</rdfs:label>
        <rdfs:comment xml:lang="en">To associate an Event with a
            Location.</rdfs:comment>
        <rdfs:range rdf:resource="&ebucore;Event"/>
    </owl:ObjectProperty>
    


    <!-- http://www.ebu.ch/metadata/ontologies/ebucore/ebucore#hasKeyCareerEvent -->

    <owl:ObjectProperty rdf:about="&ebucore;hasKeyCareerEvent">
        <rdfs:label rdf:datatype="&xsd;string">Career event</rdfs:label>
        <rdfs:range rdf:resource="&ebucore;KeyCareerEvent"/>
    </owl:ObjectProperty>
    


    <!-- http://www.ebu.ch/metadata/ontologies/ebucore/ebucore#hasKeyPersonalEvent -->

    <owl:ObjectProperty rdf:about="&ebucore;hasKeyPersonalEvent">
        <rdfs:label rdf:datatype="&xsd;string">Personal event</rdfs:label>
        <rdfs:range rdf:resource="&ebucore;KeyPersonalEvent"/>
    </owl:ObjectProperty>
    


    <!-- http://www.ebu.ch/metadata/ontologies/ebucore/ebucore#hasLogo -->

    <owl:ObjectProperty rdf:about="&ebucore;hasLogo">
        <rdfs:label xml:lang="en">Logo</rdfs:label>
        <rdfs:comment xml:lang="en">Logos can be used in a variety of contexts.
            Logo can be associated with an Organisation or a Service or a PublicationChannel.</rdfs:comment>
        <rdfs:range rdf:resource="&ebucore;Logo"/>
    </owl:ObjectProperty>
    


    <!-- http://www.ebu.ch/metadata/ontologies/ebucore/ebucore#hasMediaFragment -->

    <owl:ObjectProperty rdf:about="&ebucore;hasMediaFragment">
        <rdfs:label xml:lang="en">Part</rdfs:label>
        <rdfs:comment xml:lang="en">To define Parts (segments, fragments, etc.)
            withiin a MediaResource.</rdfs:comment>
        <rdfs:range rdf:resource="&ebucore;MediaFragment"/>
        <rdfs:subPropertyOf rdf:resource="&ebucore;hasRelatedResource"/>
        <rdfs:domain>
            <owl:Class>
                <owl:unionOf rdf:parseType="Collection">
                    <rdf:Description rdf:about="&ebucore;EditorialObject"/>
                    <rdf:Description rdf:about="&ebucore;MediaResource"/>
                </owl:unionOf>
            </owl:Class>
        </rdfs:domain>
    </owl:ObjectProperty>
    


    <!-- http://www.ebu.ch/metadata/ontologies/ebucore/ebucore#hasMember -->

    <owl:ObjectProperty rdf:about="&ebucore;hasMember">
        <rdfs:label xml:lang="en">Member.</rdfs:label>
        <rdfs:comment xml:lang="en">To establish group/collection relationship between EditorialObjects.</rdfs:comment>
        <rdfs:range rdf:resource="&ebucore;EditorialObject"/>
        <rdfs:domain rdf:resource="&ebucore;Group"/>
    </owl:ObjectProperty>
    


    <!-- http://www.ebu.ch/metadata/ontologies/ebucore/ebucore#hasMetadataAttributor -->

    <owl:ObjectProperty rdf:about="&ebucore;hasMetadataAttributor">
        <rdfs:label xml:lang="en">Metadata attributor</rdfs:label>
        <rdfs:comment xml:lang="en">To identify the Agent (Contact/person or
            Organisation) who has created the metadata.</rdfs:comment>
        <rdfs:range rdf:resource="&ebucore;Agent"/>
    </owl:ObjectProperty>
    


    <!-- http://www.ebu.ch/metadata/ontologies/ebucore/ebucore#hasPart -->

    <owl:ObjectProperty rdf:about="&ebucore;hasPart">
        <rdfs:label xml:lang="en">Part</rdfs:label>
        <rdfs:comment xml:lang="en">To define Parts (segments, fragments, etc.)
            within a BusinessObject.</rdfs:comment>
        <rdfs:domain rdf:resource="&ebucore;EditorialObject"/>
        <rdfs:range rdf:resource="&ebucore;EditorialObject"/>
        <rdfs:subPropertyOf rdf:resource="&ebucore;hasRelatedBusinessObject"/>
    </owl:ObjectProperty>
    


    <!-- http://www.ebu.ch/metadata/ontologies/ebucore/ebucore#hasPictogram -->

    <owl:ObjectProperty rdf:about="&ebucore;hasPictogram">
        <rdfs:label xml:lang="en">Pictogram</rdfs:label>
        <rdfs:comment xml:lang="en">To provide a visual representation of  TargetAudience or Rating.</rdfs:comment>
        <rdfs:range rdf:resource="&ebucore;Pictogram"/>
    </owl:ObjectProperty>
    


    <!-- http://www.ebu.ch/metadata/ontologies/ebucore/ebucore#hasPublicationChannel -->

    <owl:ObjectProperty rdf:about="&ebucore;hasPublicationChannel">
        <rdfs:label xml:lang="en">Publication channel</rdfs:label>
        <rdfs:comment xml:lang="en">To associate a PublicationEvent with a
            PublicationChannel.</rdfs:comment>
        <rdfs:range rdf:resource="&ebucore;PublicationChannel"/>
    </owl:ObjectProperty>
    


    <!-- http://www.ebu.ch/metadata/ontologies/ebucore/ebucore#hasPublicationEvent -->

    <owl:ObjectProperty rdf:about="&ebucore;hasPublicationEvent">
        <rdfs:label xml:lang="en">Publication event</rdfs:label>
        <rdfs:comment xml:lang="en">To associate PublicationEvents with
            PublicationChannels or as elements of a PublicationHistory or PublicationPlanning.</rdfs:comment>
        <rdfs:range rdf:resource="&ebucore;PublicationEvent"/>
    </owl:ObjectProperty>
    


    <!-- http://www.ebu.ch/metadata/ontologies/ebucore/ebucore#hasPublicationHistory -->

    <owl:ObjectProperty rdf:about="&ebucore;hasPublicationHistory">
        <rdfs:label rdf:datatype="&xsd;string">has publication history</rdfs:label>
        <rdfs:range rdf:resource="&ebucore;PublicationHistory"/>
    </owl:ObjectProperty>
    


    <!-- http://www.ebu.ch/metadata/ontologies/ebucore/ebucore#hasRating -->

    <owl:ObjectProperty rdf:about="&ebucore;hasRating">
        <rdfs:label xml:lang="en">Rating</rdfs:label>
        <rdfs:comment xml:lang="en">To identify the presence of Rating attributed
            to a Resource or BusinessObject.</rdfs:comment>
        <rdfs:range rdf:resource="&ebucore;Rating"/>
    </owl:ObjectProperty>
    


    <!-- http://www.ebu.ch/metadata/ontologies/ebucore/ebucore#hasRatingSource -->

    <owl:ObjectProperty rdf:about="&ebucore;hasRatingSource">
        <rdfs:label xml:lang="en">Rating provider</rdfs:label>
        <rdfs:comment xml:lang="en">To identify an Agent (Contact/person or
            Organisation) who has proposed a Rating.</rdfs:comment>
        <rdfs:range rdf:resource="&ebucore;Agent"/>
    </owl:ObjectProperty>
    


    <!-- http://www.ebu.ch/metadata/ontologies/ebucore/ebucore#hasRelatedAudioChannel -->

    <owl:ObjectProperty rdf:about="&ebucore;hasRelatedAudioChannel">
        <rdfs:label xml:lang="en">Audio channel</rdfs:label>
        <rdfs:comment xml:lang="en">To associate an AudioChannel with an AudioPack or an AudioStream.</rdfs:comment>
        <rdfs:range rdf:resource="&ebucore;AudioChannel"/>
        <rdfs:subPropertyOf rdf:resource="&ebucore;hasRelatedResource"/>
    </owl:ObjectProperty>
    


    <!-- http://www.ebu.ch/metadata/ontologies/ebucore/ebucore#hasRelatedAudioContent -->

    <owl:ObjectProperty rdf:about="&ebucore;hasRelatedAudioContent">
        <rdfs:label xml:lang="en">Audio content</rdfs:label>
        <rdfs:comment xml:lang="en">To identify the AudioContent associated with an AudioProgramme.</rdfs:comment>
        <rdfs:range rdf:resource="&ebucore;AudioContent"/>
        <rdfs:domain rdf:resource="&ebucore;AudioProgramme"/>
        <rdfs:subPropertyOf rdf:resource="&ebucore;hasRelatedBusinessObject"/>
    </owl:ObjectProperty>
    


    <!-- http://www.ebu.ch/metadata/ontologies/ebucore/ebucore#hasRelatedAudioObject -->

    <owl:ObjectProperty rdf:about="&ebucore;hasRelatedAudioObject">
        <rdfs:label xml:lang="en">Audio object</rdfs:label>
        <rdfs:comment xml:lang="en">To identify AudioObjects associated with AudioContent or other AudioObjects.</rdfs:comment>
        <rdfs:subPropertyOf rdf:resource="&ebucore;hasRelatedBusinessObject"/>
    </owl:ObjectProperty>
    


    <!-- http://www.ebu.ch/metadata/ontologies/ebucore/ebucore#hasRelatedAudioStream -->

    <owl:ObjectProperty rdf:about="&ebucore;hasRelatedAudioStream">
        <rdfs:label xml:lang="en">Audio stream</rdfs:label>
        <rdfs:comment xml:lang="en">To associate an AudioStream with an AudioTrack.</rdfs:comment>
        <rdfs:range rdf:resource="&ebucore;AudioStream"/>
    </owl:ObjectProperty>
    


    <!-- http://www.ebu.ch/metadata/ontologies/ebucore/ebucore#hasRelatedAudioTrack -->

    <owl:ObjectProperty rdf:about="&ebucore;hasRelatedAudioTrack">
        <rdfs:label xml:lang="en">Audio track</rdfs:label>
        <rdfs:comment xml:lang="en">To associate an AudioTrack with an AudioStream or an AudioTrackUID.</rdfs:comment>
        <rdfs:range rdf:resource="&ebucore;AudioTrack"/>
    </owl:ObjectProperty>
    


    <!-- http://www.ebu.ch/metadata/ontologies/ebucore/ebucore#hasRelatedBusinessObject -->

    <owl:ObjectProperty rdf:about="&ebucore;hasRelatedBusinessObject">
        <rdfs:label xml:lang="en">Editorial object</rdfs:label>
        <rdfs:comment xml:lang="en">EditorialObjects can be related to other BusinessOjects, Assets (and associated rights), PublicationEvents(defined when commissioning the EditorialObject before it is instantiated as a Resource (manifestation), or Resources, or Ratings.</rdfs:comment>
        <rdfs:subPropertyOf rdf:resource="&dc;relation"/>
        <rdfs:range rdf:resource="&ebucore;BusinessObject"/>
        <rdfs:domain>
            <owl:Class>
                <owl:unionOf rdf:parseType="Collection">
                    <rdf:Description rdf:about="&ebucore;Asset"/>
                    <rdf:Description rdf:about="&ebucore;BusinessObject"/>
                    <rdf:Description rdf:about="&ebucore;PublicationEvent"/>
                    <rdf:Description rdf:about="&ebucore;Rating"/>
                    <rdf:Description rdf:about="&ebucore;Resource"/>
                </owl:unionOf>
            </owl:Class>
        </rdfs:domain>
    </owl:ObjectProperty>
    


    <!-- http://www.ebu.ch/metadata/ontologies/ebucore/ebucore#hasRelatedEvent -->

    <owl:ObjectProperty rdf:about="&ebucore;hasRelatedEvent">
        <rdfs:label rdf:datatype="&xsd;string">has related event</rdfs:label>
        <rdfs:range rdf:resource="&ebucore;Event"/>
    </owl:ObjectProperty>
    


    <!-- http://www.ebu.ch/metadata/ontologies/ebucore/ebucore#hasRelatedImage -->

    <owl:ObjectProperty rdf:about="&ebucore;hasRelatedImage">
        <rdfs:label xml:lang="en">Image</rdfs:label>
        <rdfs:comment xml:lang="en">To associate an Image with a BusinessObject.</rdfs:comment>
        <rdfs:domain rdf:resource="&ebucore;BusinessObject"/>
        <rdfs:range rdf:resource="&ebucore;Image"/>
        <rdfs:subPropertyOf rdf:resource="&ebucore;hasRelatedBusinessObject"/>
    </owl:ObjectProperty>
    


    <!-- http://www.ebu.ch/metadata/ontologies/ebucore/ebucore#hasRelatedLocation -->

    <owl:ObjectProperty rdf:about="&ebucore;hasRelatedLocation">
        <rdfs:label rdf:datatype="&xsd;string">has related event</rdfs:label>
        <rdfs:subPropertyOf rdf:resource="&dc;relation"/>
        <rdfs:range rdf:resource="&ebucore;Location"/>
        <rdfs:domain>
            <owl:Class>
                <owl:unionOf rdf:parseType="Collection">
                    <rdf:Description rdf:about="&ebucore;BusinessObject"/>
                    <rdf:Description rdf:about="&ebucore;Resource"/>
                </owl:unionOf>
            </owl:Class>
        </rdfs:domain>
    </owl:ObjectProperty>
    


    <!-- http://www.ebu.ch/metadata/ontologies/ebucore/ebucore#hasRelatedMediaFragment -->

    <owl:ObjectProperty rdf:about="&ebucore;hasRelatedMediaFragment">
        <rdfs:label xml:lang="en">Media fragment</rdfs:label>
        <rdfs:comment xml:lang="en">To associate a Part of an EditorialObject with a MediaFragment within the association MediaResource instantiating the EditorialObject.</rdfs:comment>
        <rdfs:range rdf:resource="&ebucore;MediaFragment"/>
        <rdfs:domain rdf:resource="&ebucore;Part"/>
        <rdfs:subPropertyOf rdf:resource="&ebucore;hasMediaFragment"/>
    </owl:ObjectProperty>
    


    <!-- http://www.ebu.ch/metadata/ontologies/ebucore/ebucore#hasRelatedPicture -->

    <owl:ObjectProperty rdf:about="&ebucore;hasRelatedPicture">
        <rdfs:label xml:lang="en">Picture</rdfs:label>
        <rdfs:comment xml:lang="en">To associate a Picture with a BusinessObject or a Resource.</rdfs:comment>
        <rdfs:range rdf:resource="&ebucore;Picture"/>
    </owl:ObjectProperty>
    


    <!-- http://www.ebu.ch/metadata/ontologies/ebucore/ebucore#hasRelatedPublicationEvent -->

    <owl:ObjectProperty rdf:about="&ebucore;hasRelatedPublicationEvent">
        <rdfs:label xml:lang="en">Publication event</rdfs:label>
        <rdfs:comment xml:lang="en">To identify the PublicationEvent associated with a MediaResource (manifestation of an EditorialObject).</rdfs:comment>
        <rdfs:subPropertyOf rdf:resource="&dc;relation"/>
        <rdfs:domain rdf:resource="&ebucore;MediaResource"/>
        <rdfs:range rdf:resource="&ebucore;PublicationEvent"/>
    </owl:ObjectProperty>
    


    <!-- http://www.ebu.ch/metadata/ontologies/ebucore/ebucore#hasRelatedResource -->

    <owl:ObjectProperty rdf:about="&ebucore;hasRelatedResource">
        <rdfs:label rdf:datatype="&xsd;string">Related resource</rdfs:label>
        <rdfs:comment xml:lang="en">To identify a Resource associated with an Asset or a BusinessObject or a PublicationEvent or another Resource.</rdfs:comment>
        <rdfs:subPropertyOf rdf:resource="&dc;relation"/>
        <rdfs:range rdf:resource="&ebucore;Resource"/>
        <rdfs:domain>
            <owl:Class>
                <owl:unionOf rdf:parseType="Collection">
                    <rdf:Description rdf:about="&ebucore;Asset"/>
                    <rdf:Description rdf:about="&ebucore;BusinessObject"/>
                    <rdf:Description rdf:about="&ebucore;PublicationEvent"/>
                    <rdf:Description rdf:about="&ebucore;Rating"/>
                    <rdf:Description rdf:about="&ebucore;Resource"/>
                </owl:unionOf>
            </owl:Class>
        </rdfs:domain>
    </owl:ObjectProperty>
    


    <!-- http://www.ebu.ch/metadata/ontologies/ebucore/ebucore#hasRightsContact -->

    <owl:ObjectProperty rdf:about="&ebucore;hasRightsContact">
        <rdfs:label xml:lang="en">Contact</rdfs:label>
        <rdfs:comment xml:lang="en">To identify a Contact/person who can provide
            assistance / guidance regarding the associated Rights.</rdfs:comment>
        <rdfs:range rdf:resource="&ebucore;Contact"/>
    </owl:ObjectProperty>
    


    <!-- http://www.ebu.ch/metadata/ontologies/ebucore/ebucore#hasRightsHolder -->

    <owl:ObjectProperty rdf:about="&ebucore;hasRightsHolder">
        <rdfs:label xml:lang="en">Rights holder</rdfs:label>
        <rdfs:comment xml:lang="en">To identify an Agent (Contact/person or
            Organisation) having/managing Rights.</rdfs:comment>
        <rdfs:range rdf:resource="&ebucore;Agent"/>
    </owl:ObjectProperty>
    


    <!-- http://www.ebu.ch/metadata/ontologies/ebucore/ebucore#hasSeason -->

    <owl:ObjectProperty rdf:about="&ebucore;hasSeason">
        <rdfs:label xml:lang="en">Season</rdfs:label>
        <rdfs:comment xml:lang="en">The Season of a Series.</rdfs:comment>
        <rdfs:range rdf:resource="&ebucore;Season"/>
        <rdfs:domain rdf:resource="&ebucore;Series"/>
        <rdfs:subPropertyOf rdf:resource="&ebucore;hasRelatedBusinessObject"/>
    </owl:ObjectProperty>
    


    <!-- http://www.ebu.ch/metadata/ontologies/ebucore/ebucore#hasSigning -->

    <owl:ObjectProperty rdf:about="&ebucore;hasSigning">
        <rdfs:label xml:lang="en">Accessibility - signing</rdfs:label>
        <rdfs:comment xml:lang="en">To identify the presence of Signing associated
            to the BusinessObject/Resource.</rdfs:comment>
        <rdfs:range rdf:resource="&ebucore;Signing"/>
    </owl:ObjectProperty>
    


    <!-- http://www.ebu.ch/metadata/ontologies/ebucore/ebucore#hasSource -->

    <owl:ObjectProperty rdf:about="&ebucore;hasSource">
        <rdfs:label xml:lang="en">Source</rdfs:label>
        <rdfs:comment xml:lang="en">To identify a Resource as the source of another Resource.</rdfs:comment>
        <rdfs:range rdf:resource="&ebucore;Resource"/>
    </owl:ObjectProperty>
    


    <!-- http://www.ebu.ch/metadata/ontologies/ebucore/ebucore#hasStaff -->

    <owl:ObjectProperty rdf:about="&ebucore;hasStaff">
        <rdfs:label xml:lang="en">Staff</rdfs:label>
        <rdfs:comment xml:lang="en">To identify staff working within an Organisation.</rdfs:comment>
        <rdfs:range rdf:resource="&ebucore;Contact"/>
    </owl:ObjectProperty>
    


    <!-- http://www.ebu.ch/metadata/ontologies/ebucore/ebucore#hasSubtitling -->

    <owl:ObjectProperty rdf:about="&ebucore;hasSubtitling">
        <rdfs:label xml:lang="en">Subtitling</rdfs:label>
        <rdfs:comment xml:lang="en">To signal the presence of Subtitling associated
            with the EditorialObject or MediaResource.</rdfs:comment>
        <rdfs:range rdf:resource="&ebucore;Subtitling"/>
    </owl:ObjectProperty>
    


    <!-- http://www.ebu.ch/metadata/ontologies/ebucore/ebucore#hasTrack -->

    <owl:ObjectProperty rdf:about="&ebucore;hasTrack">
        <rdfs:label xml:lang="en">Track</rdfs:label>
        <rdfs:comment xml:lang="en">To associate audio/data/video tracks with a MediaResource.</rdfs:comment>
        <rdfs:range rdf:resource="&ebucore;Track"/>
    </owl:ObjectProperty>
    


    <!-- http://www.ebu.ch/metadata/ontologies/ebucore/ebucore#hasVersion -->

    <owl:ObjectProperty rdf:about="&ebucore;hasVersion">
        <rdfs:label xml:lang="en">Version</rdfs:label>
        <rdfs:comment xml:lang="en">To identify another version of an Asset, BusinessObject or Resource.</rdfs:comment>
        <rdfs:subPropertyOf rdf:resource="&dc;relation"/>
        <rdfs:range>
            <owl:Class>
                <owl:unionOf rdf:parseType="Collection">
                    <rdf:Description rdf:about="&ebucore;Asset"/>
                    <rdf:Description rdf:about="&ebucore;BusinessObject"/>
                    <rdf:Description rdf:about="&ebucore;Resource"/>
                </owl:unionOf>
            </owl:Class>
        </rdfs:range>
        <rdfs:domain>
            <owl:Class>
                <owl:unionOf rdf:parseType="Collection">
                    <rdf:Description rdf:about="&ebucore;Asset"/>
                    <rdf:Description rdf:about="&ebucore;BusinessObject"/>
                    <rdf:Description rdf:about="&ebucore;Resource"/>
                </owl:unionOf>
            </owl:Class>
        </rdfs:domain>
    </owl:ObjectProperty>
    


    <!-- http://www.ebu.ch/metadata/ontologies/ebucore/ebucore#holdsRightsOver -->

    <owl:ObjectProperty rdf:about="&ebucore;holdsRightsOver">
        <rdfs:label xml:lang="en">Asset, resource, object</rdfs:label>
        <rdfs:comment xml:lang="en">To identify a BusinessObject or Resource on
            which an Agent (Contact/person or Organisation) holds Rights.</rdfs:comment>
        <rdfs:range>
            <owl:Class>
                <owl:unionOf rdf:parseType="Collection">
                    <rdf:Description rdf:about="&ebucore;Asset"/>
                    <rdf:Description rdf:about="&ebucore;BusinessObject"/>
                    <rdf:Description rdf:about="&ebucore;Resource"/>
                </owl:unionOf>
            </owl:Class>
        </rdfs:range>
    </owl:ObjectProperty>
    


    <!-- http://www.ebu.ch/metadata/ontologies/ebucore/ebucore#instantiates -->

    <owl:ObjectProperty rdf:about="&ebucore;instantiates">
        <rdfs:label xml:lang="en">Business object</rdfs:label>
        <rdfs:comment xml:lang="en">To link a particular manifestation of a
            BusinessObject to the corresponding Resource.</rdfs:comment>
        <rdfs:range rdf:resource="&ebucore;BusinessObject"/>
        <rdfs:domain rdf:resource="&ebucore;Resource"/>
        <rdfs:subPropertyOf rdf:resource="&ebucore;hasRelatedBusinessObject"/>
    </owl:ObjectProperty>
    


    <!-- http://www.ebu.ch/metadata/ontologies/ebucore/ebucore#isAgent -->

    <owl:ObjectProperty rdf:about="&ebucore;isAgent">
        <rdfs:label xml:lang="en">Agent</rdfs:label>
        <rdfs:comment xml:lang="en">To identify a Contact/person or Organisation as part of a cast list.</rdfs:comment>
        <rdfs:range>
            <owl:Class>
                <owl:unionOf rdf:parseType="Collection">
                    <rdf:Description rdf:about="&ebucore;Contact"/>
                    <rdf:Description rdf:about="&ebucore;Organisation"/>
                </owl:unionOf>
            </owl:Class>
        </rdfs:range>
    </owl:ObjectProperty>
    


    <!-- http://www.ebu.ch/metadata/ontologies/ebucore/ebucore#isCharacter -->

    <owl:ObjectProperty rdf:about="&ebucore;isCharacter">
        <rdfs:label xml:lang="en">Character</rdfs:label>
        <rdfs:comment xml:lang="en">To identify the character personified by a Cast individual.</rdfs:comment>
        <rdfs:range rdf:resource="&ebucore;Character"/>
    </owl:ObjectProperty>
    


    <!-- http://www.ebu.ch/metadata/ontologies/ebucore/ebucore#isEpisodeOf -->

    <owl:ObjectProperty rdf:about="&ebucore;isEpisodeOf">
        <rdfs:label xml:lang="en">Parent season</rdfs:label>
        <rdfs:comment xml:lang="en">The Episode of a Series or a Season.</rdfs:comment>
        <rdfs:domain rdf:resource="&ebucore;Programme"/>
        <rdfs:subPropertyOf rdf:resource="&ebucore;hasRelatedBusinessObject"/>
        <rdfs:range>
            <owl:Class>
                <owl:unionOf rdf:parseType="Collection">
                    <rdf:Description rdf:about="&ebucore;Season"/>
                    <rdf:Description rdf:about="&ebucore;Series"/>
                </owl:unionOf>
            </owl:Class>
        </rdfs:range>
    </owl:ObjectProperty>
    


    <!-- http://www.ebu.ch/metadata/ontologies/ebucore/ebucore#isFictitiousContact -->

    <owl:ObjectProperty rdf:about="&ebucore;isFictitiousContact">
        <rdfs:label xml:lang="en">Fictitious contact</rdfs:label>
        <rdfs:comment xml:lang="en">To identify Contact/persons being fictitious.</rdfs:comment>
        <rdfs:range rdf:resource="&ebucore;Contact"/>
    </owl:ObjectProperty>
    


    <!-- http://www.ebu.ch/metadata/ontologies/ebucore/ebucore#isMediaFragmentOf -->

    <owl:ObjectProperty rdf:about="&ebucore;isMediaFragmentOf">
        <rdfs:label xml:lang="en">Source</rdfs:label>
        <rdfs:comment xml:lang="en">To identify the MediaResource to which the MediaFragment belongs to.</rdfs:comment>
        <rdfs:domain rdf:resource="&ebucore;MediaFragment"/>
        <rdfs:range rdf:resource="&ebucore;MediaResource"/>
        <owl:inverseOf rdf:resource="&ebucore;hasMediaFragment"/>
        <rdfs:subPropertyOf rdf:resource="&ebucore;hasRelatedResource"/>
    </owl:ObjectProperty>
    


    <!-- http://www.ebu.ch/metadata/ontologies/ebucore/ebucore#isMemberOf -->

    <owl:ObjectProperty rdf:about="&ebucore;isMemberOf">
        <rdfs:label xml:lang="en">Member of</rdfs:label>
        <rdfs:comment xml:lang="en">To identify a Group to which an EidtorialObject is a member of.</rdfs:comment>
        <rdfs:subPropertyOf rdf:resource="&dc;relation"/>
        <rdfs:domain rdf:resource="&ebucore;EditorialObject"/>
        <rdfs:range rdf:resource="&ebucore;Group"/>
        <owl:inverseOf rdf:resource="&ebucore;hasMember"/>
    </owl:ObjectProperty>
    


    <!-- http://www.ebu.ch/metadata/ontologies/ebucore/ebucore#isNextInSequence -->

    <owl:ObjectProperty rdf:about="&ebucore;isNextInSequence">
        <rdfs:label rdf:datatype="&xsd;string">Next</rdfs:label>
        <rdfs:comment rdf:datatype="&xsd;string">A link to a an BusinessObject or a Resource following the current BusinessObject or Resource in an ordered sequence</rdfs:comment>
        <rdfs:range>
            <owl:Class>
                <owl:unionOf rdf:parseType="Collection">
                    <rdf:Description rdf:about="&ebucore;BusinessObject"/>
                    <rdf:Description rdf:about="&ebucore;Resource"/>
                </owl:unionOf>
            </owl:Class>
        </rdfs:range>
    </owl:ObjectProperty>
    


    <!-- http://www.ebu.ch/metadata/ontologies/ebucore/ebucore#isOperatedBy -->

    <owl:ObjectProperty rdf:about="&ebucore;isOperatedBy">
        <rdfs:label xml:lang="en">Operator, owner</rdfs:label>
        <rdfs:comment xml:lang="en">To identify the Service that operates the
            PublicationChannel.</rdfs:comment>
        <rdfs:subPropertyOf rdf:resource="&dc;relation"/>
        <rdfs:domain rdf:resource="&ebucore;PublicationChannel"/>
        <rdfs:range rdf:resource="&ebucore;Service"/>
    </owl:ObjectProperty>
    


    <!-- http://www.ebu.ch/metadata/ontologies/ebucore/ebucore#isOwnedBy -->

    <owl:ObjectProperty rdf:about="&ebucore;isOwnedBy">
        <rdfs:label xml:lang="en">Owner</rdfs:label>
        <rdfs:comment xml:lang="en">To identify the Agent (Contact/person or
            Organisation) who owns a Service operating a PublicationChannel.</rdfs:comment>
        <rdfs:subPropertyOf rdf:resource="&dc;relation"/>
        <rdfs:range rdf:resource="&ebucore;Agent"/>
        <rdfs:domain rdf:resource="&ebucore;Service"/>
    </owl:ObjectProperty>
    


    <!-- http://www.ebu.ch/metadata/ontologies/ebucore/ebucore#isReferencedBy -->

    <owl:ObjectProperty rdf:about="&ebucore;isReferencedBy">
        <rdfs:label xml:lang="en">Related object, resource</rdfs:label>
        <rdfs:comment xml:lang="en">To express references across Assets, BusinessObjects or Resources.</rdfs:comment>
        <rdfs:range>
            <owl:Class>
                <owl:unionOf rdf:parseType="Collection">
                    <rdf:Description rdf:about="&ebucore;Asset"/>
                    <rdf:Description rdf:about="&ebucore;BusinessObject"/>
                    <rdf:Description rdf:about="&ebucore;Resource"/>
                </owl:unionOf>
            </owl:Class>
        </rdfs:range>
    </owl:ObjectProperty>
    


    <!-- http://www.ebu.ch/metadata/ontologies/ebucore/ebucore#isRelatedTo -->

    <owl:ObjectProperty rdf:about="&ebucore;isRelatedTo">
        <rdfs:label xml:lang="en">Related to</rdfs:label>
        <rdfs:comment xml:lang="en">To establish relationships between Assets,
            BusinessObjects, PublicationEvents, Ratings and Resources.</rdfs:comment>
        <rdfs:subPropertyOf rdf:resource="&dc;relation"/>
        <rdfs:domain>
            <owl:Class>
                <owl:unionOf rdf:parseType="Collection">
                    <rdf:Description rdf:about="&ebucore;Asset"/>
                    <rdf:Description rdf:about="&ebucore;BusinessObject"/>
                    <rdf:Description rdf:about="&ebucore;PublicationEvent"/>
                    <rdf:Description rdf:about="&ebucore;Rating"/>
                    <rdf:Description rdf:about="&ebucore;Resource"/>
                </owl:unionOf>
            </owl:Class>
        </rdfs:domain>
        <rdfs:range>
            <owl:Class>
                <owl:unionOf rdf:parseType="Collection">
                    <rdf:Description rdf:about="&ebucore;Asset"/>
                    <rdf:Description rdf:about="&ebucore;BusinessObject"/>
                    <rdf:Description rdf:about="&ebucore;PublicationEvent"/>
                    <rdf:Description rdf:about="&ebucore;Rating"/>
                    <rdf:Description rdf:about="&ebucore;Resource"/>
                </owl:unionOf>
            </owl:Class>
        </rdfs:range>
    </owl:ObjectProperty>
    


    <!-- http://www.ebu.ch/metadata/ontologies/ebucore/ebucore#isReplacedBy -->

    <owl:ObjectProperty rdf:about="&ebucore;isReplacedBy">
        <rdfs:label xml:lang="en">Replacement</rdfs:label>
        <rdfs:comment xml:lang="en">To identify substitutions.</rdfs:comment>
        <rdfs:subPropertyOf rdf:resource="&dc;relation"/>
        <rdfs:domain>
            <owl:Class>
                <owl:unionOf rdf:parseType="Collection">
                    <rdf:Description rdf:about="&ebucore;Asset"/>
                    <rdf:Description rdf:about="&ebucore;BusinessObject"/>
                    <rdf:Description rdf:about="&ebucore;Resource"/>
                </owl:unionOf>
            </owl:Class>
        </rdfs:domain>
        <rdfs:range>
            <owl:Class>
                <owl:unionOf rdf:parseType="Collection">
                    <rdf:Description rdf:about="&ebucore;Asset"/>
                    <rdf:Description rdf:about="&ebucore;BusinessObject"/>
                    <rdf:Description rdf:about="&ebucore;Resource"/>
                </owl:unionOf>
            </owl:Class>
        </rdfs:range>
    </owl:ObjectProperty>
    


    <!-- http://www.ebu.ch/metadata/ontologies/ebucore/ebucore#isRequiredBy -->

    <owl:ObjectProperty rdf:about="&ebucore;isRequiredBy">
        <rdfs:label xml:lang="en">Required</rdfs:label>
        <rdfs:comment xml:lang="en">To express strong relations between Assets, BusinessObjects or Resources.</rdfs:comment>
        <rdfs:subPropertyOf rdf:resource="&dc;relation"/>
        <rdfs:domain>
            <owl:Class>
                <owl:unionOf rdf:parseType="Collection">
                    <rdf:Description rdf:about="&ebucore;Asset"/>
                    <rdf:Description rdf:about="&ebucore;BusinessObject"/>
                    <rdf:Description rdf:about="&ebucore;Resource"/>
                </owl:unionOf>
            </owl:Class>
        </rdfs:domain>
        <rdfs:range>
            <owl:Class>
                <owl:unionOf rdf:parseType="Collection">
                    <rdf:Description rdf:about="&ebucore;Asset"/>
                    <rdf:Description rdf:about="&ebucore;BusinessObject"/>
                    <rdf:Description rdf:about="&ebucore;Resource"/>
                </owl:unionOf>
            </owl:Class>
        </rdfs:range>
    </owl:ObjectProperty>
    


    <!-- http://www.ebu.ch/metadata/ontologies/ebucore/ebucore#isSeasonOf -->

    <owl:ObjectProperty rdf:about="&ebucore;isSeasonOf">
        <rdfs:label xml:lang="en">Parent Series</rdfs:label>
        <rdfs:comment xml:lang="en">The Season of a Series.</rdfs:comment>
        <rdfs:domain rdf:resource="&ebucore;Season"/>
        <rdfs:range rdf:resource="&ebucore;Series"/>
        <rdfs:subPropertyOf rdf:resource="&ebucore;hasRelatedBusinessObject"/>
        <owl:inverseOf rdf:resource="&ebucore;hasSeason"/>
    </owl:ObjectProperty>
    


    <!-- http://www.ebu.ch/metadata/ontologies/ebucore/ebucore#isVersionOf -->

    <owl:ObjectProperty rdf:about="&ebucore;isVersionOf">
        <rdfs:label xml:lang="en">Version of</rdfs:label>
        <rdfs:comment xml:lang="en">To identify related versions.</rdfs:comment>
        <rdfs:subPropertyOf rdf:resource="&dc;relation"/>
        <owl:inverseOf rdf:resource="&ebucore;hasVersion"/>
        <rdfs:range>
            <owl:Class>
                <owl:unionOf rdf:parseType="Collection">
                    <rdf:Description rdf:about="&ebucore;Asset"/>
                    <rdf:Description rdf:about="&ebucore;BusinessObject"/>
                    <rdf:Description rdf:about="&ebucore;Resource"/>
                </owl:unionOf>
            </owl:Class>
        </rdfs:range>
        <rdfs:domain>
            <owl:Class>
                <owl:unionOf rdf:parseType="Collection">
                    <rdf:Description rdf:about="&ebucore;Asset"/>
                    <rdf:Description rdf:about="&ebucore;BusinessObject"/>
                    <rdf:Description rdf:about="&ebucore;Resource"/>
                </owl:unionOf>
            </owl:Class>
        </rdfs:domain>
    </owl:ObjectProperty>
    


    <!-- http://www.ebu.ch/metadata/ontologies/ebucore/ebucore#owns -->

    <owl:ObjectProperty rdf:about="&ebucore;owns">
        <rdfs:label xml:lang="en">Owns</rdfs:label>
        <rdfs:comment xml:lang="en">To identify the service (s) that an Agent
            (Contact/person or Organisation) owns.</rdfs:comment>
        <rdfs:subPropertyOf rdf:resource="&dc;relation"/>
        <rdfs:domain rdf:resource="&ebucore;Agent"/>
        <rdfs:range rdf:resource="&ebucore;Service"/>
        <owl:inverseOf rdf:resource="&ebucore;isOwnedBy"/>
    </owl:ObjectProperty>
    


    <!-- http://www.ebu.ch/metadata/ontologies/ebucore/ebucore#references -->

    <owl:ObjectProperty rdf:about="&ebucore;references">
        <rdfs:label xml:lang="en">References</rdfs:label>
        <rdfs:comment xml:lang="en">To express a reference between Assets, BusinessObjects or Resources.</rdfs:comment>
        <rdfs:range>
            <owl:Class>
                <owl:unionOf rdf:parseType="Collection">
                    <rdf:Description rdf:about="&ebucore;Asset"/>
                    <rdf:Description rdf:about="&ebucore;BusinessObject"/>
                    <rdf:Description rdf:about="&ebucore;Resource"/>
                </owl:unionOf>
            </owl:Class>
        </rdfs:range>
    </owl:ObjectProperty>
    


    <!-- http://www.ebu.ch/metadata/ontologies/ebucore/ebucore#replaces -->

    <owl:ObjectProperty rdf:about="&ebucore;replaces">
        <rdfs:label xml:lang="en">Replaces</rdfs:label>
        <rdfs:comment xml:lang="en">To identify substitution.</rdfs:comment>
        <rdfs:range>
            <owl:Class>
                <owl:unionOf rdf:parseType="Collection">
                    <rdf:Description rdf:about="&ebucore;Asset"/>
                    <rdf:Description rdf:about="&ebucore;BusinessObject"/>
                    <rdf:Description rdf:about="&ebucore;Resource"/>
                </owl:unionOf>
            </owl:Class>
        </rdfs:range>
    </owl:ObjectProperty>
    


    <!-- http://www.ebu.ch/metadata/ontologies/ebucore/ebucore#requires -->

    <owl:ObjectProperty rdf:about="&ebucore;requires">
        <rdfs:label xml:lang="en">Requires</rdfs:label>
        <rdfs:comment xml:lang="en">To express dependency.</rdfs:comment>
        <rdfs:range>
            <owl:Class>
                <owl:unionOf rdf:parseType="Collection">
                    <rdf:Description rdf:about="&ebucore;Asset"/>
                    <rdf:Description rdf:about="&ebucore;BusinessObject"/>
                    <rdf:Description rdf:about="&ebucore;Resource"/>
                </owl:unionOf>
            </owl:Class>
        </rdfs:range>
    </owl:ObjectProperty>
    


    <!-- http://xmlns.com/foaf/0.1/member -->

    <owl:ObjectProperty rdf:about="&foaf;member">
        <rdfs:label xml:lang="en">Group member</rdfs:label>
        <rdfs:comment xml:lang="en">To identify an Agent member of a Group.</rdfs:comment>
        <rdfs:range rdf:resource="&foaf;Agent"/>
    </owl:ObjectProperty>
    


    <!-- 
    ///////////////////////////////////////////////////////////////////////////////////////
    //
    // Data properties
    //
    ///////////////////////////////////////////////////////////////////////////////////////
     -->

    


    <!-- http://purl.org/dc/elements/1.1/alternative -->

    <owl:DatatypeProperty rdf:about="&dc;alternative">
        <rdfs:label xml:lang="en">Alternative title</rdfs:label>
        <rdfs:comment xml:lang="en">An alternative to the title.</rdfs:comment>
        <rdfs:range rdf:resource="&xsd;string"/>
    </owl:DatatypeProperty>
    


    <!-- http://purl.org/dc/elements/1.1/date -->

    <owl:DatatypeProperty rdf:about="&dc;date">
        <rdfs:label xml:lang="en">date</rdfs:label>
        <rdfs:comment xml:lang="en">A date associated with the BusinessObject, Resource or Contact/Person.</rdfs:comment>
        <rdfs:range rdf:resource="&xsd;date"/>
    </owl:DatatypeProperty>
    


    <!-- http://purl.org/dc/elements/1.1/identifier -->

    <owl:DatatypeProperty rdf:about="&dc;identifier">
        <rdfs:label xml:lang="en">identifier</rdfs:label>
        <rdfs:comment xml:lang="en">An identifier associated with a BusinessObject or a resource.</rdfs:comment>
        <rdfs:range rdf:resource="&xsd;anyURI"/>
    </owl:DatatypeProperty>
    


    <!-- http://www.ebu.ch/metadata/ontologies/ebucore/ebucore#AffiliationEndDate -->

    <owl:DatatypeProperty rdf:about="&ebucore;AffiliationEndDate">
        <rdfs:label xml:lang="en">Affiliation start date</rdfs:label>
        <rdfs:comment xml:lang="en">The date when a Contact left an Organisation</rdfs:comment>
        <rdfs:range rdf:resource="&xsd;date"/>
    </owl:DatatypeProperty>
    


    <!-- http://www.ebu.ch/metadata/ontologies/ebucore/ebucore#AffiliationStartDate -->

    <owl:DatatypeProperty rdf:about="&ebucore;AffiliationStartDate">
        <rdfs:label rdf:datatype="&xsd;string">Affiliation start date</rdfs:label>
        <rdfs:range rdf:resource="&xsd;date"/>
    </owl:DatatypeProperty>
    


    <!-- http://www.ebu.ch/metadata/ontologies/ebucore/ebucore#DID -->

    <owl:DatatypeProperty rdf:about="&ebucore;DID">
        <rdfs:label xml:lang="en">DID</rdfs:label>
        <rdfs:comment xml:lang="en">The Data Identifier word (along with the SDID,
            if used), indicates the type of ancillary data that the packet corresponds
            to.</rdfs:comment>
        <rdfs:range rdf:resource="&xsd;integer"/>
    </owl:DatatypeProperty>
    


    <!-- http://www.ebu.ch/metadata/ontologies/ebucore/ebucore#SDID -->

    <owl:DatatypeProperty rdf:about="&ebucore;SDID">
        <rdfs:label xml:lang="en">SDID</rdfs:label>
        <rdfs:comment xml:lang="en">Secondary data identification word for
            ancillary data. Send mode identifier. An identifier which indicates the transmission
            timing for closed caption data.</rdfs:comment>
        <rdfs:range rdf:resource="&xsd;integer"/>
    </owl:DatatypeProperty>
    


    <!-- http://www.ebu.ch/metadata/ontologies/ebucore/ebucore#absoluteDistance -->

    <owl:DatatypeProperty rdf:about="&ebucore;absoluteDistance">
        <rdfs:label xml:lang="en">Absolute distance (in meters)</rdfs:label>
        <rdfs:comment xml:lang="en">To express an absolute distance in meters.</rdfs:comment>
        <rdfs:range rdf:resource="&xsd;float"/>
    </owl:DatatypeProperty>
    


    <!-- http://www.ebu.ch/metadata/ontologies/ebucore/ebucore#adultContent -->

    <owl:DatatypeProperty rdf:about="&ebucore;adultContent">
        <rdfs:label rdf:datatype="&xsd;string">adult content</rdfs:label>
        <rdfs:range rdf:resource="&xsd;boolean"/>
    </owl:DatatypeProperty>
    


    <!-- http://www.ebu.ch/metadata/ontologies/ebucore/ebucore#agentAddress -->

    <owl:DatatypeProperty rdf:about="&ebucore;agentAddress">
        <rdfs:label xml:lang="en">Address</rdfs:label>
        <rdfs:comment xml:lang="en">To provide the address of an Agent
            (Contact/person or organisation).</rdfs:comment>
        <rdfs:range rdf:resource="&xsd;string"/>
    </owl:DatatypeProperty>
    


    <!-- http://www.ebu.ch/metadata/ontologies/ebucore/ebucore#agentAge -->

    <owl:DatatypeProperty rdf:about="&ebucore;agentAge">
        <rdfs:label xml:lang="en">Age</rdfs:label>
        <rdfs:comment rdf:datatype="&xsd;string">The age of a Contact/Person</rdfs:comment>
        <rdfs:range rdf:resource="&xsd;integer"/>
    </owl:DatatypeProperty>
    


    <!-- http://www.ebu.ch/metadata/ontologies/ebucore/ebucore#agentEmailAddress -->

    <owl:DatatypeProperty rdf:about="&ebucore;agentEmailAddress">
        <rdfs:label xml:lang="en">Email</rdfs:label>
        <rdfs:comment xml:lang="en">To provide the email address of an agent
            (Contact/person or organisation).</rdfs:comment>
        <rdfs:range rdf:resource="&xsd;string"/>
    </owl:DatatypeProperty>
    


    <!-- http://www.ebu.ch/metadata/ontologies/ebucore/ebucore#agentMobileTelephoneNumber -->

    <owl:DatatypeProperty rdf:about="&ebucore;agentMobileTelephoneNumber">
        <rdfs:label xml:lang="en">Mobile</rdfs:label>
        <rdfs:comment xml:lang="en">To provide the mobile telephone number of an
            Agent (Contact/person or organisation)</rdfs:comment>
        <rdfs:range rdf:resource="&xsd;string"/>
    </owl:DatatypeProperty>
    


    <!-- http://www.ebu.ch/metadata/ontologies/ebucore/ebucore#agentName -->

    <owl:DatatypeProperty rdf:about="&ebucore;agentName">
        <rdfs:label xml:lang="en">Name</rdfs:label>
        <rdfs:comment xml:lang="en">To provide the full name of Contact/person - family and given name.</rdfs:comment>
        <rdfs:range rdf:resource="&xsd;string"/>
    </owl:DatatypeProperty>
    


    <!-- http://www.ebu.ch/metadata/ontologies/ebucore/ebucore#agentNickname -->

    <owl:DatatypeProperty rdf:about="&ebucore;agentNickname">
        <rdfs:label xml:lang="en">Nickname</rdfs:label>
        <rdfs:comment xml:lang="en">To provide a nickname of a Contact/person.</rdfs:comment>
        <rdfs:range rdf:resource="&xsd;string"/>
    </owl:DatatypeProperty>
    


    <!-- http://www.ebu.ch/metadata/ontologies/ebucore/ebucore#agentTelephoneNumber -->

    <owl:DatatypeProperty rdf:about="&ebucore;agentTelephoneNumber">
        <rdfs:label xml:lang="en">Telephone</rdfs:label>
        <rdfs:comment xml:lang="en">To provide the telephone number of an Agent
            (Contact/person or Organisation).</rdfs:comment>
        <rdfs:range rdf:resource="&xsd;string"/>
    </owl:DatatypeProperty>
    


    <!-- http://www.ebu.ch/metadata/ontologies/ebucore/ebucore#agentWebHomepage -->

    <owl:DatatypeProperty rdf:about="&ebucore;agentWebHomepage">
        <rdfs:label xml:lang="en">Homepage</rdfs:label>
        <rdfs:comment xml:lang="en">To provide the address of the webpage of an
            Agent (Contact/person or Organisation).</rdfs:comment>
        <rdfs:range rdf:resource="&xsd;anyURI"/>
    </owl:DatatypeProperty>
    


    <!-- http://www.ebu.ch/metadata/ontologies/ebucore/ebucore#aspectRatio -->

    <owl:DatatypeProperty rdf:about="&ebucore;aspectRatio">
        <rdfs:label xml:lang="en">Aspect ratio</rdfs:label>
        <rdfs:comment xml:lang="en">To provide the aspect ratio of a video frame or
            image. Several types of different aspect ration can apply to the same video image. If
            necessary, specialised aspect ratios can be defined as subproperties.</rdfs:comment>
        <rdfs:range rdf:resource="&xsd;string"/>
    </owl:DatatypeProperty>
    


    <!-- http://www.ebu.ch/metadata/ontologies/ebucore/ebucore#audioChannelNumber -->

    <owl:DatatypeProperty rdf:about="&ebucore;audioChannelNumber">
        <rdfs:label xml:lang="en">Audio channel number</rdfs:label>
        <rdfs:comment xml:lang="en">The total number of audio channels contained in
            the MediaResource.</rdfs:comment>
        <rdfs:range rdf:resource="&xsd;nonNegativeInteger"/>
    </owl:DatatypeProperty>
    


    <!-- http://www.ebu.ch/metadata/ontologies/ebucore/ebucore#audioMXFLookup -->

    <owl:DatatypeProperty rdf:about="&ebucore;audioMXFLookup">
        <rdfs:label xml:lang="en">Audio MXFlookup</rdfs:label>
        <rdfs:comment xml:lang="en">The parameters for MXF mapping.</rdfs:comment>
        <rdfs:range rdf:resource="&rdfs;Literal"/>
    </owl:DatatypeProperty>
    


    <!-- http://www.ebu.ch/metadata/ontologies/ebucore/ebucore#audioTrackConfiguration -->

    <owl:DatatypeProperty rdf:about="&ebucore;audioTrackConfiguration">
        <rdfs:label rdf:datatype="&xsd;string">Audio track configuration</rdfs:label>
        <rdfs:comment xml:lang="en">To provide the configuration of an audio track
            (e.g. stereo pair) in a MediaResource.</rdfs:comment>
        <rdfs:range rdf:resource="&xsd;string"/>
    </owl:DatatypeProperty>
    


    <!-- http://www.ebu.ch/metadata/ontologies/ebucore/ebucore#bitDepth -->

    <owl:DatatypeProperty rdf:about="&ebucore;bitDepth">
        <rdfs:label xml:lang="en">Bit depth</rdfs:label>
        <rdfs:comment xml:lang="en">To provide the audio encoding bit depth. Also called sample size.</rdfs:comment>
        <rdfs:range rdf:resource="&xsd;integer"/>
    </owl:DatatypeProperty>
    


    <!-- http://www.ebu.ch/metadata/ontologies/ebucore/ebucore#bitRate -->

    <owl:DatatypeProperty rdf:about="&ebucore;bitRate">
        <rdfs:label rdf:datatype="&xsd;string">Bitrate</rdfs:label>
        <rdfs:comment xml:lang="en">To provide the bitrate at which the
            MediaResource can be played in bits/second. Current bitrate if constant, and average bitrate if variable.</rdfs:comment>
        <rdfs:range rdf:resource="&xsd;nonNegativeInteger"/>
    </owl:DatatypeProperty>
    


    <!-- http://www.ebu.ch/metadata/ontologies/ebucore/ebucore#bitRateMax -->

    <owl:DatatypeProperty rdf:about="&ebucore;bitRateMax">
        <rdfs:label xml:lang="en">Maximum bitrate</rdfs:label>
        <rdfs:comment xml:lang="en">The maximum bitrate when variable, in bits per second.</rdfs:comment>
        <rdfs:range rdf:resource="&xsd;integer"/>
    </owl:DatatypeProperty>
    


    <!-- http://www.ebu.ch/metadata/ontologies/ebucore/ebucore#bitRateMode -->

    <owl:DatatypeProperty rdf:about="&ebucore;bitRateMode">
        <rdfs:label xml:lang="en">Bitrate mode</rdfs:label>
        <rdfs:comment xml:lang="en">A flag to indicate if the bit rate is fixed or
            variable.</rdfs:comment>
        <rdfs:range rdf:resource="&xsd;string"/>
    </owl:DatatypeProperty>
    


    <!-- http://www.ebu.ch/metadata/ontologies/ebucore/ebucore#businessObjectName -->

    <owl:DatatypeProperty rdf:about="&ebucore;businessObjectName">
        <rdfs:label xml:lang="en">Name</rdfs:label>
        <rdfs:comment xml:lang="en">A name attributed to a
            BusinessObject.</rdfs:comment>
        <rdfs:range rdf:resource="&xsd;string"/>
    </owl:DatatypeProperty>
    


    <!-- http://www.ebu.ch/metadata/ontologies/ebucore/ebucore#captioningSource -->

    <owl:DatatypeProperty rdf:about="&ebucore;captioningSource">
        <rdfs:label xml:lang="en">Captioning source</rdfs:label>
        <rdfs:comment xml:lang="en">To provide information on the source of a
            captioning file.</rdfs:comment>
        <rdfs:range rdf:resource="&xsd;string"/>
    </owl:DatatypeProperty>
    


    <!-- http://www.ebu.ch/metadata/ontologies/ebucore/ebucore#codecFamily -->

    <owl:DatatypeProperty rdf:about="&ebucore;codecFamily">
        <rdfs:label xml:lang="en">Codec family</rdfs:label>
        <rdfs:comment xml:lang="en">To provide information on the product family of the Codec.</rdfs:comment>
        <rdfs:range rdf:resource="&xsd;string"/>
    </owl:DatatypeProperty>
    


    <!-- http://www.ebu.ch/metadata/ontologies/ebucore/ebucore#codecName -->

    <owl:DatatypeProperty rdf:about="&ebucore;codecName">
        <rdfs:label xml:lang="en">Codec name</rdfs:label>
        <rdfs:comment xml:lang="en">To provide a name for the Codec, e.g. a product name.</rdfs:comment>
        <rdfs:range rdf:resource="&xsd;string"/>
    </owl:DatatypeProperty>
    


    <!-- http://www.ebu.ch/metadata/ontologies/ebucore/ebucore#codecVendor -->

    <owl:DatatypeProperty rdf:about="&ebucore;codecVendor">
        <rdfs:label xml:lang="en">Codec vendor</rdfs:label>
        <rdfs:comment xml:lang="en">To provide a name for the vendor of the Codec.</rdfs:comment>
        <rdfs:range rdf:resource="&xsd;string"/>
    </owl:DatatypeProperty>
    


    <!-- http://www.ebu.ch/metadata/ontologies/ebucore/ebucore#codecVersion -->

    <owl:DatatypeProperty rdf:about="&ebucore;codecVersion">
        <rdfs:label xml:lang="en">Codec version</rdfs:label>
        <rdfs:comment xml:lang="en">To provide information on the version of the Codec.</rdfs:comment>
        <rdfs:range rdf:resource="&xsd;string"/>
    </owl:DatatypeProperty>
    


    <!-- http://www.ebu.ch/metadata/ontologies/ebucore/ebucore#contactEducation -->

    <owl:DatatypeProperty rdf:about="&ebucore;contactEducation">
        <rdfs:label xml:lang="en">Education</rdfs:label>
        <rdfs:comment xml:lang="en">The education details of a Contact /
            person.</rdfs:comment>
        <rdfs:range rdf:resource="&xsd;string"/>
    </owl:DatatypeProperty>
    


    <!-- http://www.ebu.ch/metadata/ontologies/ebucore/ebucore#contactFamilyInformation -->

    <owl:DatatypeProperty rdf:about="&ebucore;contactFamilyInformation">
        <rdfs:label xml:lang="en">Family information</rdfs:label>
        <rdfs:comment xml:lang="en">Information on the family of a Contact /
            person.</rdfs:comment>
        <rdfs:range rdf:resource="&xsd;string"/>
    </owl:DatatypeProperty>
    


    <!-- http://www.ebu.ch/metadata/ontologies/ebucore/ebucore#contactHobbies -->

    <owl:DatatypeProperty rdf:about="&ebucore;contactHobbies">
        <rdfs:label xml:lang="en">Hobbies</rdfs:label>
        <rdfs:comment xml:lang="en">The hobbies of a Contact /
            person.</rdfs:comment>
        <rdfs:range rdf:resource="&xsd;string"/>
    </owl:DatatypeProperty>
    


    <!-- http://www.ebu.ch/metadata/ontologies/ebucore/ebucore#contactMaritalStatus -->

    <owl:DatatypeProperty rdf:about="&ebucore;contactMaritalStatus">
        <rdfs:label xml:lang="en">Marital status</rdfs:label>
        <rdfs:comment xml:lang="en">The marital status of a Contact /
            person.</rdfs:comment>
        <rdfs:range rdf:resource="&xsd;string"/>
    </owl:DatatypeProperty>
    


    <!-- http://www.ebu.ch/metadata/ontologies/ebucore/ebucore#contactOccupation -->

    <owl:DatatypeProperty rdf:about="&ebucore;contactOccupation">
        <rdfs:label xml:lang="en">Occupation</rdfs:label>
        <rdfs:comment xml:lang="en">The job / occupation name of a Contact /
            person.</rdfs:comment>
        <rdfs:range rdf:resource="&xsd;string"/>
    </owl:DatatypeProperty>
    


    <!-- http://www.ebu.ch/metadata/ontologies/ebucore/ebucore#contactUsername -->

    <owl:DatatypeProperty rdf:about="&ebucore;contactUsername">
        <rdfs:label xml:lang="en">Username</rdfs:label>
        <rdfs:comment xml:lang="en">The username by which a Contact / person is
            known e.g. when attributing a rating value.</rdfs:comment>
        <rdfs:range rdf:resource="&xsd;string"/>
    </owl:DatatypeProperty>
    


    <!-- http://www.ebu.ch/metadata/ontologies/ebucore/ebucore#dialogue -->

    <owl:DatatypeProperty rdf:about="&ebucore;dialogue">
        <rdfs:label xml:lang="en">Dialog indicator</rdfs:label>
        <rdfs:comment xml:lang="en">A flag to indicate the AudioContent or AudioObject contains a dialogue.</rdfs:comment>
        <rdfs:range rdf:resource="&xsd;boolean"/>
    </owl:DatatypeProperty>
    


    <!-- http://www.ebu.ch/metadata/ontologies/ebucore/ebucore#duration -->

    <owl:DatatypeProperty rdf:about="&ebucore;duration">
        <rdfs:label xml:lang="en">Duration</rdfs:label>
        <rdfs:comment xml:lang="en">To provide information on the duration of a MediaResource. It corresponds to &apos;duration&apos; in the
            Ontology for Media Resources.</rdfs:comment>
        <rdfs:range rdf:resource="&rdfs;Literal"/>
    </owl:DatatypeProperty>
    


    <!-- http://www.ebu.ch/metadata/ontologies/ebucore/ebucore#durationNormalPlayTime -->

    <owl:DatatypeProperty rdf:about="&ebucore;durationNormalPlayTime">
        <rdfs:label rdf:datatype="&xsd;string">Duration (time)</rdfs:label>
        <rdfs:comment xml:lang="en">To provide a duration as normal
            time.</rdfs:comment>
        <rdfs:range rdf:resource="&xsd;time"/>
    </owl:DatatypeProperty>
    


    <!-- http://www.ebu.ch/metadata/ontologies/ebucore/ebucore#durationNumberEditUnit -->

    <owl:DatatypeProperty rdf:about="&ebucore;durationNumberEditUnit">
        <rdfs:label rdf:datatype="&xsd;string">Duration (edit units)</rdfs:label>
        <rdfs:comment xml:lang="en">To provide a duration as a number of EditUnits
            which value is for instance the inverse of the audio sample rate or video frame
            rate.</rdfs:comment>
        <rdfs:range rdf:resource="&xsd;double"/>
    </owl:DatatypeProperty>
    


    <!-- http://www.ebu.ch/metadata/ontologies/ebucore/ebucore#durationPublished -->

    <owl:DatatypeProperty rdf:about="&ebucore;durationPublished">
        <rdfs:label xml:lang="en">Published Duration</rdfs:label>
        <rdfs:comment xml:lang="en">To provide information on the published / announced duration of an EditorialObject.</rdfs:comment>
        <rdfs:range rdf:resource="&rdfs;Literal"/>
    </owl:DatatypeProperty>
    


    <!-- http://www.ebu.ch/metadata/ontologies/ebucore/ebucore#durationPublishedNormalPlayTime -->

    <owl:DatatypeProperty rdf:about="&ebucore;durationPublishedNormalPlayTime">
        <rdfs:label xml:lang="en">Published duration (time)</rdfs:label>
        <rdfs:comment xml:lang="en">To provide a published duration as normal
            time.</rdfs:comment>
        <rdfs:range rdf:resource="&xsd;dateTime"/>
    </owl:DatatypeProperty>
    


    <!-- http://www.ebu.ch/metadata/ontologies/ebucore/ebucore#durationPublishedNumberEditUnit -->

    <owl:DatatypeProperty rdf:about="&ebucore;durationPublishedNumberEditUnit">
        <rdfs:label xml:lang="en">Published duration (edit units)</rdfs:label>
        <rdfs:comment xml:lang="en">To provide a published duration as a number of EditUnits
            which value is for instance the inverse of the audio sample rate or video frame
            rate.</rdfs:comment>
        <rdfs:range rdf:resource="&xsd;double"/>
    </owl:DatatypeProperty>
    


    <!-- http://www.ebu.ch/metadata/ontologies/ebucore/ebucore#durationPublishedTimecode -->

    <owl:DatatypeProperty rdf:about="&ebucore;durationPublishedTimecode">
        <rdfs:label xml:lang="en">Published duration (timecode)</rdfs:label>
        <rdfs:comment xml:lang="en">The published duration expressed as a
            timecode.</rdfs:comment>
        <rdfs:range rdf:resource="&xsd;string"/>
    </owl:DatatypeProperty>
    


    <!-- http://www.ebu.ch/metadata/ontologies/ebucore/ebucore#durationTimecode -->

    <owl:DatatypeProperty rdf:about="&ebucore;durationTimecode">
        <rdfs:label rdf:datatype="&xsd;string">Duration (timecode)</rdfs:label>
        <rdfs:comment xml:lang="en">The duration expressed as a
            timecode.</rdfs:comment>
        <rdfs:range rdf:resource="&xsd;string"/>
    </owl:DatatypeProperty>
    


    <!-- http://www.ebu.ch/metadata/ontologies/ebucore/ebucore#editUnit -->

    <owl:DatatypeProperty rdf:about="&ebucore;editUnit">
        <rdfs:label xml:lang="en">Edit unit</rdfs:label>
        <rdfs:comment xml:lang="en">The edit unit is e.g. the inverse of the audio
            sample rate or video frame rate.</rdfs:comment>
        <rdfs:range rdf:resource="&xsd;float"/>
    </owl:DatatypeProperty>
    


    <!-- http://www.ebu.ch/metadata/ontologies/ebucore/ebucore#end -->

    <owl:DatatypeProperty rdf:about="&ebucore;end">
        <rdfs:label xml:lang="en">End time</rdfs:label>
        <rdfs:comment xml:lang="en">The start point of the media
            resource.</rdfs:comment>
        <rdfs:range rdf:resource="&rdfs;Literal"/>
    </owl:DatatypeProperty>
    


    <!-- http://www.ebu.ch/metadata/ontologies/ebucore/ebucore#endNormalPlayTime -->

    <owl:DatatypeProperty rdf:about="&ebucore;endNormalPlayTime">
        <rdfs:label xml:lang="en">End time (time)</rdfs:label>
        <rdfs:comment xml:lang="en">The start time expressed using a time
            expression.</rdfs:comment>
        <rdfs:range rdf:resource="&xsd;time"/>
    </owl:DatatypeProperty>
    


    <!-- http://www.ebu.ch/metadata/ontologies/ebucore/ebucore#endNumberEditUnits -->

    <owl:DatatypeProperty rdf:about="&ebucore;endNumberEditUnits">
        <rdfs:label xml:lang="en">End time (edit units)</rdfs:label>
        <rdfs:comment xml:lang="en">A start time expressed as a number of edit
            units.</rdfs:comment>
        <rdfs:range rdf:resource="&xsd;double"/>
    </owl:DatatypeProperty>
    


    <!-- http://www.ebu.ch/metadata/ontologies/ebucore/ebucore#endTimecode -->

    <owl:DatatypeProperty rdf:about="&ebucore;endTimecode">
        <rdfs:label xml:lang="en">End time (timecode)</rdfs:label>
        <rdfs:comment xml:lang="en">A start time expressed as
            timecode.</rdfs:comment>
        <rdfs:range rdf:resource="&xsd;string"/>
    </owl:DatatypeProperty>
    


    <!-- http://www.ebu.ch/metadata/ontologies/ebucore/ebucore#eventDescription -->

    <owl:DatatypeProperty rdf:about="&ebucore;eventDescription">
        <rdfs:label xml:lang="en">Description</rdfs:label>
        <rdfs:comment xml:lang="en">To provide a deescription for an
            Event.</rdfs:comment>
        <rdfs:range rdf:resource="&xsd;string"/>
    </owl:DatatypeProperty>
    


    <!-- http://www.ebu.ch/metadata/ontologies/ebucore/ebucore#eventDuration -->

    <owl:DatatypeProperty rdf:about="&ebucore;eventDuration">
        <rdfs:label rdf:datatype="&xsd;string">Duration</rdfs:label>
        <rdfs:comment rdf:datatype="&xsd;string">The duration of an event.</rdfs:comment>
        <rdfs:range rdf:resource="&xsd;duration"/>
    </owl:DatatypeProperty>
    


    <!-- http://www.ebu.ch/metadata/ontologies/ebucore/ebucore#eventEndDate -->

    <owl:DatatypeProperty rdf:about="&ebucore;eventEndDate">
        <rdfs:label xml:lang="en">Event end date</rdfs:label>
        <rdfs:comment xml:lang="en">The end date of an Event.</rdfs:comment>
        <rdfs:range rdf:resource="&xsd;string"/>
    </owl:DatatypeProperty>
    


    <!-- http://www.ebu.ch/metadata/ontologies/ebucore/ebucore#eventName -->

    <owl:DatatypeProperty rdf:about="&ebucore;eventName">
        <rdfs:label xml:lang="en">Event name</rdfs:label>
        <rdfs:comment xml:lang="en">To provide a name for an Event.</rdfs:comment>
        <rdfs:range rdf:resource="&xsd;string"/>
    </owl:DatatypeProperty>
    


    <!-- http://www.ebu.ch/metadata/ontologies/ebucore/ebucore#eventStartDate -->

    <owl:DatatypeProperty rdf:about="&ebucore;eventStartDate">
        <rdfs:label xml:lang="en">Event start date</rdfs:label>
        <rdfs:comment xml:lang="en">The start date of an Event.</rdfs:comment>
        <rdfs:range rdf:resource="&xsd;string"/>
    </owl:DatatypeProperty>
    


    <!-- http://www.ebu.ch/metadata/ontologies/ebucore/ebucore#fictitious -->

    <owl:DatatypeProperty rdf:about="&ebucore;fictitious">
        <rdfs:label xml:lang="en">Fictitious agent indicator</rdfs:label>
        <rdfs:comment xml:lang="en">A flag to indicate if an agent of fictitious
            (set to true).</rdfs:comment>
        <rdfs:range rdf:resource="&xsd;boolean"/>
    </owl:DatatypeProperty>
    


    <!-- http://www.ebu.ch/metadata/ontologies/ebucore/ebucore#fileSize -->

    <owl:DatatypeProperty rdf:about="&ebucore;fileSize">
        <rdfs:label rdf:datatype="&xsd;string">File size</rdfs:label>
        <rdfs:comment xml:lang="en">to provide the size of a MediaResource in
            bytes.</rdfs:comment>
        <rdfs:range rdf:resource="&xsd;double"/>
    </owl:DatatypeProperty>
    


    <!-- http://www.ebu.ch/metadata/ontologies/ebucore/ebucore#filename -->

    <owl:DatatypeProperty rdf:about="&ebucore;filename">
        <rdfs:label xml:lang="en">File name</rdfs:label>
        <rdfs:comment xml:lang="en">The name of the file containing the
            Resource.</rdfs:comment>
        <rdfs:range rdf:resource="&xsd;string"/>
    </owl:DatatypeProperty>
    


    <!-- http://www.ebu.ch/metadata/ontologies/ebucore/ebucore#frameRate -->

    <owl:DatatypeProperty rdf:about="&ebucore;frameRate">
        <rdfs:label xml:lang="en">Frame rate</rdfs:label>
        <rdfs:comment xml:lang="en">The frame rate of the video signal in frame per
            second.</rdfs:comment>
        <rdfs:range rdf:resource="&xsd;double"/>
    </owl:DatatypeProperty>
    


    <!-- http://www.ebu.ch/metadata/ontologies/ebucore/ebucore#frameSizeUnit -->

    <owl:DatatypeProperty rdf:about="&ebucore;frameSizeUnit">
        <rdfs:label xml:lang="en">Frame size unit</rdfs:label>
        <rdfs:comment xml:lang="en">The unit used to express the frame width or
            height. The unit by default is &apos;pixel&apos;.</rdfs:comment>
        <rdfs:range rdf:resource="&xsd;string"/>
    </owl:DatatypeProperty>
    


    <!-- http://www.ebu.ch/metadata/ontologies/ebucore/ebucore#frequency -->

    <owl:DatatypeProperty rdf:about="&ebucore;frequency">
        <rdfs:label xml:lang="en">Frequency</rdfs:label>
        <rdfs:comment xml:lang="en">To provide the frequency of an AudioChannel filter</rdfs:comment>
        <rdfs:range rdf:resource="&xsd;integer"/>
    </owl:DatatypeProperty>
    


    <!-- http://www.ebu.ch/metadata/ontologies/ebucore/ebucore#groupDescription -->

    <owl:DatatypeProperty rdf:about="&ebucore;groupDescription">
        <rdfs:label xml:lang="en">Group description</rdfs:label>
        <rdfs:comment xml:lang="en">A textual description of a
            Group.</rdfs:comment>
        <rdfs:range rdf:resource="&xsd;string"/>
    </owl:DatatypeProperty>
    


    <!-- http://www.ebu.ch/metadata/ontologies/ebucore/ebucore#groupName -->

    <owl:DatatypeProperty rdf:about="&ebucore;groupName">
        <rdfs:label xml:lang="en">Group name</rdfs:label>
        <rdfs:comment xml:lang="en">The name attributed to a Group.</rdfs:comment>
        <rdfs:range rdf:resource="&xsd;string"/>
    </owl:DatatypeProperty>
    


    <!-- http://www.ebu.ch/metadata/ontologies/ebucore/ebucore#hash -->

    <owl:DatatypeProperty rdf:about="&ebucore;hash">
        <rdfs:label xml:lang="en">Hash code</rdfs:label>
        <rdfs:comment xml:lang="en">The hash value associated to a Resource. There
            are different methods / algorithms to calculate hash values, which can be defined as
            subproperties.</rdfs:comment>
        <rdfs:range rdf:resource="&xsd;string"/>
    </owl:DatatypeProperty>
    


    <!-- http://www.ebu.ch/metadata/ontologies/ebucore/ebucore#height -->

    <owl:DatatypeProperty rdf:about="&ebucore;height">
        <rdfs:label xml:lang="en">Height</rdfs:label>
        <rdfs:comment xml:lang="en">The height of e.g. a video frame typically
            expressed as a number of lines or the height of a picture/image expressed in millimeters
            or else.</rdfs:comment>
        <rdfs:range rdf:resource="&xsd;integer"/>
    </owl:DatatypeProperty>
    


    <!-- http://www.ebu.ch/metadata/ontologies/ebucore/ebucore#heightUnit -->

    <owl:DatatypeProperty rdf:about="&ebucore;heightUnit">
        <rdfs:label xml:lang="en">Height unit</rdfs:label>
        <rdfs:comment xml:lang="en">The unit used to measure a Height e.g. in
            pixels or number of lines or millimeters or else.</rdfs:comment>
        <rdfs:range rdf:resource="&xsd;string"/>
    </owl:DatatypeProperty>
    


    <!-- http://www.ebu.ch/metadata/ontologies/ebucore/ebucore#importance -->

    <owl:DatatypeProperty rdf:about="&ebucore;importance">
        <rdfs:label xml:lang="en">Audio object importance</rdfs:label>
        <rdfs:comment xml:lang="en">To indicate the importance of an AudioObject or AudioPack.</rdfs:comment>
        <rdfs:range rdf:resource="&xsd;string"/>
    </owl:DatatypeProperty>
    


    <!-- http://www.ebu.ch/metadata/ontologies/ebucore/ebucore#interact -->

    <owl:DatatypeProperty rdf:about="&ebucore;interact">
        <rdfs:label xml:lang="en">Interaction flag</rdfs:label>
        <rdfs:comment xml:lang="en">A flag to indicate if the user can interact woith the content.</rdfs:comment>
        <rdfs:range rdf:resource="&xsd;boolean"/>
    </owl:DatatypeProperty>
    


    <!-- http://www.ebu.ch/metadata/ontologies/ebucore/ebucore#keywordDefinition -->

    <owl:DatatypeProperty rdf:about="&ebucore;keywordDefinition">
        <rdfs:label xml:lang="en">Keyword definition</rdfs:label>
        <rdfs:comment xml:lang="en">To provide a definition for a Keyword.</rdfs:comment>
        <rdfs:range rdf:resource="&xsd;string"/>
    </owl:DatatypeProperty>
    


    <!-- http://www.ebu.ch/metadata/ontologies/ebucore/ebucore#lineNumber -->

    <owl:DatatypeProperty rdf:about="&ebucore;lineNumber">
        <rdfs:label xml:lang="en">Line number</rdfs:label>
        <rdfs:comment xml:lang="en">To provide the number of the line on which
            ancillary data is being carried and the equivalent in the digital domain.</rdfs:comment>
        <rdfs:range rdf:resource="&xsd;integer"/>
    </owl:DatatypeProperty>
    


    <!-- http://www.ebu.ch/metadata/ontologies/ebucore/ebucore#locationAddress -->

    <owl:DatatypeProperty rdf:about="&ebucore;locationAddress">
        <rdfs:label xml:lang="en">Address</rdfs:label>
        <rdfs:comment xml:lang="en">To provide the address of a
           Location.</rdfs:comment>
        <rdfs:range rdf:resource="&xsd;string"/>
    </owl:DatatypeProperty>
    


    <!-- http://www.ebu.ch/metadata/ontologies/ebucore/ebucore#locationAltitude -->

    <owl:DatatypeProperty rdf:about="&ebucore;locationAltitude">
        <rdfs:label xml:lang="en">Altitude</rdfs:label>
        <rdfs:comment xml:lang="en">To define the altitude of a Location in
            meters.</rdfs:comment>
        <rdfs:range rdf:resource="&xsd;double"/>
    </owl:DatatypeProperty>
    


    <!-- http://www.ebu.ch/metadata/ontologies/ebucore/ebucore#locationCoordinateSystemName -->

    <owl:DatatypeProperty rdf:about="&ebucore;locationCoordinateSystemName">
        <rdfs:label xml:lang="en">Coordinate system</rdfs:label>
        <rdfs:comment xml:lang="en">To specify the name of the gps coordinate
            system used for the Location.</rdfs:comment>
        <rdfs:range rdf:resource="&xsd;string"/>
    </owl:DatatypeProperty>
    


    <!-- http://www.ebu.ch/metadata/ontologies/ebucore/ebucore#locationDescription -->

    <owl:DatatypeProperty rdf:about="&ebucore;locationDescription">
        <rdfs:label xml:lang="en">Location description</rdfs:label>
        <rdfs:comment xml:lang="en">To provide a description of a particular Location.</rdfs:comment>
        <rdfs:range rdf:resource="&xsd;string"/>
    </owl:DatatypeProperty>
    


    <!-- http://www.ebu.ch/metadata/ontologies/ebucore/ebucore#locationLatitude -->

    <owl:DatatypeProperty rdf:about="&ebucore;locationLatitude">
        <rdfs:label xml:lang="en">Latitude</rdfs:label>
        <rdfs:comment xml:lang="en">The latitude of the Location.</rdfs:comment>
        <rdfs:range rdf:resource="&xsd;double"/>
    </owl:DatatypeProperty>
    


    <!-- http://www.ebu.ch/metadata/ontologies/ebucore/ebucore#locationLongitude -->

    <owl:DatatypeProperty rdf:about="&ebucore;locationLongitude">
        <rdfs:label xml:lang="en">Longitude</rdfs:label>
        <rdfs:comment xml:lang="en">To define the longitude of the
            Location.</rdfs:comment>
        <rdfs:range rdf:resource="&xsd;double"/>
    </owl:DatatypeProperty>
    


    <!-- http://www.ebu.ch/metadata/ontologies/ebucore/ebucore#locationName -->

    <owl:DatatypeProperty rdf:about="&ebucore;locationName">
        <rdfs:label xml:lang="en">Location name</rdfs:label>
        <rdfs:comment xml:lang="en">The name by which a Location is
            known.</rdfs:comment>
        <rdfs:range rdf:resource="&xsd;string"/>
    </owl:DatatypeProperty>
    


    <!-- http://www.ebu.ch/metadata/ontologies/ebucore/ebucore#locationRegion -->

    <owl:DatatypeProperty rdf:about="&ebucore;locationRegion">
        <rdfs:label xml:lang="en">Region</rdfs:label>
        <rdfs:comment xml:lang="en">To provide a description of a particular region assocoated to the Location.</rdfs:comment>
        <rdfs:range rdf:resource="&xsd;string"/>
    </owl:DatatypeProperty>
    


    <!-- http://www.ebu.ch/metadata/ontologies/ebucore/ebucore#locator -->

    <owl:DatatypeProperty rdf:about="&ebucore;locator">
        <rdfs:label rdf:datatype="&xsd;string">Locator</rdfs:label>
        <rdfs:comment xml:lang="en">A locator from where the Resource can be accessed.</rdfs:comment>
        <rdfs:range rdf:resource="&xsd;string"/>
    </owl:DatatypeProperty>
    


    <!-- http://www.ebu.ch/metadata/ontologies/ebucore/ebucore#locatorTargetInformation -->

    <owl:DatatypeProperty rdf:about="&ebucore;locatorTargetInformation">
        <rdfs:label xml:lang="en">Target information</rdfs:label>
        <rdfs:comment xml:lang="en">Information about storage accessed by the locator.</rdfs:comment>
        <rdfs:range rdf:resource="&xsd;string"/>
    </owl:DatatypeProperty>
    


    <!-- http://www.ebu.ch/metadata/ontologies/ebucore/ebucore#loudnessIntegratedLoudness -->

    <owl:DatatypeProperty rdf:about="&ebucore;loudnessIntegratedLoudness">
        <rdfs:label xml:lang="en">Integrated loudness</rdfs:label>
        <rdfs:comment xml:lang="en">The value for integrated loudness measured at AudioProgramme or AudioContent level.</rdfs:comment>
        <rdfs:range rdf:resource="&xsd;float"/>
    </owl:DatatypeProperty>
    


    <!-- http://www.ebu.ch/metadata/ontologies/ebucore/ebucore#loudnessMaxMomentary -->

    <owl:DatatypeProperty rdf:about="&ebucore;loudnessMaxMomentary">
        <rdfs:label xml:lang="en">Max momentary loudness</rdfs:label>
        <rdfs:comment xml:lang="en">The value for maximum momentary loudness measured at AudioProgramme or AudioContent level.</rdfs:comment>
        <rdfs:range rdf:resource="&xsd;float"/>
    </owl:DatatypeProperty>
    


    <!-- http://www.ebu.ch/metadata/ontologies/ebucore/ebucore#loudnessMaxTruepeak -->

    <owl:DatatypeProperty rdf:about="&ebucore;loudnessMaxTruepeak">
        <rdfs:label xml:lang="en">Max true peak loudness</rdfs:label>
        <rdfs:comment xml:lang="en">The value for maximum true peak loudness measured at AudioProgramme or AudioContent level.</rdfs:comment>
        <rdfs:range rdf:resource="&xsd;float"/>
    </owl:DatatypeProperty>
    


    <!-- http://www.ebu.ch/metadata/ontologies/ebucore/ebucore#loudnessMethod -->

    <owl:DatatypeProperty rdf:about="&ebucore;loudnessMethod">
        <rdfs:label xml:lang="en">Loudness method</rdfs:label>
        <rdfs:comment xml:lang="en">The method for loudness measurement at AudioProgramme or AudioContent level.</rdfs:comment>
        <rdfs:range rdf:resource="&xsd;float"/>
    </owl:DatatypeProperty>
    


    <!-- http://www.ebu.ch/metadata/ontologies/ebucore/ebucore#loudnessParameters -->

    <owl:DatatypeProperty rdf:about="&ebucore;loudnessParameters">
        <rdfs:label xml:lang="en">loudness parameters</rdfs:label>
        <rdfs:comment xml:lang="en">All the parameters for measurement of loudness at the AudioContent or AudioProgramme level.</rdfs:comment>
        <rdfs:range rdf:resource="&rdfs;Literal"/>
    </owl:DatatypeProperty>
    


    <!-- http://www.ebu.ch/metadata/ontologies/ebucore/ebucore#loudnessRange -->

    <owl:DatatypeProperty rdf:about="&ebucore;loudnessRange">
        <rdfs:label xml:lang="en">Loudness range</rdfs:label>
        <rdfs:comment xml:lang="en">The loudness range measured at AudioProgramme or AudioContent level.</rdfs:comment>
        <rdfs:range rdf:resource="&xsd;float"/>
    </owl:DatatypeProperty>
    


    <!-- http://www.ebu.ch/metadata/ontologies/ebucore/ebucore#lounessMaxShortTerm -->

    <owl:DatatypeProperty rdf:about="&ebucore;lounessMaxShortTerm">
        <rdfs:label xml:lang="en">Max short term loudness</rdfs:label>
        <rdfs:comment xml:lang="en">The maximum short term loudness measured at AudioProgramme or AudioContent level.</rdfs:comment>
        <rdfs:range rdf:resource="&xsd;float"/>
    </owl:DatatypeProperty>
    


    <!-- http://www.ebu.ch/metadata/ontologies/ebucore/ebucore#noiseFilter -->

    <owl:DatatypeProperty rdf:about="&ebucore;noiseFilter">
        <rdfs:label xml:lang="en">Noise filter</rdfs:label>
        <rdfs:comment xml:lang="en">A flag to signal that a noise filter has been
            used.</rdfs:comment>
        <rdfs:range rdf:resource="&xsd;boolean"/>
    </owl:DatatypeProperty>
    


    <!-- http://www.ebu.ch/metadata/ontologies/ebucore/ebucore#notRated -->

    <owl:DatatypeProperty rdf:about="&ebucore;notRated">
        <rdfs:label xml:lang="en">Not rated</rdfs:label>
        <rdfs:comment xml:lang="en">A flag to indicate that the BusinessObejct has not been rated.</rdfs:comment>
        <rdfs:range rdf:resource="&xsd;boolean"/>
    </owl:DatatypeProperty>
    


    <!-- http://www.ebu.ch/metadata/ontologies/ebucore/ebucore#numberOfTracks -->

    <owl:DatatypeProperty rdf:about="&ebucore;numberOfTracks">
        <rdfs:label xml:lang="en">Number of tracks</rdfs:label>
        <rdfs:comment xml:lang="en">The number of Tracks composing the MediaResource.</rdfs:comment>
        <rdfs:range rdf:resource="&xsd;integer"/>
    </owl:DatatypeProperty>
    


    <!-- http://www.ebu.ch/metadata/ontologies/ebucore/ebucore#objectTypeDefinition -->

    <owl:DatatypeProperty rdf:about="&ebucore;objectTypeDefinition">
        <rdfs:label xml:lang="en">Audio object type definition</rdfs:label>
        <rdfs:comment xml:lang="en">To provide a definition of an AudioObject type.</rdfs:comment>
        <rdfs:range rdf:resource="&xsd;string"/>
    </owl:DatatypeProperty>
    


    <!-- http://www.ebu.ch/metadata/ontologies/ebucore/ebucore#officeHomepage -->

    <owl:DatatypeProperty rdf:about="&ebucore;officeHomepage">
        <rdfs:label xml:lang="en">Homepage (office)</rdfs:label>
        <rdfs:comment xml:lang="en">To provide an office/professional/company web
            homepage of an Agent (Contact/person or Organisation).</rdfs:comment>
        <rdfs:range rdf:resource="&xsd;anyURI"/>
    </owl:DatatypeProperty>
    


    <!-- http://www.ebu.ch/metadata/ontologies/ebucore/ebucore#officeMailAddress -->

    <owl:DatatypeProperty rdf:about="&ebucore;officeMailAddress">
        <rdfs:label xml:lang="en">Office mail address</rdfs:label>
        <rdfs:comment xml:lang="en">To provide the professional / office address of
            an agent (Contact/person or organisation).</rdfs:comment>
        <rdfs:range rdf:resource="&xsd;string"/>
    </owl:DatatypeProperty>
    


    <!-- http://www.ebu.ch/metadata/ontologies/ebucore/ebucore#officeTelephoneNumber -->

    <owl:DatatypeProperty rdf:about="&ebucore;officeTelephoneNumber">
        <rdfs:label xml:lang="en">Telephone (office)</rdfs:label>
        <rdfs:comment xml:lang="en">To provide an office/professional/company
            telephone number of an Agent (Contact/person or Organisation).</rdfs:comment>
        <rdfs:range rdf:resource="&xsd;string"/>
    </owl:DatatypeProperty>
    


    <!-- http://www.ebu.ch/metadata/ontologies/ebucore/ebucore#organisationName -->

    <owl:DatatypeProperty rdf:about="&ebucore;organisationName">
        <rdfs:label xml:lang="en">Name</rdfs:label>
        <rdfs:comment xml:lang="en">To provide the full name of an Organisation.</rdfs:comment>
        <rdfs:range rdf:resource="&xsd;string"/>
    </owl:DatatypeProperty>
    


    <!-- http://www.ebu.ch/metadata/ontologies/ebucore/ebucore#orientation -->

    <owl:DatatypeProperty rdf:about="&ebucore;orientation">
        <rdfs:label xml:lang="en">Orientation</rdfs:label>
        <rdfs:comment xml:lang="en">The orientation of a Document or an Image i.e. landscape or
            portrait.</rdfs:comment>
        <rdfs:range rdf:resource="&xsd;string"/>
    </owl:DatatypeProperty>
    


    <!-- http://www.ebu.ch/metadata/ontologies/ebucore/ebucore#packageByteSize -->

    <owl:DatatypeProperty rdf:about="&ebucore;packageByteSize">
        <rdfs:label xml:lang="en">Package size (in bytes)</rdfs:label>
        <rdfs:comment xml:lang="en">The size of a media package in
            Bytes.</rdfs:comment>
        <rdfs:range rdf:resource="&xsd;long"/>
    </owl:DatatypeProperty>
    


    <!-- http://www.ebu.ch/metadata/ontologies/ebucore/ebucore#packageName -->

    <owl:DatatypeProperty rdf:about="&ebucore;packageName">
        <rdfs:label xml:lang="en">Package name</rdfs:label>
        <rdfs:comment xml:lang="en">The name attributed to a
            package.</rdfs:comment>
        <rdfs:range rdf:resource="&xsd;long"/>
    </owl:DatatypeProperty>
    


    <!-- http://www.ebu.ch/metadata/ontologies/ebucore/ebucore#partDefinition -->

    <owl:DatatypeProperty rdf:about="&ebucore;partDefinition">
        <rdfs:label xml:lang="en">Part definition</rdfs:label>
        <rdfs:comment xml:lang="en">A definition associated with the Part.</rdfs:comment>
        <rdfs:range rdf:resource="&xsd;string"/>
    </owl:DatatypeProperty>
    


    <!-- http://www.ebu.ch/metadata/ontologies/ebucore/ebucore#partName -->

    <owl:DatatypeProperty rdf:about="&ebucore;partName">
        <rdfs:label xml:lang="en">Part name</rdfs:label>
        <rdfs:comment xml:lang="en">A name by which the Part is identified.</rdfs:comment>
        <rdfs:range rdf:resource="&xsd;string"/>
    </owl:DatatypeProperty>
    


    <!-- http://www.ebu.ch/metadata/ontologies/ebucore/ebucore#partNumber -->

    <owl:DatatypeProperty rdf:about="&ebucore;partNumber">
        <rdfs:label xml:lang="en">Part number</rdfs:label>
        <rdfs:comment xml:lang="en">The number associated to a Part as one among
            many.</rdfs:comment>
        <rdfs:range rdf:resource="&xsd;integer"/>
    </owl:DatatypeProperty>
    


    <!-- http://www.ebu.ch/metadata/ontologies/ebucore/ebucore#partTotalNumber -->

    <owl:DatatypeProperty rdf:about="&ebucore;partTotalNumber">
        <rdfs:label xml:lang="en">Total number of parts</rdfs:label>
        <rdfs:comment xml:lang="en">The total number of Parts associated with a
            BusinessObject.</rdfs:comment>
        <rdfs:range rdf:resource="&xsd;integer"/>
    </owl:DatatypeProperty>
    


    <!-- http://www.ebu.ch/metadata/ontologies/ebucore/ebucore#privateHomepage -->

    <owl:DatatypeProperty rdf:about="&ebucore;privateHomepage">
        <rdfs:label xml:lang="en">Homepage (private)</rdfs:label>
        <rdfs:comment xml:lang="en">To provide an private web homepage of an Agent
            (Contact/person).</rdfs:comment>
        <rdfs:range rdf:resource="&xsd;anyURI"/>
    </owl:DatatypeProperty>
    


    <!-- http://www.ebu.ch/metadata/ontologies/ebucore/ebucore#privateMailAddress -->

    <owl:DatatypeProperty rdf:about="&ebucore;privateMailAddress">
        <rdfs:label xml:lang="en">Private mail address</rdfs:label>
        <rdfs:comment xml:lang="en">To provide the private / personal address of an
            agent (Contact/person).</rdfs:comment>
        <rdfs:range rdf:resource="&xsd;string"/>
    </owl:DatatypeProperty>
    


    <!-- http://www.ebu.ch/metadata/ontologies/ebucore/ebucore#privateTelephoneNumber -->

    <owl:DatatypeProperty rdf:about="&ebucore;privateTelephoneNumber">
        <rdfs:label xml:lang="en">Telephone (private)</rdfs:label>
        <rdfs:comment xml:lang="en">To provide the private telephone number of an
            Agent (Contact/person).</rdfs:comment>
        <rdfs:range rdf:resource="&xsd;string"/>
    </owl:DatatypeProperty>
    


    <!-- http://www.ebu.ch/metadata/ontologies/ebucore/ebucore#publicationChannelName -->

    <owl:DatatypeProperty rdf:about="&ebucore;publicationChannelName">
        <rdfs:label xml:lang="en">Publication channel name</rdfs:label>
        <rdfs:comment xml:lang="en">To provide a name to a PublicationChannel e.g. a TV channel or website.</rdfs:comment>
        <rdfs:range rdf:resource="&xsd;string"/>
    </owl:DatatypeProperty>
    


    <!-- http://www.ebu.ch/metadata/ontologies/ebucore/ebucore#publicationEndDateTime -->

    <owl:DatatypeProperty rdf:about="&ebucore;publicationEndDateTime">
        <rdfs:label xml:lang="en">Publication end date &amp; time</rdfs:label>
        <rdfs:comment xml:lang="en">The actual end date and time of a PublicationEvent.</rdfs:comment>
        <rdfs:range rdf:resource="&xsd;dateTime"/>
    </owl:DatatypeProperty>
    


    <!-- http://www.ebu.ch/metadata/ontologies/ebucore/ebucore#publicationEventName -->

    <owl:DatatypeProperty rdf:about="&ebucore;publicationEventName">
        <rdfs:label xml:lang="en">Publication event name</rdfs:label>
        <rdfs:comment xml:lang="en">To provide a name to a PublicationEvent.</rdfs:comment>
        <rdfs:range rdf:resource="&xsd;string"/>
    </owl:DatatypeProperty>
    


    <!-- http://www.ebu.ch/metadata/ontologies/ebucore/ebucore#publicationScheduleDate -->

    <owl:DatatypeProperty rdf:about="&ebucore;publicationScheduleDate">
        <rdfs:label xml:lang="en">schedule date</rdfs:label>
        <rdfs:comment xml:lang="en">To express specifically the schedule date to which a PublicationEvent is related in particular if the broacdast time is after midnight. For example, the schedule date would be May 29th and the programme is published at 1 am on May 30th, while still associated in the schedule with the night of May 29th.</rdfs:comment>
        <rdfs:range rdf:resource="&xsd;date"/>
    </owl:DatatypeProperty>
    


    <!-- http://www.ebu.ch/metadata/ontologies/ebucore/ebucore#publicationStartDateTime -->

    <owl:DatatypeProperty rdf:about="&ebucore;publicationStartDateTime">
        <rdfs:label xml:lang="en">Publication start date &amp; time</rdfs:label>
        <rdfs:comment xml:lang="en">The actual start date and time of a PublicationEvent.</rdfs:comment>
        <rdfs:range rdf:resource="&xsd;dateTime"/>
    </owl:DatatypeProperty>
    


    <!-- http://www.ebu.ch/metadata/ontologies/ebucore/ebucore#publishedEndDateTime -->

    <owl:DatatypeProperty rdf:about="&ebucore;publishedEndDateTime">
        <rdfs:label xml:lang="en">Publication end date &amp; time</rdfs:label>
        <rdfs:comment xml:lang="en">The end date and time of a PublicationEvent as
            scheduled.</rdfs:comment>
        <rdfs:range rdf:resource="&xsd;dateTime"/>
    </owl:DatatypeProperty>
    


    <!-- http://www.ebu.ch/metadata/ontologies/ebucore/ebucore#publishedStartDateTime -->

    <owl:DatatypeProperty rdf:about="&ebucore;publishedStartDateTime">
        <rdfs:label xml:lang="en">Publication start date &amp; time</rdfs:label>
        <rdfs:comment xml:lang="en">The start date and time of a PublicationEvent
            as scheduled.</rdfs:comment>
        <rdfs:range rdf:resource="&xsd;dateTime"/>
    </owl:DatatypeProperty>
    


    <!-- http://www.ebu.ch/metadata/ontologies/ebucore/ebucore#publishedTitle -->

    <owl:DatatypeProperty rdf:about="&ebucore;publishedTitle">
        <rdfs:label xml:lang="en">Published title.</rdfs:label>
        <rdfs:comment xml:lang="en">The title used to identify the work at publication time.</rdfs:comment>
        <rdfs:range rdf:resource="&xsd;string"/>
    </owl:DatatypeProperty>
    


    <!-- http://www.ebu.ch/metadata/ontologies/ebucore/ebucore#ratingScaleMax -->

    <owl:DatatypeProperty rdf:about="&ebucore;ratingScaleMax">
        <rdfs:label xml:lang="en">Rating scale (top value)</rdfs:label>
        <rdfs:comment xml:lang="en">The maximum value of the scale used for rating
            a media resource.</rdfs:comment>
        <rdfs:range rdf:resource="&xsd;string"/>
    </owl:DatatypeProperty>
    


    <!-- http://www.ebu.ch/metadata/ontologies/ebucore/ebucore#ratingScaleMin -->

    <owl:DatatypeProperty rdf:about="&ebucore;ratingScaleMin">
        <rdfs:label xml:lang="en">Rating scale (min. value)</rdfs:label>
        <rdfs:comment xml:lang="en">The minimum value of the scale used for rating
            a Resource.</rdfs:comment>
        <rdfs:range rdf:resource="&xsd;string"/>
    </owl:DatatypeProperty>
    


    <!-- http://www.ebu.ch/metadata/ontologies/ebucore/ebucore#ratingSystemEnvironment -->

    <owl:DatatypeProperty rdf:about="&ebucore;ratingSystemEnvironment">
        <rdfs:label xml:lang="en">Rating environment</rdfs:label>
        <rdfs:comment xml:lang="en">To identify the environment in which rating applies.</rdfs:comment>
        <rdfs:range rdf:resource="&xsd;string"/>
    </owl:DatatypeProperty>
    


    <!-- http://www.ebu.ch/metadata/ontologies/ebucore/ebucore#ratingSystemName -->

    <owl:DatatypeProperty rdf:about="&ebucore;ratingSystemName">
        <rdfs:label xml:lang="en">Rating system</rdfs:label>
        <rdfs:comment xml:lang="en">To identify a rating system by its name.</rdfs:comment>
        <rdfs:range rdf:resource="&xsd;string"/>
    </owl:DatatypeProperty>
    


    <!-- http://www.ebu.ch/metadata/ontologies/ebucore/ebucore#ratingValue -->

    <owl:DatatypeProperty rdf:about="&ebucore;ratingValue">
        <rdfs:label xml:lang="en">Rating</rdfs:label>
        <rdfs:comment xml:lang="en">To express a free text rating value defined in
            a rating classification scheme.</rdfs:comment>
        <rdfs:range rdf:resource="&xsd;string"/>
    </owl:DatatypeProperty>
    


    <!-- http://www.ebu.ch/metadata/ontologies/ebucore/ebucore#reason -->

    <owl:DatatypeProperty rdf:about="&ebucore;reason">
        <rdfs:label xml:lang="en">Reason</rdfs:label>
        <rdfs:comment xml:lang="en">To provide a reason for which Rating as been attributed as provided.</rdfs:comment>
        <rdfs:range rdf:resource="&xsd;string"/>
    </owl:DatatypeProperty>
    


    <!-- http://www.ebu.ch/metadata/ontologies/ebucore/ebucore#regionDelimX -->

    <owl:DatatypeProperty rdf:about="&ebucore;regionDelimX">
        <rdfs:label xml:lang="en">Region delimiter (x-axis)</rdfs:label>
        <rdfs:comment xml:lang="en">To define the bottom right corner of a zone on
            the x-axis. If present with regionDelimY, the zone definition is complemented by the
            associated values of the height and width.</rdfs:comment>
        <rdfs:range rdf:resource="&xsd;integer"/>
    </owl:DatatypeProperty>
    


    <!-- http://www.ebu.ch/metadata/ontologies/ebucore/ebucore#regionDelimY -->

    <owl:DatatypeProperty rdf:about="&ebucore;regionDelimY">
        <rdfs:label xml:lang="en">Region delimiter (y-axis)</rdfs:label>
        <rdfs:comment xml:lang="en">To define the bottom right corner of a zone on
            the y-axis. If present with regionDelimX, the zone definition is complemented by the
            associated values of the height and width.</rdfs:comment>
        <rdfs:range rdf:resource="&xsd;integer"/>
    </owl:DatatypeProperty>
    


    <!-- http://www.ebu.ch/metadata/ontologies/ebucore/ebucore#relatedLink -->

    <owl:DatatypeProperty rdf:about="&ebucore;relatedLink">
        <rdfs:label xml:lang="en">Related resources</rdfs:label>
        <rdfs:comment xml:lang="en">To provide a link to a web resource containing
            information related to an Agent (Contact/person or Organisation).</rdfs:comment>
        <rdfs:range rdf:resource="&xsd;anyURI"/>
    </owl:DatatypeProperty>
    


    <!-- http://www.ebu.ch/metadata/ontologies/ebucore/ebucore#resourceName -->

    <owl:DatatypeProperty rdf:about="&ebucore;resourceName">
        <rdfs:label xml:lang="en">Resource description</rdfs:label>
        <rdfs:comment xml:lang="en">A name by which the resource can be identified.</rdfs:comment>
        <rdfs:range rdf:resource="&xsd;string"/>
    </owl:DatatypeProperty>
    


    <!-- http://www.ebu.ch/metadata/ontologies/ebucore/ebucore#rightsExpression -->

    <owl:DatatypeProperty rdf:about="&ebucore;rightsExpression">
        <rdfs:label xml:lang="en">Rights expression</rdfs:label>
        <rdfs:comment xml:lang="en">The expression of Rights as free
            text.</rdfs:comment>
        <rdfs:range rdf:resource="&xsd;string"/>
    </owl:DatatypeProperty>
    


    <!-- http://www.ebu.ch/metadata/ontologies/ebucore/ebucore#rightsLink -->

    <owl:DatatypeProperty rdf:about="&ebucore;rightsLink">
        <rdfs:label xml:lang="en">Rights web resource</rdfs:label>
        <rdfs:comment xml:lang="en">A link to e.g. a webpage where an expression of
            the rights can be found and consulted.</rdfs:comment>
        <rdfs:range rdf:resource="&xsd;anyURI"/>
    </owl:DatatypeProperty>
    


    <!-- http://www.ebu.ch/metadata/ontologies/ebucore/ebucore#roleDefinition -->

    <owl:DatatypeProperty rdf:about="&ebucore;roleDefinition">
        <rdfs:label xml:lang="en">Role definition</rdfs:label>
        <rdfs:comment xml:lang="en">To provide a definition for a role</rdfs:comment>
        <rdfs:range rdf:resource="&xsd;string"/>
    </owl:DatatypeProperty>
    


    <!-- http://www.ebu.ch/metadata/ontologies/ebucore/ebucore#sampleRate -->

    <owl:DatatypeProperty rdf:about="&ebucore;sampleRate">
        <rdfs:label xml:lang="en">Sample Rate</rdfs:label>
        <rdfs:comment xml:lang="en">The frequency at which audio is sampled per second. Also called sampling rate.</rdfs:comment>
        <rdfs:range rdf:resource="&xsd;integer"/>
    </owl:DatatypeProperty>
    


    <!-- http://www.ebu.ch/metadata/ontologies/ebucore/ebucore#sampleSize -->

    <owl:DatatypeProperty rdf:about="&ebucore;sampleSize">
        <rdfs:label xml:lang="en">Sample size</rdfs:label>
        <rdfs:comment xml:lang="en">The size of an audio sample in
            bits. Also called bit depth.</rdfs:comment>
        <rdfs:range rdf:resource="&xsd;integer"/>
    </owl:DatatypeProperty>
    


    <!-- http://www.ebu.ch/metadata/ontologies/ebucore/ebucore#sampleType -->

    <owl:DatatypeProperty rdf:about="&ebucore;sampleType">
        <rdfs:label xml:lang="en">Sample type</rdfs:label>
        <rdfs:comment xml:lang="en">The type of audio sample.</rdfs:comment>
        <rdfs:range rdf:resource="&xsd;string"/>
    </owl:DatatypeProperty>
    


    <!-- http://www.ebu.ch/metadata/ontologies/ebucore/ebucore#scanningFormat -->

    <owl:DatatypeProperty rdf:about="&ebucore;scanningFormat">
        <rdfs:label xml:lang="en">Sampling format</rdfs:label>
        <rdfs:comment xml:lang="en">To define the scanning format for a
            MediaResource. For video, the two main values are &quot;interlaced&quot; or
            &quot;progressive&quot;.</rdfs:comment>
        <rdfs:range rdf:resource="&xsd;string"/>
    </owl:DatatypeProperty>
    


    <!-- http://www.ebu.ch/metadata/ontologies/ebucore/ebucore#signingSource -->

    <owl:DatatypeProperty rdf:about="&ebucore;signingSource">
        <rdfs:label xml:lang="en">Signing source</rdfs:label>
        <rdfs:comment xml:lang="en">To identify the source of the signing
            resource.</rdfs:comment>
        <rdfs:range rdf:resource="&xsd;string"/>
    </owl:DatatypeProperty>
    


    <!-- http://www.ebu.ch/metadata/ontologies/ebucore/ebucore#start -->

    <owl:DatatypeProperty rdf:about="&ebucore;start">
        <rdfs:label xml:lang="en">Start time</rdfs:label>
        <rdfs:comment xml:lang="en">The start point of the MediaResource.</rdfs:comment>
        <rdfs:range rdf:resource="&rdfs;Literal"/>
    </owl:DatatypeProperty>
    


    <!-- http://www.ebu.ch/metadata/ontologies/ebucore/ebucore#startNormalPlayTime -->

    <owl:DatatypeProperty rdf:about="&ebucore;startNormalPlayTime">
        <rdfs:label xml:lang="en">Start time (time)</rdfs:label>
        <rdfs:comment xml:lang="en">The start time expressed using a time
            expression.</rdfs:comment>
        <rdfs:range rdf:resource="&xsd;time"/>
    </owl:DatatypeProperty>
    


    <!-- http://www.ebu.ch/metadata/ontologies/ebucore/ebucore#startNumberEditUnits -->

    <owl:DatatypeProperty rdf:about="&ebucore;startNumberEditUnits">
        <rdfs:label xml:lang="en">Start time (edit units)</rdfs:label>
        <rdfs:comment xml:lang="en">A start time expressed as a number of edit
            units.</rdfs:comment>
        <rdfs:range rdf:resource="&xsd;double"/>
    </owl:DatatypeProperty>
    


    <!-- http://www.ebu.ch/metadata/ontologies/ebucore/ebucore#startTimecode -->

    <owl:DatatypeProperty rdf:about="&ebucore;startTimecode">
        <rdfs:label xml:lang="en">Start time (timecode)</rdfs:label>
        <rdfs:comment xml:lang="en">A start time expressed as
            timecode.</rdfs:comment>
        <rdfs:range rdf:resource="&xsd;string"/>
    </owl:DatatypeProperty>
    


    <!-- http://www.ebu.ch/metadata/ontologies/ebucore/ebucore#storageDefinition -->

    <owl:DatatypeProperty rdf:about="&ebucore;storageDefinition">
        <rdfs:label xml:lang="en">Storage definition</rdfs:label>
        <rdfs:comment xml:lang="en">To provide a definition for storage.</rdfs:comment>
        <rdfs:range rdf:resource="&xsd;string"/>
    </owl:DatatypeProperty>
    


    <!-- http://www.ebu.ch/metadata/ontologies/ebucore/ebucore#subtitlingSource -->

    <owl:DatatypeProperty rdf:about="&ebucore;subtitlingSource">
        <rdfs:label xml:lang="en">Subtitling source</rdfs:label>
        <rdfs:comment xml:lang="en">To identify the source of the Subtitling
            resource.</rdfs:comment>
        <rdfs:range rdf:resource="&xsd;string"/>
    </owl:DatatypeProperty>
    


    <!-- http://www.ebu.ch/metadata/ontologies/ebucore/ebucore#summary -->

    <owl:DatatypeProperty rdf:about="&ebucore;summary">
        <rdfs:label xml:lang="en">Summary</rdfs:label>
        <rdfs:comment xml:lang="en">To provide a summary.</rdfs:comment>
        <rdfs:range rdf:resource="&xsd;string"/>
    </owl:DatatypeProperty>
    


    <!-- http://www.ebu.ch/metadata/ontologies/ebucore/ebucore#synopsis -->

    <owl:DatatypeProperty rdf:about="&ebucore;synopsis">
        <rdfs:label xml:lang="en">Synopsis</rdfs:label>
        <rdfs:comment xml:lang="en">To provide a summary.</rdfs:comment>
        <rdfs:range rdf:resource="&xsd;string"/>
    </owl:DatatypeProperty>
    


    <!-- http://www.ebu.ch/metadata/ontologies/ebucore/ebucore#targetAudienceSystem -->

    <owl:DatatypeProperty rdf:about="&ebucore;targetAudienceSystem">
        <rdfs:label xml:lang="en">Target audience system</rdfs:label>
        <rdfs:comment xml:lang="en">To define the system used to provide a TargetAudience.</rdfs:comment>
        <rdfs:range rdf:resource="&xsd;string"/>
    </owl:DatatypeProperty>
    


    <!-- http://www.ebu.ch/metadata/ontologies/ebucore/ebucore#textualAnnotation -->

    <owl:DatatypeProperty rdf:about="&ebucore;textualAnnotation">
        <rdfs:label xml:lang="en">Note</rdfs:label>
        <rdfs:comment xml:lang="en">The value of an Annotation as free
            text.</rdfs:comment>
        <rdfs:range rdf:resource="&xsd;string"/>
    </owl:DatatypeProperty>
    


    <!-- http://www.ebu.ch/metadata/ontologies/ebucore/ebucore#trackDefinition -->

    <owl:DatatypeProperty rdf:about="&ebucore;trackDefinition">
        <rdfs:label xml:lang="en">Definition</rdfs:label>
        <rdfs:comment xml:lang="en">To provide a definition associated to a
            Track.</rdfs:comment>
        <rdfs:range rdf:resource="&xsd;string"/>
    </owl:DatatypeProperty>
    


    <!-- http://www.ebu.ch/metadata/ontologies/ebucore/ebucore#trackName -->

    <owl:DatatypeProperty rdf:about="&ebucore;trackName">
        <rdfs:label xml:lang="en">Track name</rdfs:label>
        <rdfs:comment xml:lang="en">The name attributed to a Track.</rdfs:comment>
        <rdfs:range rdf:resource="&xsd;string"/>
    </owl:DatatypeProperty>
    


    <!-- http://www.ebu.ch/metadata/ontologies/ebucore/ebucore#width -->

    <owl:DatatypeProperty rdf:about="&ebucore;width">
        <rdfs:label xml:lang="en">Width</rdfs:label>
        <rdfs:comment xml:lang="en">The width of e.g. a video frame typically
            expressed as a number of pixels, or picture/image in millimeters.</rdfs:comment>
        <rdfs:range rdf:resource="&xsd;integer"/>
    </owl:DatatypeProperty>
    


    <!-- http://www.ebu.ch/metadata/ontologies/ebucore/ebucore#widthUnit -->

    <owl:DatatypeProperty rdf:about="&ebucore;widthUnit">
        <rdfs:label xml:lang="en">Width unit</rdfs:label>
        <rdfs:comment xml:lang="en">The unit used to measure a width e.g. in pixels
            or number of lines or millimeters or else.</rdfs:comment>
        <rdfs:range rdf:resource="&xsd;string"/>
    </owl:DatatypeProperty>
    


    <!-- http://www.ebu.ch/metadata/ontologies/ebucore/ebucore#wordCount -->

    <owl:DatatypeProperty rdf:about="&ebucore;wordCount">
        <rdfs:label xml:lang="en">Word count</rdfs:label>
        <rdfs:comment xml:lang="en">The number of words contained in a
            document.</rdfs:comment>
        <rdfs:range rdf:resource="&xsd;integer"/>
    </owl:DatatypeProperty>
    


    <!-- http://www.ebu.ch/metadata/ontologies/ebucore/ebucore#wrappingType -->

    <owl:DatatypeProperty rdf:about="&ebucore;wrappingType">
        <rdfs:label xml:lang="en">Wrapping type</rdfs:label>
        <rdfs:comment xml:lang="en">To provide additional information on the
            wrapping type of ancillary data.</rdfs:comment>
        <rdfs:range rdf:resource="&xsd;string"/>
    </owl:DatatypeProperty>
    


    <!-- 
    ///////////////////////////////////////////////////////////////////////////////////////
    //
    // Classes
    //
    ///////////////////////////////////////////////////////////////////////////////////////
     -->

    


    <!-- http://purl.org/dc/elements/1.1/Agent -->

    <owl:Class rdf:about="&dc;Agent">
        <rdfs:label xml:lang="en">Agent</rdfs:label>
        <rdfs:subClassOf rdf:resource="&owl;Thing"/>
        <rdfs:comment xml:lang="en">A resource that acts or has the power to act.</rdfs:comment>
    </owl:Class>
    


    <!-- http://www.bbc.co.uk/ontologies/coreconcepts/Event -->

    <owl:Class rdf:about="&core;Event">
        <rdfs:label xml:lang="en">Event</rdfs:label>
        <rdfs:subClassOf rdf:resource="&ebucore;Event"/>
        <rdfs:comment xml:lang="en">Music events, historic events, sports events, politics events, e.t.c.</rdfs:comment>
    </owl:Class>
    


    <!-- http://www.bbc.co.uk/ontologies/coreconcepts/Organisation -->

    <owl:Class rdf:about="&core;Organisation">
        <rdfs:label xml:lang="en">Organisation</rdfs:label>
        <rdfs:subClassOf rdf:resource="&ebucore;Organisation"/>
        <rdfs:comment xml:lang="en">E.g., Businesses.</rdfs:comment>
    </owl:Class>
    


    <!-- http://www.bbc.co.uk/ontologies/coreconcepts/Person -->

    <owl:Class rdf:about="&core;Person">
        <rdfs:label xml:lang="en">Person</rdfs:label>
        <rdfs:subClassOf rdf:resource="&ebucore;Contact"/>
        <rdfs:comment xml:lang="en">all types of people such as politicians, athletes, historic figures, contributors in programmes e.t.c.</rdfs:comment>
    </owl:Class>
    


    <!-- http://www.bbc.co.uk/ontologies/coreconcepts/Place -->

    <owl:Class rdf:about="&core;Place">
        <rdfs:label xml:lang="en">Place</rdfs:label>
        <rdfs:subClassOf rdf:resource="&ebucore;Location"/>
        <rdfs:comment xml:lang="en">Another type of location.</rdfs:comment>
    </owl:Class>
    


    <!-- http://www.bbc.co.uk/ontologies/coreconcepts/Theme -->

    <owl:Class rdf:about="&core;Theme">
        <rdfs:label xml:lang="en">Theme</rdfs:label>
        <rdfs:subClassOf rdf:resource="&ebucore;Keyword"/>
        <rdfs:comment xml:lang="en">This concept is used to represent intangible things or abstract concepts. For example, Financial Crisis, Midwifery, Happiness.</rdfs:comment>
    </owl:Class>
    


    <!-- http://www.ebu.ch/metadata/ontologies/ebucore/ebucore#AccessConditions -->

    <owl:Class rdf:about="&ebucore;AccessConditions">
        <rdfs:label xml:lang="en">Access conditions</rdfs:label>
        <rdfs:subClassOf rdf:resource="&ebucore;Rights"/>
        <rdfs:comment xml:lang="en">The conditions under which content can be accessed.</rdfs:comment>
    </owl:Class>
    


    <!-- http://www.ebu.ch/metadata/ontologies/ebucore/ebucore#Affiliation -->

    <owl:Class rdf:about="&ebucore;Affiliation">
        <rdfs:label xml:lang="en">Affiliation</rdfs:label>
        <rdfs:subClassOf rdf:resource="&ebucore;Organisation"/>
        <rdfs:comment xml:lang="en">An Organisation to which a Contact is affiliated (with period of validity).</rdfs:comment>
    </owl:Class>
    


    <!-- http://www.ebu.ch/metadata/ontologies/ebucore/ebucore#Agent -->

    <owl:Class rdf:about="&ebucore;Agent">
        <rdfs:label xml:lang="en">Agent</rdfs:label>
        <rdfs:subClassOf rdf:resource="&foaf;Agent"/>
        <rdfs:comment xml:lang="en">A person / contact or organisation contributing
            to the media resource.</rdfs:comment>
    </owl:Class>
    


    <!-- http://www.ebu.ch/metadata/ontologies/ebucore/ebucore#AncillaryData -->

    <owl:Class rdf:about="&ebucore;AncillaryData">
        <rdfs:label xml:lang="en">Ancillary data</rdfs:label>
        <rdfs:subClassOf rdf:resource="&ebucore;DataTrack"/>
        <rdfs:comment xml:lang="en">Any ancillary data provided with the content
            other than captioning and subtitling.</rdfs:comment>
    </owl:Class>
    


    <!-- http://www.ebu.ch/metadata/ontologies/ebucore/ebucore#AncillaryDataFormat -->

    <owl:Class rdf:about="&ebucore;AncillaryDataFormat">
        <rdfs:label xml:lang="en">Ancillary data format</rdfs:label>
        <rdfs:subClassOf rdf:resource="&ebucore;DataFormat"/>
        <rdfs:comment xml:lang="en">To define the format of AncillaryData such as
            legacy data used to be carried in vertical blanking intervals. This is provided as free
            text in an annotation label or as an identifier pointing to a term in a classification
            scheme.</rdfs:comment>
    </owl:Class>
    


    <!-- http://www.ebu.ch/metadata/ontologies/ebucore/ebucore#Annotation -->

    <owl:Class rdf:about="&ebucore;Annotation">
        <rdfs:label xml:lang="en">Annotation</rdfs:label>
        <rdfs:subClassOf rdf:resource="&owl;Thing"/>
        <rdfs:comment xml:lang="en">A set of descriptive or technical metadata.
            Annotation can also be made in the form of a document or media resource such as an or
            video audio file . An annotation can exist on its own and be related / associated to
            other editorial objects or resources.</rdfs:comment>
    </owl:Class>
    


    <!-- http://www.ebu.ch/metadata/ontologies/ebucore/ebucore#Asset -->

    <owl:Class rdf:about="&ebucore;Asset">
        <rdfs:label xml:lang="en">Asset</rdfs:label>
        <rdfs:subClassOf rdf:resource="&owl;Thing"/>
        <rdfs:comment xml:lang="en">The Class &quot;Asset&quot; is an
            object to which an identifier will be associated at commissioning. It will serve as a
            central reference point to manage rights associated to EditorialObjects, Resources,
            MediaResources or Essences, and PublicationEvents (distribution and exploitation
            conditions).</rdfs:comment>
    </owl:Class>
    


    <!-- http://www.ebu.ch/metadata/ontologies/ebucore/ebucore#AudienceRating -->

    <owl:Class rdf:about="&ebucore;AudienceRating">
        <rdfs:label xml:lang="en">Audience rating</rdfs:label>
        <rdfs:subClassOf rdf:resource="&ebucore;Rating"/>
        <rdfs:comment xml:lang="en">The audience by which the Resource can be
            seen according to ratings like MPAA  (http://en.wikipedia.org/wiki/Motion_picture_rating_system) or other organisational / national / local standards.</rdfs:comment>
    </owl:Class>
    


    <!-- http://www.ebu.ch/metadata/ontologies/ebucore/ebucore#AudioChannel -->

    <owl:Class rdf:about="&ebucore;AudioChannel">
        <rdfs:label rdf:datatype="&xsd;string">Audio channel</rdfs:label>
        <rdfs:subClassOf rdf:resource="&ebucore;Essence"/>
        <rdfs:comment rdf:datatype="&xsd;string">An audioChannel represents a single sequence of audio samples. It
				is sub-divided in the time domain into audioBlocks, which is must contain at
				least one of. The typeDefintion of the audioChannel format specifies the type of
				audio it is describing, and also determines which parameters are used within its
				audioBlock children.</rdfs:comment>
    </owl:Class>
    


    <!-- http://www.ebu.ch/metadata/ontologies/ebucore/ebucore#AudioContent -->

    <owl:Class rdf:about="&ebucore;AudioContent">
        <rdfs:label xml:lang="en">Audio content</rdfs:label>
        <rdfs:subClassOf rdf:resource="&ebucore;AudioProgramme"/>
        <rdfs:comment xml:lang="en">An audioContent defines one component of a programme (e.g. background
				music), its association with an audioGroup (e.g. a 2.0 audioPackFormat of
				audioChannelFormats for stereo reproduction), its association with an
				audioStreamFormat, and its set of loudness parameters.</rdfs:comment>
    </owl:Class>
    


    <!-- http://www.ebu.ch/metadata/ontologies/ebucore/ebucore#AudioEncodingFormat -->

    <owl:Class rdf:about="&ebucore;AudioEncodingFormat">
        <rdfs:label xml:lang="en">Audio encoding format</rdfs:label>
        <rdfs:subClassOf rdf:resource="&ebucore;EncodingFormat"/>
        <rdfs:comment xml:lang="en">The encoding format for the audio.</rdfs:comment>
    </owl:Class>
    


    <!-- http://www.ebu.ch/metadata/ontologies/ebucore/ebucore#AudioFormat -->

    <owl:Class rdf:about="&ebucore;AudioFormat">
        <rdfs:label xml:lang="en">Audio Format</rdfs:label>
        <rdfs:subClassOf rdf:resource="&ebucore;Format"/>
        <rdfs:comment xml:lang="en">The technical characteristics of an
            AudioResource such as the sampleRate. This is provided as free text in an annotation
            label or as an identifier pointing to a term in a classification scheme e.g.
            http://www.ebu.ch/metadata/ontologies/skos/ebu_AudioFormatCodeCS.rdf.</rdfs:comment>
    </owl:Class>
    


    <!-- http://www.ebu.ch/metadata/ontologies/ebucore/ebucore#AudioPackFormat -->

    <owl:Class rdf:about="&ebucore;AudioPackFormat">
        <rdfs:label xml:lang="en">Audio pack format</rdfs:label>
        <rdfs:subClassOf rdf:resource="&ebucore;AudioFormat"/>
        <rdfs:comment xml:lang="en">The format of an AudioPack. Examples of audioPackFormats are &apos;stereo&apos; and &apos;5.1&apos; for channel-based formats.</rdfs:comment>
    </owl:Class>
    


    <!-- http://www.ebu.ch/metadata/ontologies/ebucore/ebucore#AudioProgramme -->

    <owl:Class rdf:about="&ebucore;AudioProgramme">
        <rdfs:label xml:lang="en">Audio programme</rdfs:label>
        <rdfs:subClassOf rdf:resource="&ebucore;Programme"/>
        <rdfs:comment xml:lang="en">A set of one or more audioContent that derive from the same material,
				i.e. an audioMultiplex, and the definition of its multiplexed audioContents (e.g.
				foreground and commentary, background music).</rdfs:comment>
    </owl:Class>
    


    <!-- http://www.ebu.ch/metadata/ontologies/ebucore/ebucore#AudioStream -->

    <owl:Class rdf:about="&ebucore;AudioStream">
        <rdfs:label xml:lang="en">Audio stream</rdfs:label>
        <rdfs:subClassOf rdf:resource="&ebucore;Stream"/>
        <rdfs:comment xml:lang="en">An audioStreamFormat describes a decodable signal - PCM signal or a Dolby E stream for example. It is composed of one or more AudioTracks.</rdfs:comment>
    </owl:Class>
    


    <!-- http://www.ebu.ch/metadata/ontologies/ebucore/ebucore#AudioStreamFormat -->

    <owl:Class rdf:about="&ebucore;AudioStreamFormat">
        <rdfs:label xml:lang="en">Audio stream format</rdfs:label>
        <rdfs:subClassOf rdf:resource="&ebucore;AudioFormat"/>
        <rdfs:comment xml:lang="en">The format of an AudioStream, e.g. PCM_FrontLeft or Dolby E.</rdfs:comment>
    </owl:Class>
    


    <!-- http://www.ebu.ch/metadata/ontologies/ebucore/ebucore#AudioTrack -->

    <owl:Class rdf:about="&ebucore;AudioTrack">
        <rdfs:label xml:lang="en">Audio track</rdfs:label>
        <rdfs:subClassOf rdf:resource="&ebucore;Track"/>
        <rdfs:comment xml:lang="en">An audioTrack is the basic audio data container of a medium. Attribute is
				an unambiguous reference to this container in a given medium.</rdfs:comment>
        <rdfs:comment xml:lang="en">An audioTrack object defines a component of an audioStream.
				A single set of samples or data in the storage medium.</rdfs:comment>
        <rdfs:comment xml:lang="en">Represents a physical container or carrier to hold an audio stream. This
				should be usually defined by many attributes such as ID, format (e.g. 48 kHz/24
				bits), linkage information (e.g. odd/even)</rdfs:comment>
    </owl:Class>
    


    <!-- http://www.ebu.ch/metadata/ontologies/ebucore/ebucore#AudioTrackFormat -->

    <owl:Class rdf:about="&ebucore;AudioTrackFormat">
        <rdfs:label xml:lang="en">Audio track format</rdfs:label>
        <rdfs:subClassOf rdf:resource="&ebucore;AudioFormat"/>
        <rdfs:comment xml:lang="en">The format of an AudioTrack e.g. PCM_FrontLeft.</rdfs:comment>
    </owl:Class>
    


    <!-- http://www.ebu.ch/metadata/ontologies/ebucore/ebucore#Brand -->

    <owl:Class rdf:about="&ebucore;Brand">
        <rdfs:label rdf:datatype="&xsd;string">Brand</rdfs:label>
        <rdfs:subClassOf rdf:resource="&ebucore;Group"/>
        <rdfs:comment rdf:datatype="&xsd;string">A group of EditorialObjects having a Brand as a
            common denominator</rdfs:comment>
    </owl:Class>
    


    <!-- http://www.ebu.ch/metadata/ontologies/ebucore/ebucore#BusinessObject -->

    <owl:Class rdf:about="&ebucore;BusinessObject">
        <rdfs:label xml:lang="en">Business Object</rdfs:label>
        <rdfs:subClassOf rdf:resource="&owl;Thing"/>
        <rdfs:comment xml:lang="en">An image, a document, an annotation
            (descriptive textual metadata or audio/video tag), a tag (time related in audiovisual
            media resources), or an audiovisual media resource (optionally composed of one or more
            fragment / part and / or audio, video data tracks). Other types of BusinessObjects may
            be defined as subclasses.</rdfs:comment>
    </owl:Class>
    


    <!-- http://www.ebu.ch/metadata/ontologies/ebucore/ebucore#Captioning -->

    <owl:Class rdf:about="&ebucore;Captioning">
        <rdfs:label xml:lang="en">Captioning</rdfs:label>
        <rdfs:subClassOf rdf:resource="&ebucore;DataTrack"/>
        <rdfs:comment xml:lang="en">To signal the presence of hard of hearing
            captioning.</rdfs:comment>
    </owl:Class>
    


    <!-- http://www.ebu.ch/metadata/ontologies/ebucore/ebucore#CaptioningFormat -->

    <owl:Class rdf:about="&ebucore;CaptioningFormat">
        <rdfs:label xml:lang="en">Captioning format</rdfs:label>
        <rdfs:subClassOf rdf:resource="&ebucore;DataFormat"/>
        <rdfs:comment xml:lang="en">To define the format of captioning.
            Captioning&apos;s main use isfor hard of hearing transcription. This is provided as
            free text in an annotation label or as an identifier pointing to a term in a
            classification scheme.</rdfs:comment>
    </owl:Class>
    


    <!-- http://www.ebu.ch/metadata/ontologies/ebucore/ebucore#Cast -->

    <owl:Class rdf:about="&ebucore;Cast">
        <rdfs:label xml:lang="en">Cast member</rdfs:label>
        <rdfs:subClassOf rdf:resource="&ebucore;Agent"/>
        <rdfs:comment xml:lang="en">A member of the cast list (a list of fictitious
            characters).</rdfs:comment>
    </owl:Class>
    


    <!-- http://www.ebu.ch/metadata/ontologies/ebucore/ebucore#Character -->

    <owl:Class rdf:about="&ebucore;Character">
        <rdfs:label xml:lang="en">Character</rdfs:label>
        <rdfs:subClassOf rdf:resource="&ebucore;Agent"/>
        <rdfs:comment xml:lang="en">A fictitious contact / person.</rdfs:comment>
    </owl:Class>
    


    <!-- http://www.ebu.ch/metadata/ontologies/ebucore/ebucore#ClosedCaptions -->

    <owl:Class rdf:about="&ebucore;ClosedCaptions">
        <rdfs:label xml:lang="en">Closed caption</rdfs:label>
        <rdfs:subClassOf rdf:resource="&ebucore;Captioning"/>
        <rdfs:comment xml:lang="en">Closed captioning is provided as separate
            content.</rdfs:comment>
    </owl:Class>
    


    <!-- http://www.ebu.ch/metadata/ontologies/ebucore/ebucore#ClosedSubtitling -->

    <owl:Class rdf:about="&ebucore;ClosedSubtitling">
        <rdfs:label xml:lang="en">Closed subtitling</rdfs:label>
        <rdfs:subClassOf rdf:resource="&ebucore;Subtitling"/>
        <rdfs:comment xml:lang="en">Closed subtitles are provided as separate
            content.</rdfs:comment>
    </owl:Class>
    


    <!-- http://www.ebu.ch/metadata/ontologies/ebucore/ebucore#Codec -->

    <owl:Class rdf:about="&ebucore;Codec">
        <rdfs:label xml:lang="en">Codec</rdfs:label>
        <rdfs:subClassOf rdf:resource="&skos;Concept"/>
        <rdfs:comment xml:lang="en">To provide information on a codec.</rdfs:comment>
    </owl:Class>
    


    <!-- http://www.ebu.ch/metadata/ontologies/ebucore/ebucore#Collection -->

    <owl:Class rdf:about="&ebucore;Collection">
        <rdfs:label rdf:datatype="&xsd;string">Collection</rdfs:label>
        <rdfs:subClassOf rdf:resource="&ebucore;Group"/>
        <rdfs:comment rdf:datatype="&xsd;string">A group of EditorialObjects. There can be many
            types of collections for which specific sub-classes should be defined. In the worl of
            archives, A collection corresponds to all items belonging to an individual /
            collector.</rdfs:comment>
    </owl:Class>
    


    <!-- http://www.ebu.ch/metadata/ontologies/ebucore/ebucore#ColourSpace -->

    <owl:Class rdf:about="&ebucore;ColourSpace">
        <rdfs:label xml:lang="en">Colour space</rdfs:label>
        <rdfs:subClassOf rdf:resource="&ebucore;Format"/>
        <rdfs:comment xml:lang="en">The CoulourSpace of a VideoResource. A
            ColourSpace is defined as free text in an annotation label or as an identifier pointing
            to a term in a classification scheme such as
            http://www.ebu.ch/metadata/ontologies/skos/ebu_ColourCodeCS.rdf.</rdfs:comment>
    </owl:Class>
    


    <!-- http://www.ebu.ch/metadata/ontologies/ebucore/ebucore#Component -->

    <owl:Class rdf:about="&ebucore;Component">
        <rdfs:label xml:lang="en">Component</rdfs:label>
        <rdfs:subClassOf rdf:resource="&ebucore;Essence"/>
        <rdfs:comment xml:lang="en">A component e.g. audio, video, data or else or a MediaResource or Essence.</rdfs:comment>
    </owl:Class>
    


    <!-- http://www.ebu.ch/metadata/ontologies/ebucore/ebucore#Contact -->

    <owl:Class rdf:about="&ebucore;Contact">
        <rdfs:label xml:lang="en">Contact</rdfs:label>
        <rdfs:subClassOf rdf:resource="&ebucore;Agent"/>
        <rdfs:comment xml:lang="en">A physical person.</rdfs:comment>
    </owl:Class>
    


    <!-- http://www.ebu.ch/metadata/ontologies/ebucore/ebucore#ContainerFormat -->

    <owl:Class rdf:about="&ebucore;ContainerFormat">
        <rdfs:label xml:lang="en">Container format</rdfs:label>
        <rdfs:subClassOf rdf:resource="&ebucore;Format"/>
        <rdfs:comment xml:lang="en">The container or wrapper format used to package
            audio, video and data components of a Mediaresource. The format is defined as free text
            or pointing at a term in a classification scheme e.g.
            http://www.ebu.ch/metadata/ontologies/skos/ebu_ContainerFormatCS.rdf.</rdfs:comment>
    </owl:Class>
    


    <!-- http://www.ebu.ch/metadata/ontologies/ebucore/ebucore#ContainerMimeType -->

    <owl:Class rdf:about="&ebucore;ContainerMimeType">
        <rdfs:label xml:lang="en">Container Mime type</rdfs:label>
        <rdfs:subClassOf rdf:resource="&ebucore;Format"/>
        <rdfs:comment xml:lang="en">The definition of the container if available as
            a MIME type. This is provided as free text in an annotation label or as an identifier
            pointing to a term in a classification scheme. For more information:
            http://www.iana.org/assignments/media-types/application/index.html.</rdfs:comment>
    </owl:Class>
    


    <!-- http://www.ebu.ch/metadata/ontologies/ebucore/ebucore#Copyright -->

    <owl:Class rdf:about="&ebucore;Copyright">
        <rdfs:label xml:lang="en">Copyright</rdfs:label>
        <rdfs:subClassOf rdf:resource="&ebucore;Rights"/>
        <rdfs:comment xml:lang="en">To provide a copyright
            statement.</rdfs:comment>
    </owl:Class>
    


    <!-- http://www.ebu.ch/metadata/ontologies/ebucore/ebucore#CoverageRestrictions -->

    <owl:Class rdf:about="&ebucore;CoverageRestrictions">
        <rdfs:label xml:lang="en">Coverage restrictions</rdfs:label>
        <rdfs:subClassOf rdf:resource="&ebucore;Rights"/>
        <rdfs:comment xml:lang="en">To provide information on possible restrictions
            regarding the temporal and spatial coverage for publication.</rdfs:comment>
    </owl:Class>
    


    <!-- http://www.ebu.ch/metadata/ontologies/ebucore/ebucore#DataFormat -->

    <owl:Class rdf:about="&ebucore;DataFormat">
        <rdfs:label xml:lang="en">Data format</rdfs:label>
        <rdfs:subClassOf rdf:resource="&ebucore;Format"/>
        <rdfs:comment xml:lang="en">To provide addtional technical information on
            the characteristics of data streams in a MediaResource including but not limited to
            AncillaryData, Subtilting and Captioning. Additional specific data format may be defined
            as subclasses of DataFormat.</rdfs:comment>
    </owl:Class>
    


    <!-- http://www.ebu.ch/metadata/ontologies/ebucore/ebucore#DataTrack -->

    <owl:Class rdf:about="&ebucore;DataTrack">
        <rdfs:label xml:lang="en">Data track</rdfs:label>
        <rdfs:subClassOf rdf:resource="&ebucore;Track"/>
        <rdfs:comment xml:lang="en">Ancillary data track e.g. captioning&quot;
            or &quot;subtitling&quot; in addition to video and audio tracks.</rdfs:comment>
    </owl:Class>
    


    <!-- http://www.ebu.ch/metadata/ontologies/ebucore/ebucore#Department -->

    <owl:Class rdf:about="&ebucore;Department">
        <rdfs:label xml:lang="en">Department</rdfs:label>
        <rdfs:subClassOf rdf:resource="&ebucore;Organisation"/>
        <rdfs:comment xml:lang="en">A department within and
            organisation.</rdfs:comment>
    </owl:Class>
    


    <!-- http://www.ebu.ch/metadata/ontologies/ebucore/ebucore#DepictedEvent -->

    <owl:Class rdf:about="&ebucore;DepictedEvent">
        <rdfs:label xml:lang="en">Depicted Event</rdfs:label>
        <rdfs:subClassOf rdf:resource="&core;Event"/>
        <rdfs:comment xml:lang="en">A DepictedEVent is fictitious or historical or
            other sort of Event that the content of the BusinessObject or resource relates
            to.</rdfs:comment>
    </owl:Class>
    


    <!-- http://www.ebu.ch/metadata/ontologies/ebucore/ebucore#Disclaimer -->

    <owl:Class rdf:about="&ebucore;Disclaimer">
        <rdfs:label xml:lang="en">Disclaimer</rdfs:label>
        <rdfs:subClassOf rdf:resource="&ebucore;Rights"/>
        <rdfs:comment xml:lang="en">To provide a disclaimer of any
            form.</rdfs:comment>
    </owl:Class>
    


    <!-- http://www.ebu.ch/metadata/ontologies/ebucore/ebucore#Document -->

    <owl:Class rdf:about="&ebucore;Document">
        <rdfs:label xml:lang="en">Document</rdfs:label>
        <rdfs:subClassOf rdf:resource="&ebucore;Resource"/>
        <rdfs:comment xml:lang="en">To describe a publication in the form of a
            document e.g. a html webpage (news item) or a pdf document e.g. a script.</rdfs:comment>
    </owl:Class>
    


    <!-- http://www.ebu.ch/metadata/ontologies/ebucore/ebucore#DocumentFormat -->

    <owl:Class rdf:about="&ebucore;DocumentFormat">
        <rdfs:label xml:lang="en">Document format</rdfs:label>
        <rdfs:subClassOf rdf:resource="&ebucore;Format"/>
        <rdfs:comment xml:lang="en">To provide technical information about the
            format of a document such as the orientation. This is provided as free text in an
            annotation label or as an identifier pointing to a term in a classification
            scheme.</rdfs:comment>
    </owl:Class>
    


    <!-- http://www.ebu.ch/metadata/ontologies/ebucore/ebucore#Dopesheet -->

    <owl:Class rdf:about="&ebucore;Dopesheet">
        <rdfs:label xml:lang="en">Dopesheet</rdfs:label>
        <rdfs:subClassOf rdf:resource="&ebucore;Document"/>
        <rdfs:comment xml:lang="en">Provides additional information about a NewsItem, e.g. date and place, subject.</rdfs:comment>
    </owl:Class>
    


    <!-- http://www.ebu.ch/metadata/ontologies/ebucore/ebucore#EditorialObject -->

    <owl:Class rdf:about="&ebucore;EditorialObject">
        <rdfs:label xml:lang="en">Editorial Object</rdfs:label>
        <rdfs:subClassOf rdf:resource="&ebucore;BusinessObject"/>
        <rdfs:comment xml:lang="en">In the audiovisual domain, the Class
            EditorialObject transforms a commissioned concept into an editorial definition of a
            MediaResource before fabrication (in the Production Domain) and Distribution (in the
            Distribution Domain). An EditorialObject is a set of descriptive metadata summarising
            e.g. editing decisions. An EditorialObject can also be a part of an EditorialObject,
            which is defined by its start time and duration. An EditorialObject can also be a group
            of EditorialObjects. For example a series composed of episodes is defined as an
            EditorialObject.</rdfs:comment>
    </owl:Class>
    


    <!-- http://www.ebu.ch/metadata/ontologies/ebucore/ebucore#EncodingFormat -->

    <owl:Class rdf:about="&ebucore;EncodingFormat">
        <rdfs:label xml:lang="en">Encoding</rdfs:label>
        <rdfs:subClassOf rdf:resource="&ebucore;Format"/>
        <rdfs:comment xml:lang="en">To provide a definition of the encoding format
            for audio and video. This is provided as free text in an annotation label or as an
            identifier pointing to a term in a classification scheme e.g.
            http://www.ebu.ch/metadata/ontologies/skos/ebu_AudioCompressionCodeCS.rdf or
            http://www.ebu.ch/metadata/ontologies/skos/ebu_VideoCompressionCodeCS.rdf.</rdfs:comment>
    </owl:Class>
    


    <!-- http://www.ebu.ch/metadata/ontologies/ebucore/ebucore#Essence -->

    <owl:Class rdf:about="&ebucore;Essence">
        <rdfs:label xml:lang="en">Essence</rdfs:label>
        <rdfs:subClassOf rdf:resource="&ebucore;MediaResource"/>
        <rdfs:comment xml:lang="en">In some audiovisual standardisation groups,
            Essence is preferred to MediaResource. In also has subclasses well known as MediaObject
            clustered in AudioObjects and VideoObjects.</rdfs:comment>
    </owl:Class>
    


    <!-- http://www.ebu.ch/metadata/ontologies/ebucore/ebucore#Event -->

    <owl:Class rdf:about="&ebucore;Event">
        <rdfs:label xml:lang="en">Event</rdfs:label>
        <rdfs:subClassOf rdf:resource="&owl;Thing"/>
        <rdfs:comment xml:lang="en">Additional types of event shall be defined as
            new sub-classes of event.</rdfs:comment>
        <rdfs:comment xml:lang="en">An event related to the media resource, e.g.
            depicted in the resource (possibly fictional), etc.</rdfs:comment>
    </owl:Class>
    


    <!-- http://www.ebu.ch/metadata/ontologies/ebucore/ebucore#ExploitationIssues -->

    <owl:Class rdf:about="&ebucore;ExploitationIssues">
        <rdfs:label xml:lang="en">Exploitation issues</rdfs:label>
        <rdfs:subClassOf rdf:resource="&ebucore;Rights"/>
        <rdfs:comment xml:lang="en">To highlight potential exploitation
            issues.</rdfs:comment>
    </owl:Class>
    


    <!-- http://www.ebu.ch/metadata/ontologies/ebucore/ebucore#FileFormat -->

    <owl:Class rdf:about="&ebucore;FileFormat">
        <rdfs:label xml:lang="en">File format</rdfs:label>
        <rdfs:subClassOf rdf:resource="&ebucore;Format"/>
        <rdfs:comment xml:lang="en">A file format for Resources other than
            audiovisual resources. The format is defined as free text or pointing at a term in a
            classification scheme e.g.
            http://www.ebu.ch/metadata/ontologies/skos/ebu_FileFormatCS.rdf.</rdfs:comment>
    </owl:Class>
    


    <!-- http://www.ebu.ch/metadata/ontologies/ebucore/ebucore#Format -->

    <owl:Class rdf:about="&ebucore;Format">
        <rdfs:label xml:lang="en">Format</rdfs:label>
        <rdfs:subClassOf rdf:resource="&skos;Concept"/>
        <rdfs:comment xml:lang="en">The format provides technical information on
            the format of a Resource. A BusinessObject can be instantiated in a variety of Resources
            each in a particular Format. Other specific data formats may be defined as subclasses of
            format.</rdfs:comment>
    </owl:Class>
    


    <!-- http://www.ebu.ch/metadata/ontologies/ebucore/ebucore#Genre -->

    <owl:Class rdf:about="&ebucore;Genre">
        <rdfs:label xml:lang="en">Genre</rdfs:label>
        <rdfs:subClassOf rdf:resource="&ebucore;Type"/>
        <rdfs:comment xml:lang="en">This class shall be used to provide information
            on the genre of the BusinessObject or Resource. This is provided as free text in an
            annotation label or as an identifier pointing to a term in a classification scheme e.g.
            http://www.ebu.ch/metadata/ontologies/skos/ebu_ContentGenreCS.rdf or
            http://www.ebu.ch/metadata/ontologies/skos/ebu_EditorialFormatCodeCS.rdf.</rdfs:comment>
    </owl:Class>
    


    <!-- http://www.ebu.ch/metadata/ontologies/ebucore/ebucore#Group -->

    <owl:Class rdf:about="&ebucore;Group">
        <rdfs:label xml:lang="en">Group</rdfs:label>
        <rdfs:subClassOf rdf:resource="&ebucore;EditorialObject"/>
        <rdfs:comment xml:lang="en">To define a collection / group of media
            resources, for example a series made of episodes.</rdfs:comment>
    </owl:Class>
    


    <!-- http://www.ebu.ch/metadata/ontologies/ebucore/ebucore#IPRRestrictions -->

    <owl:Class rdf:about="&ebucore;IPRRestrictions">
        <rdfs:label xml:lang="en">IPR restrictions</rdfs:label>
        <rdfs:subClassOf rdf:resource="&ebucore;Rights"/>
        <rdfs:comment xml:lang="en">To provide information on intellectual
            property.</rdfs:comment>
    </owl:Class>
    


    <!-- http://www.ebu.ch/metadata/ontologies/ebucore/ebucore#Image -->

    <owl:Class rdf:about="&ebucore;Image">
        <rdfs:label rdf:datatype="&xsd;string">Image</rdfs:label>
        <rdfs:subClassOf rdf:resource="&ebucore;BusinessObject"/>
        <rdfs:comment rdf:datatype="&xsd;string">A still image / thumbnail / key frame / logo
            related to the media resource or being the media resource itself</rdfs:comment>
    </owl:Class>
    


    <!-- http://www.ebu.ch/metadata/ontologies/ebucore/ebucore#ImageFormat -->

    <owl:Class rdf:about="&ebucore;ImageFormat">
        <rdfs:label xml:lang="en">Image format</rdfs:label>
        <rdfs:subClassOf rdf:resource="&ebucore;Format"/>
        <rdfs:comment xml:lang="en">To provide technical information about the
            format of an image such as the orientation. This is provided as free text in an
            annotation label or as an identifier pointing to a term in a classification
            scheme.</rdfs:comment>
    </owl:Class>
    


    <!-- http://www.ebu.ch/metadata/ontologies/ebucore/ebucore#Item -->

    <owl:Class rdf:about="&ebucore;Item">
        <rdfs:label xml:lang="en">Item</rdfs:label>
        <rdfs:subClassOf rdf:resource="&ebucore;EditorialObject"/>
        <rdfs:comment xml:lang="en">An item e.g. newsItem or sportItem</rdfs:comment>
    </owl:Class>
    


    <!-- http://www.ebu.ch/metadata/ontologies/ebucore/ebucore#KeyCareerEvent -->

    <owl:Class rdf:about="&ebucore;KeyCareerEvent">
        <rdfs:label rdf:datatype="&xsd;string">Key career event</rdfs:label>
        <rdfs:subClassOf rdf:resource="&ebucore;KeyEvent"/>
    </owl:Class>
    


    <!-- http://www.ebu.ch/metadata/ontologies/ebucore/ebucore#KeyEvent -->

    <owl:Class rdf:about="&ebucore;KeyEvent">
        <rdfs:label rdf:datatype="&xsd;string">Key event</rdfs:label>
        <rdfs:subClassOf rdf:resource="&core;Event"/>
    </owl:Class>
    


    <!-- http://www.ebu.ch/metadata/ontologies/ebucore/ebucore#KeyPersonalEvent -->

    <owl:Class rdf:about="&ebucore;KeyPersonalEvent">
        <rdfs:label rdf:datatype="&xsd;string">Key personal event</rdfs:label>
        <rdfs:subClassOf rdf:resource="&ebucore;KeyEvent"/>
    </owl:Class>
    


    <!-- http://www.ebu.ch/metadata/ontologies/ebucore/ebucore#Keyframe -->

    <owl:Class rdf:about="&ebucore;Keyframe">
        <rdfs:label xml:lang="en">key frame</rdfs:label>
        <rdfs:subClassOf rdf:resource="&ebucore;Picture"/>
        <rdfs:comment xml:lang="en">A key frame is a frame extarcted from video,
            e.g. representative of a part of a MediaResource.</rdfs:comment>
    </owl:Class>
    


    <!-- http://www.ebu.ch/metadata/ontologies/ebucore/ebucore#Keyword -->

    <owl:Class rdf:about="&ebucore;Keyword">
        <rdfs:label xml:lang="en">Keyword</rdfs:label>
        <rdfs:subClassOf rdf:resource="&skos;Concept"/>
        <rdfs:comment xml:lang="en">To proivde keywords and define key concepts
            illustrating the content of the Resource or EditorialObject. This is provided as free
            text in an annotation label or as an identifier pointing to a term in a classification
            scheme.</rdfs:comment>
    </owl:Class>
    


    <!-- http://www.ebu.ch/metadata/ontologies/ebucore/ebucore#Language -->

    <owl:Class rdf:about="&ebucore;Language">
        <rdfs:label xml:lang="en">Language</rdfs:label>
        <rdfs:subClassOf rdf:resource="&skos;Concept"/>
        <rdfs:comment xml:lang="en">To provide information on languages present in
            the BusinessObject and its purpose. This is provided as free text in an annotation label
            or as an identifier pointing to a term in a classification scheme.Other language
            specific types may be added as subclasses of language.</rdfs:comment>
    </owl:Class>
    


    <!-- http://www.ebu.ch/metadata/ontologies/ebucore/ebucore#Location -->

    <owl:Class rdf:about="&ebucore;Location">
        <rdfs:label rdf:datatype="&xsd;string">Location</rdfs:label>
        <rdfs:subClassOf rdf:resource="&owl;Thing"/>
        <rdfs:comment xml:lang="en">A location related to the media resource, e.g.
            depicted in the resource (possibly fictional) or where the resource was created
            (shooting location), etc.</rdfs:comment>
        <rdfs:comment xml:lang="en">A type of location is defined as a sub-class of 
            location.</rdfs:comment>
        <rdfs:comment xml:lang="en">This is provided as free text in an annotation
            label or as an identifier pointing to a term in a classification scheme.</rdfs:comment>
    </owl:Class>
    


    <!-- http://www.ebu.ch/metadata/ontologies/ebucore/ebucore#Logo -->

    <owl:Class rdf:about="&ebucore;Logo">
        <rdfs:label xml:lang="en">Logo</rdfs:label>
        <rdfs:subClassOf rdf:resource="&ebucore;Picture"/>
        <rdfs:comment xml:lang="en">A Logo allows to visually identify an
            organisation, publicationService, publicationChannel, or ratings /
            parentalGuidance</rdfs:comment>
    </owl:Class>
    


    <!-- http://www.ebu.ch/metadata/ontologies/ebucore/ebucore#MediaFragment -->

    <owl:Class rdf:about="&ebucore;MediaFragment">
        <rdfs:label xml:lang="en">Media Fragment</rdfs:label>
        <rdfs:subClassOf rdf:resource="&ebucore;MediaResource"/>
        <rdfs:comment xml:lang="en">A MediaFragment is a temporal or spatial segment of a resource identified by a MediaGragment URI (http://www.w3.org/2008/WebVideo/Fragments/WD-media-fragments-spec/).</rdfs:comment>
    </owl:Class>
    


    <!-- http://www.ebu.ch/metadata/ontologies/ebucore/ebucore#MediaResource -->

    <owl:Class rdf:about="&ebucore;MediaResource">
        <rdfs:label xml:lang="en">Media Resource</rdfs:label>
        <rdfs:subClassOf rdf:resource="&ebucore;Resource"/>
        <rdfs:comment xml:lang="en">The use of MediaResource is reserved to
            audiovisual content.</rdfs:comment>
    </owl:Class>
    


    <!-- http://www.ebu.ch/metadata/ontologies/ebucore/ebucore#Medium -->

    <owl:Class rdf:about="&ebucore;Medium">
        <rdfs:label xml:lang="en">Medium</rdfs:label>
        <rdfs:subClassOf rdf:resource="&ebucore;Format"/>
        <rdfs:comment xml:lang="en">To provide information on the medium formats in
            which the resource is available. This is provided as free text in an annotation label or
            as an identifier pointing to a term in a classification scheme.</rdfs:comment>
    </owl:Class>
    


    <!-- http://www.ebu.ch/metadata/ontologies/ebucore/ebucore#MetadataTrack -->

    <owl:Class rdf:about="&ebucore;MetadataTrack">
        <rdfs:label rdf:datatype="&xsd;string">Metadata track</rdfs:label>
        <rdfs:subClassOf rdf:resource="&ebucore;Track"/>
        <skos:prefLabel rdf:datatype="&xsd;string">Metadata track</skos:prefLabel>
    </owl:Class>
    


    <!-- http://www.ebu.ch/metadata/ontologies/ebucore/ebucore#MimeType -->

    <owl:Class rdf:about="&ebucore;MimeType">
        <rdfs:label xml:lang="en">Mime type</rdfs:label>
        <rdfs:subClassOf rdf:resource="&ebucore;Format"/>
        <rdfs:comment xml:lang="en">The definition of the container if available as
            a MIME type. This is provided as free text in an annotation label or as an identifier
            pointing to a term in a classification scheme. For more information:
            http://www.iana.org/assignments/media-types/index.html.</rdfs:comment>
    </owl:Class>
    


    <!-- http://www.ebu.ch/metadata/ontologies/ebucore/ebucore#NewsItem -->

    <owl:Class rdf:about="&ebucore;NewsItem">
        <rdfs:label xml:lang="en">News Item</rdfs:label>
        <rdfs:subClassOf rdf:resource="&ebucore;Item"/>
        <rdfs:comment xml:lang="en">A NewsItem aggregates all information about a particular news event.</rdfs:comment>
    </owl:Class>
    


    <!-- http://www.ebu.ch/metadata/ontologies/ebucore/ebucore#ObjectType -->

    <owl:Class rdf:about="&ebucore;ObjectType">
        <rdfs:label xml:lang="en">Object type</rdfs:label>
        <rdfs:subClassOf rdf:resource="&ebucore;Type"/>
        <rdfs:comment xml:lang="en">To specify the type of BusinessObject e.g. and
            EditorialObject of type &quot;programme&quot; or clip&quot;. This is
            provided as free text in an annotation label or as an identifier pointing to a term in a
            classification scheme e.g.
            http://www.ebu.ch/metadata/ontologies/skos/ebu_ObjectTypeCodeCS.rdf.</rdfs:comment>
    </owl:Class>
    


    <!-- http://www.ebu.ch/metadata/ontologies/ebucore/ebucore#OpenCaptions -->

    <owl:Class rdf:about="&ebucore;OpenCaptions">
        <rdfs:label xml:lang="en">Open captions</rdfs:label>
        <rdfs:subClassOf rdf:resource="&ebucore;Captioning"/>
        <rdfs:comment xml:lang="en">Open Captions are burned in the
            image.</rdfs:comment>
    </owl:Class>
    


    <!-- http://www.ebu.ch/metadata/ontologies/ebucore/ebucore#OpenSubtitling -->

    <owl:Class rdf:about="&ebucore;OpenSubtitling">
        <rdfs:label xml:lang="en">Open subtitling</rdfs:label>
        <rdfs:subClassOf rdf:resource="&ebucore;Subtitling"/>
        <rdfs:comment xml:lang="en">Open subtitles are burned in the
            image.</rdfs:comment>
    </owl:Class>
    


    <!-- http://www.ebu.ch/metadata/ontologies/ebucore/ebucore#Organisation -->

    <owl:Class rdf:about="&ebucore;Organisation">
        <rdfs:label xml:lang="en">Organisation</rdfs:label>
        <rdfs:subClassOf rdf:resource="&ebucore;Agent"/>
        <rdfs:comment xml:lang="en">An organisation (business, corporation, federation, etc.) or moral agent (gvernment body).</rdfs:comment>
    </owl:Class>
    


    <!-- http://www.ebu.ch/metadata/ontologies/ebucore/ebucore#OriginalLanguage -->

    <owl:Class rdf:about="&ebucore;OriginalLanguage">
        <rdfs:subClassOf rdf:resource="&ebucore;Language"/>
        <rdfs:comment rdf:datatype="&xsd;string">The original language in which the
            BusinessObject or Resource has been created and released. This is provided as free text
            in an annotation label or as an identifier pointing to a term in a classification
            scheme.</rdfs:comment>
    </owl:Class>
    


    <!-- http://www.ebu.ch/metadata/ontologies/ebucore/ebucore#Part -->

    <owl:Class rdf:about="&ebucore;Part">
        <rdfs:label xml:lang="en">Part, Fragment, Segment</rdfs:label>
        <rdfs:subClassOf rdf:resource="&ebucore;EditorialObject"/>
        <rdfs:comment xml:lang="en">A Fragment is a particular section of a
            MediaResource identified by a start and end time or duration. Fragment can also be
            called segment or part.</rdfs:comment>
        <rdfs:comment xml:lang="en">One of more media fragment (audio, video, data)
            composing an audiovisual media resource. In other ontolgies fragment is often referred
            to e.g. as a &apos;part&apos; or &apos;segment&apos; or
            &apos;fragment&apos;.</rdfs:comment>
    </owl:Class>
    


    <!-- http://www.ebu.ch/metadata/ontologies/ebucore/ebucore#Pictogram -->

    <owl:Class rdf:about="&ebucore;Pictogram">
        <rdfs:label xml:lang="en">Pictogram</rdfs:label>
        <rdfs:subClassOf rdf:resource="&ebucore;Picture"/>
        <rdfs:comment xml:lang="en">A visual / graphical representation of a concept.</rdfs:comment>
    </owl:Class>
    


    <!-- http://www.ebu.ch/metadata/ontologies/ebucore/ebucore#Picture -->

    <owl:Class rdf:about="&ebucore;Picture">
        <rdfs:label xml:lang="en">Picture</rdfs:label>
        <rdfs:subClassOf rdf:resource="&ebucore;Resource"/>
        <rdfs:comment xml:lang="en">A photography, a logo, a pictogram, etc.</rdfs:comment>
    </owl:Class>
    


    <!-- http://www.ebu.ch/metadata/ontologies/ebucore/ebucore#Programme -->

    <owl:Class rdf:about="&ebucore;Programme">
        <rdfs:label xml:lang="en">Programme</rdfs:label>
        <rdfs:subClassOf rdf:resource="&ebucore;EditorialObject"/>
        <rdfs:comment xml:lang="en">An EditorialObject corresponding to a
            MediaResource ready for publication.</rdfs:comment>
    </owl:Class>
    


    <!-- http://www.ebu.ch/metadata/ontologies/ebucore/ebucore#PublicationChannel -->

    <owl:Class rdf:about="&ebucore;PublicationChannel">
        <rdfs:label xml:lang="en">Publication Channel</rdfs:label>
        <rdfs:subClassOf rdf:resource="&owl;Thing"/>
        <rdfs:comment xml:lang="en">The name of the channel through which a
            Resource has been published as a PublicationEvent. A PublicationChannel can use a
            variety of medias e.g. broadcast or online.</rdfs:comment>
    </owl:Class>
    


    <!-- http://www.ebu.ch/metadata/ontologies/ebucore/ebucore#PublicationEvent -->

    <owl:Class rdf:about="&ebucore;PublicationEvent">
        <rdfs:label xml:lang="en">Publication Event</rdfs:label>
        <rdfs:subClassOf rdf:resource="&owl;Thing"/>
        <rdfs:comment xml:lang="en">To describe any manifestation of a media
            resource on any media (live, on demand, catch-up TV, etc.) and the appropriate
            PublciationChannel.</rdfs:comment>
    </owl:Class>
    


    <!-- http://www.ebu.ch/metadata/ontologies/ebucore/ebucore#PublicationHistory -->

    <owl:Class rdf:about="&ebucore;PublicationHistory">
        <rdfs:label xml:lang="en">Publication History</rdfs:label>
        <rdfs:subClassOf rdf:resource="&owl;Thing"/>
        <rdfs:comment xml:lang="en">A collection of PublicationEvents through which
            a resource has been published.</rdfs:comment>
    </owl:Class>
    


    <!-- http://www.ebu.ch/metadata/ontologies/ebucore/ebucore#PublicationPlanning -->

    <owl:Class rdf:about="&ebucore;PublicationPlanning">
        <rdfs:label xml:lang="en">Publication History</rdfs:label>
        <rdfs:subClassOf rdf:resource="&owl;Thing"/>
        <rdfs:comment xml:lang="en">A collection of PublicationEvents organised as a PublicationPlanning.</rdfs:comment>
    </owl:Class>
    


    <!-- http://www.ebu.ch/metadata/ontologies/ebucore/ebucore#RadioProgramme -->

    <owl:Class rdf:about="&ebucore;RadioProgramme">
        <rdfs:label xml:lang="en">Radio Programme</rdfs:label>
        <rdfs:subClassOf rdf:resource="&ebucore;Programme"/>
        <rdfs:comment xml:lang="en">A programme for distribution on radio
            channels.</rdfs:comment>
    </owl:Class>
    


    <!-- http://www.ebu.ch/metadata/ontologies/ebucore/ebucore#Rating -->

    <owl:Class rdf:about="&ebucore;Rating">
        <rdfs:label xml:lang="en">Rating</rdfs:label>
        <rdfs:subClassOf rdf:resource="&owl;Thing"/>
        <rdfs:comment xml:lang="en">All the information about the rating/evaluation
            given to a media resource by an Agent i.e. a person/Contact or
            Organisation.</rdfs:comment>
        <rdfs:comment xml:lang="en">This is provided as free text in an annotation
            label or as an identifier pointing to a term in a classification scheme.</rdfs:comment>
    </owl:Class>
    


    <!-- http://www.ebu.ch/metadata/ontologies/ebucore/ebucore#Resource -->

    <owl:Class rdf:about="&ebucore;Resource">
        <rdfs:label xml:lang="en">Resource</rdfs:label>
        <rdfs:subClassOf rdf:resource="&owl;Thing"/>
        <rdfs:comment xml:lang="en">A manifestation of a
            BusinessObject.</rdfs:comment>
    </owl:Class>
    


    <!-- http://www.ebu.ch/metadata/ontologies/ebucore/ebucore#Rights -->

    <owl:Class rdf:about="&ebucore;Rights">
        <rdfs:label xml:lang="en">Rights</rdfs:label>
        <rdfs:subClassOf rdf:resource="&owl;Thing"/>
        <rdfs:comment xml:lang="en">To provide information on the rights, including
            intellectual property, related to a BusinessObject or Resource.</rdfs:comment>
    </owl:Class>
    


    <!-- http://www.ebu.ch/metadata/ontologies/ebucore/ebucore#RightsClearance -->

    <owl:Class rdf:about="&ebucore;RightsClearance">
        <rdfs:subClassOf rdf:resource="&ebucore;Rights"/>
        <rdfs:comment xml:lang="en">To signal that rights have been cleared (or
            not)</rdfs:comment>
    </owl:Class>
    


    <!-- http://www.ebu.ch/metadata/ontologies/ebucore/ebucore#Role -->

    <owl:Class rdf:about="&ebucore;Role">
        <rdfs:label xml:lang="en">Role</rdfs:label>
        <rdfs:subClassOf rdf:resource="&skos;Concept"/>
        <rdfs:comment xml:lang="en">To define the role / action of an agent. This
            is provided as free text in an annotation label or as an identifier pointing to a term
            in a classification scheme.</rdfs:comment>
    </owl:Class>
    


    <!-- http://www.ebu.ch/metadata/ontologies/ebucore/ebucore#Season -->

    <owl:Class rdf:about="&ebucore;Season">
        <rdfs:label rdf:datatype="&xsd;string">Season</rdfs:label>
        <rdfs:subClassOf rdf:resource="&ebucore;Group"/>
        <rdfs:comment rdf:datatype="&xsd;string">A series can be composed of one or more seasons
            clustering a certain number of episodes. Fro this reason, seasons are related to series
            using the isRelatedTo property.</rdfs:comment>
    </owl:Class>
    


    <!-- http://www.ebu.ch/metadata/ontologies/ebucore/ebucore#Series -->

    <owl:Class rdf:about="&ebucore;Series">
        <rdfs:label rdf:datatype="&xsd;string">Series</rdfs:label>
        <rdfs:subClassOf rdf:resource="&ebucore;Group"/>
        <rdfs:comment rdf:datatype="&xsd;string">Series is a particular type of collection. TV
            or Radio Series are composed of Episodes.</rdfs:comment>
    </owl:Class>
    


    <!-- http://www.ebu.ch/metadata/ontologies/ebucore/ebucore#Service -->

    <owl:Class rdf:about="&ebucore;Service">
        <rdfs:label xml:lang="en">Service</rdfs:label>
        <rdfs:subClassOf rdf:resource="&owl;Thing"/>
        <rdfs:comment xml:lang="en">A service is the umbrella under which one or
            more PublicationChannel is operated.</rdfs:comment>
    </owl:Class>
    


    <!-- http://www.ebu.ch/metadata/ontologies/ebucore/ebucore#Signing -->

    <owl:Class rdf:about="&ebucore;Signing">
        <rdfs:label xml:lang="en">Signing</rdfs:label>
        <rdfs:subClassOf rdf:resource="&ebucore;VideoTrack"/>
        <rdfs:comment xml:lang="en">To signal the presence of Signing for hard of
            hearing users. The type of Signing (e.g. incursted in or else) or language of Signing
            can be specified using the appropriate properties.</rdfs:comment>
    </owl:Class>
    


    <!-- http://www.ebu.ch/metadata/ontologies/ebucore/ebucore#SigningFormat -->

    <owl:Class rdf:about="&ebucore;SigningFormat">
        <rdfs:label xml:lang="en">Signing format</rdfs:label>
        <rdfs:subClassOf rdf:resource="&ebucore;VideoFormat"/>
        <rdfs:comment xml:lang="en">To provide additional information on the
            signing format. This is provided as free text in an annotation label or as an identifier
            pointing to a term in a classification scheme.</rdfs:comment>
    </owl:Class>
    


    <!-- http://www.ebu.ch/metadata/ontologies/ebucore/ebucore#SportItem -->

    <owl:Class rdf:about="&ebucore;SportItem">
        <rdfs:label xml:lang="en">Sport item</rdfs:label>
        <rdfs:subClassOf rdf:resource="&ebucore;Item"/>
        <rdfs:comment xml:lang="en">A SportItem aggregates all information about a sport event.</rdfs:comment>
    </owl:Class>
    


    <!-- http://www.ebu.ch/metadata/ontologies/ebucore/ebucore#Staff -->

    <owl:Class rdf:about="&ebucore;Staff">
        <rdfs:label xml:lang="en">Staff member.</rdfs:label>
        <rdfs:subClassOf rdf:resource="&ebucore;Agent"/>
        <rdfs:comment xml:lang="en">Staff or crew member.</rdfs:comment>
    </owl:Class>
    


    <!-- http://www.ebu.ch/metadata/ontologies/ebucore/ebucore#StorageType -->

    <owl:Class rdf:about="&ebucore;StorageType">
        <rdfs:label xml:lang="en">Storage type</rdfs:label>
        <rdfs:subClassOf rdf:resource="&skos;Concept"/>
        <rdfs:comment xml:lang="en">The type of storage used for the repository.
            This is provided as free text in an annotation label or as an identifier pointing to a
            term in a classification scheme.</rdfs:comment>
    </owl:Class>
    


    <!-- http://www.ebu.ch/metadata/ontologies/ebucore/ebucore#Stream -->

    <owl:Class rdf:about="&ebucore;Stream">
        <rdfs:label xml:lang="en">Stream</rdfs:label>
        <rdfs:subClassOf rdf:resource="&ebucore;Component"/>
        <rdfs:comment xml:lang="en">A continuous stream of bits.</rdfs:comment>
    </owl:Class>
    


    <!-- http://www.ebu.ch/metadata/ontologies/ebucore/ebucore#Subject -->

    <owl:Class rdf:about="&ebucore;Subject">
        <rdfs:label xml:lang="en">Subject</rdfs:label>
        <rdfs:subClassOf rdf:resource="&skos;Concept"/>
        <rdfs:comment xml:lang="en">A term describing the topic covered by the
            BusinessObject or resource. This is provided as free text in an annotation label or as
            an identifier pointing to a term in a classification scheme.</rdfs:comment>
    </owl:Class>
    


    <!-- http://www.ebu.ch/metadata/ontologies/ebucore/ebucore#Subtitling -->

    <owl:Class rdf:about="&ebucore;Subtitling">
        <rdfs:label xml:lang="en">Subtitling</rdfs:label>
        <rdfs:subClassOf rdf:resource="&ebucore;DataTrack"/>
        <rdfs:comment xml:lang="en">To signal the presence of subtitles for
            translation in alternative languages.</rdfs:comment>
    </owl:Class>
    


    <!-- http://www.ebu.ch/metadata/ontologies/ebucore/ebucore#SubtitlingFormat -->

    <owl:Class rdf:about="&ebucore;SubtitlingFormat">
        <rdfs:label xml:lang="en">Subtitling format</rdfs:label>
        <rdfs:subClassOf rdf:resource="&ebucore;DataFormat"/>
        <rdfs:comment xml:lang="en">To define the format of subtitling.
            subtitling&apos;s main use isfor translation. This is provided as free text in an
            annotation label  or as an identifier pointing to a term in a classification
            scheme.</rdfs:comment>
    </owl:Class>
    


    <!-- http://www.ebu.ch/metadata/ontologies/ebucore/ebucore#TVProgramme -->

    <owl:Class rdf:about="&ebucore;TVProgramme">
        <rdfs:label xml:lang="en">TV Programme</rdfs:label>
        <rdfs:subClassOf rdf:resource="&ebucore;Programme"/>
        <rdfs:comment xml:lang="en">A programme for distribution on television
            channels.</rdfs:comment>
    </owl:Class>
    


    <!-- http://www.ebu.ch/metadata/ontologies/ebucore/ebucore#Tag -->

    <owl:Class rdf:about="&ebucore;Tag">
        <rdfs:label rdf:datatype="&xsd;string">Tag</rdfs:label>
        <rdfs:subClassOf rdf:resource="&ebucore;Annotation"/>
        <rdfs:comment rdf:datatype="&xsd;string">An annotation specific to a particular
            timestamp in audiovisual MediaResources.</rdfs:comment>
    </owl:Class>
    


    <!-- http://www.ebu.ch/metadata/ontologies/ebucore/ebucore#Thumbnail -->

    <owl:Class rdf:about="&ebucore;Thumbnail">
        <rdfs:label xml:lang="en">Thumbnail</rdfs:label>
        <rdfs:subClassOf rdf:resource="&ebucore;Picture"/>
        <rdfs:comment xml:lang="en">A thumbnail is a low resolution picture that
            can be associated with EditorialObjects or e.g. MediaResources or
            Contacts.</rdfs:comment>
    </owl:Class>
    


    <!-- http://www.ebu.ch/metadata/ontologies/ebucore/ebucore#TimecodeTrack -->

    <owl:Class rdf:about="&ebucore;TimecodeTrack">
        <rdfs:label rdf:datatype="&xsd;string">Timecode track</rdfs:label>
        <rdfs:subClassOf rdf:resource="&ebucore;Track"/>
        <rdfs:comment rdf:datatype="&xsd;string">A track with timecode information.</rdfs:comment>
    </owl:Class>
    


    <!-- http://www.ebu.ch/metadata/ontologies/ebucore/ebucore#Topic -->

    <owl:Class rdf:about="&ebucore;Topic">
        <rdfs:label xml:lang="en">Topic</rdfs:label>
        <rdfs:subClassOf rdf:resource="&ebucore;Subject"/>
        <rdfs:comment xml:lang="en">A type subject for use in some contexts. This
            is provided as free text in an annotation label or as an identifier pointing to a term
            in a classification scheme.</rdfs:comment>
    </owl:Class>
    


    <!-- http://www.ebu.ch/metadata/ontologies/ebucore/ebucore#Track -->

    <owl:Class rdf:about="&ebucore;Track">
        <rdfs:label xml:lang="en">Track</rdfs:label>
        <rdfs:subClassOf rdf:resource="&ebucore;Essence"/>
        <rdfs:comment xml:lang="en">Audiovisual content can be composed of audio,
            video and data Tracks (including captioning and subtitling).</rdfs:comment>
    </owl:Class>
    


    <!-- http://www.ebu.ch/metadata/ontologies/ebucore/ebucore#Type -->

    <owl:Class rdf:about="&ebucore;Type">
        <rdfs:label xml:lang="en">Type</rdfs:label>
        <rdfs:subClassOf rdf:resource="&skos;Concept"/>
        <rdfs:comment xml:lang="en">An expression of type in textual form or as a term from a classification scheme.</rdfs:comment>
    </owl:Class>
    


    <!-- http://www.ebu.ch/metadata/ontologies/ebucore/ebucore#UsageRights -->

    <owl:Class rdf:about="&ebucore;UsageRights">
        <rdfs:label xml:lang="en">Usage rights</rdfs:label>
        <rdfs:subClassOf rdf:resource="&ebucore;Rights"/>
        <rdfs:comment xml:lang="en">Usage rights associated with content.</rdfs:comment>
    </owl:Class>
    


    <!-- http://www.ebu.ch/metadata/ontologies/ebucore/ebucore#VideoEncodingFormat -->

    <owl:Class rdf:about="&ebucore;VideoEncodingFormat">
        <rdfs:label xml:lang="en">Video encoding format</rdfs:label>
        <rdfs:subClassOf rdf:resource="&ebucore;EncodingFormat"/>
        <rdfs:comment xml:lang="en">The encoding format of the video.</rdfs:comment>
    </owl:Class>
    


    <!-- http://www.ebu.ch/metadata/ontologies/ebucore/ebucore#VideoFormat -->

    <owl:Class rdf:about="&ebucore;VideoFormat">
        <rdfs:label xml:lang="en">Video format</rdfs:label>
        <rdfs:subClassOf rdf:resource="&ebucore;Format"/>
        <rdfs:comment xml:lang="en">To provide additional technical information
            about a video resource such as the frame rate. This is provided as free text in an
            annotation label or as an identifier pointing to a term in a classification
            scheme.</rdfs:comment>
    </owl:Class>
    


    <!-- http://www.ebu.ch/metadata/ontologies/ebucore/ebucore#VideoStream -->

    <owl:Class rdf:about="&ebucore;VideoStream">
        <rdfs:label xml:lang="en">Video stream</rdfs:label>
        <rdfs:subClassOf rdf:resource="&ebucore;Stream"/>
        <rdfs:comment xml:lang="en">A decodable video stream of bits.</rdfs:comment>
    </owl:Class>
    


    <!-- http://www.ebu.ch/metadata/ontologies/ebucore/ebucore#VideoTrack -->

    <owl:Class rdf:about="&ebucore;VideoTrack">
        <rdfs:label xml:lang="en">Video track</rdfs:label>
        <rdfs:subClassOf rdf:resource="&ebucore;Track"/>
        <rdfs:comment xml:lang="en">A specialisation of Track for Video to provide
            a link to specific data properties such as frameRate, etc. Signing is another possible
            example of video track. Specific VideoTracks such as Signing can be defined as sub
            VideoTracks.. In advanced systems, different VideoTracks can be used to provide e.g.
            different viewing angles.</rdfs:comment>
    </owl:Class>
    


    <!-- http://www.ebu.ch/metadata/ontologies/ebucore/ebucore#YouTubeVideo -->

    <owl:Class rdf:about="&ebucore;YouTubeVideo">
        <rdfs:label rdf:datatype="&xsd;string">You tube video</rdfs:label>
        <rdfs:subClassOf rdf:resource="&ebucore;MediaResource"/>
    </owl:Class>
    


    <!-- http://www.ebu.ch/metadata/ontologies/ebucore/ebucore#audienceLevel -->

    <owl:Class rdf:about="&ebucore;audienceLevel">
        <rdfs:label xml:lang="en">Target audience</rdfs:label>
        <rdfs:subClassOf rdf:resource="&ebucore;Type"/>
        <rdfs:comment xml:lang="en">The target audience (target region, target
            audience category but also parental guidance recommendation) for which the media
            resource is intended.</rdfs:comment>
        <rdfs:comment xml:lang="en">This is provided as free text in an annotation
            label or as an identifier pointing to a term in a classification scheme.</rdfs:comment>
    </owl:Class>
    


    <!-- http://www.w3.org/2004/02/skos/core#Concept -->

    <rdf:Description rdf:about="&skos;Concept">
        <rdfs:isDefinedBy rdf:resource="http://www.w3.org/2004/02/skos/core"/>
    </rdf:Description>
    


    <!-- http://xmlns.com/foaf/0.1/Agent -->

    <owl:Class rdf:about="&foaf;Agent">
        <rdfs:label xml:lang="en">Agent</rdfs:label>
        <rdfs:subClassOf rdf:resource="&dc;Agent"/>
        <rdfs:comment xml:lang="en">A person or Organisation.</rdfs:comment>
    </owl:Class>
    


    <!-- http://xmlns.com/foaf/0.1/Group -->

    <owl:Class rdf:about="&foaf;Group">
        <rdfs:label xml:lang="en">Group</rdfs:label>
        <rdfs:subClassOf rdf:resource="&owl;Thing"/>
        <rdfs:comment xml:lang="en">A group of Agents.</rdfs:comment>
    </owl:Class>
    


    <!-- http://xmlns.com/foaf/0.1/Organization -->

    <owl:Class rdf:about="&foaf;Organization">
        <rdfs:label xml:lang="en">Organization</rdfs:label>
        <rdfs:subClassOf rdf:resource="&ebucore;Organisation"/>
        <rdfs:comment xml:lang="en">An organisation (business, corporation, federation, etc.) or moral agent (gvernment body).</rdfs:comment>
    </owl:Class>
    


    <!-- http://xmlns.com/foaf/0.1/img -->

    <owl:Class rdf:about="&foaf;img">
        <rdfs:label xml:lang="en">Image</rdfs:label>
        <rdfs:subClassOf rdf:resource="&ebucore;Picture"/>
        <rdfs:comment xml:lang="en">Animage to represent something.</rdfs:comment>
    </owl:Class>
    


    <!-- http://xmlns.com/foaf/0.1/person -->

    <owl:Class rdf:about="&foaf;person">
        <rdfs:label xml:lang="en">Person</rdfs:label>
        <rdfs:subClassOf rdf:resource="&ebucore;Contact"/>
        <rdfs:comment xml:lang="en">all types of people such as politicians, athletes, historic figures, contributors in programmes e.t.c.</rdfs:comment>
    </owl:Class>
    


    <!-- 
    ///////////////////////////////////////////////////////////////////////////////////////
    //
    // Annotations
    //
    ///////////////////////////////////////////////////////////////////////////////////////
     -->

    <rdf:Description rdf:about="&core;placeOfDeath">
        <rdfs:label xml:lang="en">Place of death</rdfs:label>
        <rdfs:comment xml:lang="en">The place where a person has passed away.</rdfs:comment>
    </rdf:Description>
    <rdf:Description rdf:about="&skos;narrowerTransitive">
        <rdfs:isDefinedBy rdf:resource="http://www.w3.org/2004/02/skos/core"/>
    </rdf:Description>
    <rdf:Description rdf:about="&dct;publisher">
        <rdfs:label xml:lang="en">Publisher</rdfs:label>
    </rdf:Description>
    <rdf:Description rdf:about="&skos;related">
        <rdfs:isDefinedBy rdf:resource="http://www.w3.org/2004/02/skos/core"/>
    </rdf:Description>
    <rdf:Description rdf:about="&dct;creator">
        <rdfs:label xml:lang="en">Creator</rdfs:label>
    </rdf:Description>
    <rdf:Description rdf:about="&skos;semanticRelation">
        <rdfs:isDefinedBy rdf:resource="http://www.w3.org/2004/02/skos/core"/>
    </rdf:Description>
    <rdf:Description rdf:about="&skos;altLabel">
        <rdfs:isDefinedBy rdf:resource="http://www.w3.org/2004/02/skos/core"/>
    </rdf:Description>
    <rdf:Description rdf:about="&skos;example">
        <rdfs:isDefinedBy rdf:resource="http://www.w3.org/2004/02/skos/core"/>
    </rdf:Description>
    <rdf:Description rdf:about="&skos;editorialNote">
        <rdfs:isDefinedBy rdf:resource="http://www.w3.org/2004/02/skos/core"/>
    </rdf:Description>
    <rdf:Description rdf:about="&skos;inScheme">
        <rdfs:isDefinedBy rdf:resource="http://www.w3.org/2004/02/skos/core"/>
    </rdf:Description>
    <rdf:Description rdf:about="&skos;hasTopConcept">
        <rdfs:isDefinedBy rdf:resource="http://www.w3.org/2004/02/skos/core"/>
    </rdf:Description>
    <rdf:Description rdf:about="&skos;topConceptOf">
        <rdfs:isDefinedBy rdf:resource="http://www.w3.org/2004/02/skos/core"/>
    </rdf:Description>
    <rdf:Description rdf:about="&dct;relation">
        <rdfs:label xml:lang="en">Relation</rdfs:label>
    </rdf:Description>
    <rdf:Description rdf:about="&skos;memberList">
        <rdfs:isDefinedBy rdf:resource="http://www.w3.org/2004/02/skos/core"/>
    </rdf:Description>
    <rdf:Description rdf:about="&dct;format">
        <rdfs:label xml:lang="en">format</rdfs:label>
    </rdf:Description>
    <rdf:Description rdf:about="&skos;definition">
        <rdfs:isDefinedBy rdf:resource="http://www.w3.org/2004/02/skos/core"/>
    </rdf:Description>
    <rdf:Description rdf:about="&skos;broadMatch">
        <rdfs:isDefinedBy rdf:resource="http://www.w3.org/2004/02/skos/core"/>
    </rdf:Description>
    <rdf:Description rdf:about="&dct;type">
        <rdfs:label xml:lang="en">type</rdfs:label>
    </rdf:Description>
    <rdf:Description rdf:about="&skos;exactMatch">
        <rdfs:isDefinedBy rdf:resource="http://www.w3.org/2004/02/skos/core"/>
    </rdf:Description>
    <rdf:Description rdf:about="&dct;language">
        <rdfs:label xml:lang="en">language</rdfs:label>
    </rdf:Description>
    <rdf:Description rdf:about="&core;placeOfBirth">
        <rdfs:label xml:lang="en">Place of birth</rdfs:label>
        <rdfs:comment xml:lang="en">The place where a person is born.</rdfs:comment>
    </rdf:Description>
    <rdf:Description rdf:about="&skos;member">
        <rdfs:isDefinedBy rdf:resource="http://www.w3.org/2004/02/skos/core"/>
    </rdf:Description>
    <rdf:Description rdf:about="&skos;closeMatch">
        <rdfs:isDefinedBy rdf:resource="http://www.w3.org/2004/02/skos/core"/>
    </rdf:Description>
    <rdf:Description rdf:about="&skos;broaderTransitive">
        <rdfs:isDefinedBy rdf:resource="http://www.w3.org/2004/02/skos/core"/>
    </rdf:Description>
    <rdf:Description rdf:about="&skos;relatedMatch">
        <rdfs:isDefinedBy rdf:resource="http://www.w3.org/2004/02/skos/core"/>
    </rdf:Description>
    <rdf:Description rdf:about="&skos;changeNote">
        <rdfs:isDefinedBy rdf:resource="http://www.w3.org/2004/02/skos/core"/>
    </rdf:Description>
    <rdf:Description rdf:about="&skos;mappingRelation">
        <rdfs:isDefinedBy rdf:resource="http://www.w3.org/2004/02/skos/core"/>
    </rdf:Description>
    <rdf:Description rdf:about="&dct;rights">
        <rdfs:label xml:lang="en">Rights</rdfs:label>
    </rdf:Description>
    <rdf:Description rdf:about="&skos;broader">
        <rdfs:isDefinedBy rdf:resource="http://www.w3.org/2004/02/skos/core"/>
    </rdf:Description>
    <rdf:Description rdf:about="&skos;scopeNote">
        <rdfs:isDefinedBy rdf:resource="http://www.w3.org/2004/02/skos/core"/>
    </rdf:Description>
    <rdf:Description rdf:about="&skos;OrderedCollection">
        <rdfs:isDefinedBy rdf:resource="http://www.w3.org/2004/02/skos/core"/>
    </rdf:Description>
    <rdf:Description rdf:about="&dct;subject">
        <rdfs:label xml:lang="en">Subject</rdfs:label>
    </rdf:Description>
    <rdf:Description rdf:about="&skos;narrower">
        <rdfs:isDefinedBy rdf:resource="http://www.w3.org/2004/02/skos/core"/>
    </rdf:Description>
    <rdf:Description rdf:about="&skos;notation">
        <rdfs:isDefinedBy rdf:resource="http://www.w3.org/2004/02/skos/core"/>
    </rdf:Description>
    <rdf:Description rdf:about="&skos;narrowMatch">
        <rdfs:isDefinedBy rdf:resource="http://www.w3.org/2004/02/skos/core"/>
    </rdf:Description>
    <rdf:Description rdf:about="&dct;source">
        <rdfs:label xml:lang="en">Source</rdfs:label>
    </rdf:Description>
    <rdf:Description rdf:about="&skos;Collection">
        <rdfs:isDefinedBy rdf:resource="http://www.w3.org/2004/02/skos/core"/>
    </rdf:Description>
    <rdf:Description rdf:about="&dct;coverage">
        <rdfs:label xml:lang="en">coverage</rdfs:label>
    </rdf:Description>
    <rdf:Description rdf:about="&skos;historyNote">
        <rdfs:isDefinedBy rdf:resource="http://www.w3.org/2004/02/skos/core"/>
    </rdf:Description>
    <rdf:Description rdf:about="&skos;hiddenLabel">
        <rdfs:isDefinedBy rdf:resource="http://www.w3.org/2004/02/skos/core"/>
    </rdf:Description>
    <rdf:Description rdf:about="&dct;contributor">
        <rdfs:label xml:lang="en">contributor</rdfs:label>
    </rdf:Description>
    <rdf:Description rdf:about="&skos;ConceptScheme">
        <rdfs:isDefinedBy rdf:resource="http://www.w3.org/2004/02/skos/core"/>
    </rdf:Description>
    <rdf:Description rdf:about="&skos;note">
        <rdfs:isDefinedBy rdf:resource="http://www.w3.org/2004/02/skos/core"/>
    </rdf:Description>
</rdf:RDF>



<!-- Generated by the OWL API (version 3.4.2) http://owlapi.sourceforge.net -->

